<?xml version="1.0"?>
<rdf:RDF xmlns="http://purl.org/auto/criticality_phenomena#"
     xml:base="http://purl.org/auto/criticality_phenomena"
     xmlns:cp="http://purl.org/auto/criticality_phenomena#"
     xmlns:owl="http://www.w3.org/2002/07/owl#"
     xmlns:rdf="http://www.w3.org/1999/02/22-rdf-syntax-ns#"
     xmlns:xml="http://www.w3.org/XML/1998/namespace"
     xmlns:xsd="http://www.w3.org/2001/XMLSchema#"
     xmlns:auto="http://purl.org/auto/"
     xmlns:rdfs="http://www.w3.org/2000/01/rdf-schema#"
     xmlns:dcterms="http://purl.org/dc/terms/">
    <owl:Ontology rdf:about="http://purl.org/auto/criticality_phenomena"/>
    


    <!-- 
    ///////////////////////////////////////////////////////////////////////////////////////
    //
    // Annotation properties
    //
    ///////////////////////////////////////////////////////////////////////////////////////
     -->

    


    <!-- http://purl.org/auto/criticality_phenomena#formalized -->

    <owl:AnnotationProperty rdf:about="http://purl.org/auto/criticality_phenomena#formalized"/>
    


    <!-- http://purl.org/dc/terms/identifier -->

    <owl:AnnotationProperty rdf:about="http://purl.org/dc/terms/identifier"/>
    


    <!-- 
    ///////////////////////////////////////////////////////////////////////////////////////
    //
    // Classes
    //
    ///////////////////////////////////////////////////////////////////////////////////////
     -->

    


    <!-- http://purl.org/auto/criticality_phenomena#Behavioral_Criticality_Phenomenon -->

    <owl:Class rdf:about="http://purl.org/auto/criticality_phenomena#Behavioral_Criticality_Phenomenon">
        <rdfs:subClassOf rdf:resource="http://purl.org/auto/criticality_phenomena#Tagged_Criticality_Phenomenon"/>
        <rdfs:label xml:lang="en">Behavioral Criticality Phenomenon</rdfs:label>
        <rdfs:label xml:lang="de">Verhaltens_Kritikalitätsphänomen</rdfs:label>
    </owl:Class>
    


    <!-- http://purl.org/auto/criticality_phenomena#CP_0 -->

    <owl:Class rdf:about="http://purl.org/auto/criticality_phenomena#CP_0">
        <rdfs:subClassOf rdf:resource="http://purl.org/auto/criticality_phenomena#CP_255"/>
        <rdfs:subClassOf rdf:resource="http://purl.org/auto/criticality_phenomena#Perfect_Perception_Criticality_Phenomenon"/>
        <dcterms:identifier rdf:datatype="http://www.w3.org/2001/XMLSchema#nonNegativeInteger">0</dcterms:identifier>
        <rdfs:comment xml:lang="en">Public transport vehicles show special behaviour which must be responded to.</rdfs:comment>
        <rdfs:label xml:lang="en">Behaviour of public transport vehicles</rdfs:label>
        <rdfs:label xml:lang="de">Verhalten von öffentlichen Verkehrsmitteln</rdfs:label>
    </owl:Class>
    


    <!-- http://purl.org/auto/criticality_phenomena#CP_1 -->

    <owl:Class rdf:about="http://purl.org/auto/criticality_phenomena#CP_1">
        <rdfs:subClassOf rdf:resource="http://purl.org/auto/criticality_phenomena#Behavioral_Criticality_Phenomenon"/>
        <rdfs:subClassOf rdf:resource="http://purl.org/auto/criticality_phenomena#CP_0"/>
        <dcterms:identifier rdf:datatype="http://www.w3.org/2001/XMLSchema#nonNegativeInteger">1</dcterms:identifier>
        <rdfs:comment xml:lang="en">A bus is indicating to its left. It therefore has right of way.</rdfs:comment>
        <rdfs:label xml:lang="en">Left indicating bus</rdfs:label>
        <rdfs:label xml:lang="de">Links blinkender Bus</rdfs:label>
    </owl:Class>
    


    <!-- http://purl.org/auto/criticality_phenomena#CP_10 -->

    <owl:Class rdf:about="http://purl.org/auto/criticality_phenomena#CP_10">
        <rdfs:subClassOf rdf:resource="http://purl.org/auto/criticality_phenomena#CP_212"/>
        <rdfs:subClassOf rdf:resource="http://purl.org/auto/criticality_phenomena#Perfect_Perception_Criticality_Phenomenon"/>
        <dcterms:identifier rdf:datatype="http://www.w3.org/2001/XMLSchema#nonNegativeInteger">10</dcterms:identifier>
        <rdfs:comment xml:lang="en">A pile of objects is present on the road which is either trash (e.g. from a fallen trash can) or lost cargo (e.g. from a truck). May or may not be overridable.</rdfs:comment>
        <rdfs:label xml:lang="en">Cargo/trash On Road</rdfs:label>
        <rdfs:label xml:lang="de">Ladung/Müll auf der Straße</rdfs:label>
    </owl:Class>
    


    <!-- http://purl.org/auto/criticality_phenomena#CP_100 -->

    <owl:Class rdf:about="http://purl.org/auto/criticality_phenomena#CP_100">
        <rdfs:subClassOf rdf:resource="http://purl.org/auto/criticality_phenomena#CP_216"/>
        <rdfs:subClassOf rdf:resource="http://purl.org/auto/criticality_phenomena#Perfect_Perception_Criticality_Phenomenon"/>
        <dcterms:identifier rdf:datatype="http://www.w3.org/2001/XMLSchema#nonNegativeInteger">100</dcterms:identifier>
        <rdfs:comment xml:lang="en">Refers to motorcyclist who push-to-front between or next to waiting vehicles, e.g. at a closed railroad crossing, a red traffic light or in a traffic jam.</rdfs:comment>
        <rdfs:label xml:lang="de">Non-Ego-TP Drängelnder Motorradfahrer</rdfs:label>
        <rdfs:label xml:lang="en">Push-to-front Of Motorcyclists</rdfs:label>
    </owl:Class>
    


    <!-- http://purl.org/auto/criticality_phenomena#CP_101 -->

    <owl:Class rdf:about="http://purl.org/auto/criticality_phenomena#CP_101">
        <rdfs:subClassOf rdf:resource="http://purl.org/auto/criticality_phenomena#CP_288"/>
        <rdfs:subClassOf rdf:resource="http://purl.org/auto/criticality_phenomena#Perfect_Perception_Criticality_Phenomenon"/>
        <dcterms:identifier rdf:datatype="http://www.w3.org/2001/XMLSchema#nonNegativeInteger">101</dcterms:identifier>
        <rdfs:comment xml:lang="en">A traffic jam reaches into an intersection area.</rdfs:comment>
        <rdfs:label xml:lang="en">Backlog On Intersection</rdfs:label>
        <rdfs:label xml:lang="de">Rückstau an Kreuzung</rdfs:label>
    </owl:Class>
    


    <!-- http://purl.org/auto/criticality_phenomena#CP_102 -->

    <owl:Class rdf:about="http://purl.org/auto/criticality_phenomena#CP_102">
        <rdfs:subClassOf rdf:resource="http://purl.org/auto/criticality_phenomena#CP_101"/>
        <dcterms:identifier rdf:datatype="http://www.w3.org/2001/XMLSchema#nonNegativeInteger">102</dcterms:identifier>
        <rdfs:comment xml:lang="en">A traffic jam reaches onto a turn lane (e.g. on a right turn lane on an intersection).</rdfs:comment>
        <rdfs:label xml:lang="en">Backlog On Turn Lane</rdfs:label>
        <rdfs:label xml:lang="de">Rückstau auf Abbiegefahrstreifen</rdfs:label>
    </owl:Class>
    


    <!-- http://purl.org/auto/criticality_phenomena#CP_103 -->

    <owl:Class rdf:about="http://purl.org/auto/criticality_phenomena#CP_103">
        <rdfs:subClassOf rdf:resource="http://purl.org/auto/criticality_phenomena#CP_216"/>
        <rdfs:subClassOf rdf:resource="http://purl.org/auto/criticality_phenomena#Perfect_Perception_Criticality_Phenomenon"/>
        <dcterms:identifier rdf:datatype="http://www.w3.org/2001/XMLSchema#nonNegativeInteger">103</dcterms:identifier>
        <rdfs:comment xml:lang="en">Strong refers to braking maneuvers with a force of 0.47G = 4.61m/s^2 or higher 
(force that the average driver can handle safely according to https://copradar.com/chapts/references/acceleration.html) in the case of Non-Ego-TP.

In the case of the Ego &apos;strong&apos; depends on the capabilities of the automated driving system.
</rdfs:comment>
        <rdfs:label xml:lang="de">Starkes Bremsmanöver von Ego/Non-Ego-TP</rdfs:label>
        <rdfs:label xml:lang="en">Strong Braking Maneuver Of Ego/non-ego-tp</rdfs:label>
    </owl:Class>
    


    <!-- http://purl.org/auto/criticality_phenomena#CP_104 -->

    <owl:Class rdf:about="http://purl.org/auto/criticality_phenomena#CP_104">
        <rdfs:subClassOf rdf:resource="http://purl.org/auto/criticality_phenomena#CP_216"/>
        <rdfs:subClassOf rdf:resource="http://purl.org/auto/criticality_phenomena#Perfect_Perception_Criticality_Phenomenon"/>
        <dcterms:identifier rdf:datatype="http://www.w3.org/2001/XMLSchema#nonNegativeInteger">104</dcterms:identifier>
        <rdfs:comment xml:lang="en">Unexpected braking of ego or non-ego-TPs refers to braking maneuvers that cannot be anticipated by other TPs or ego from the learned norm behavior of traffic participants (hard to quantify).</rdfs:comment>
        <rdfs:label xml:lang="en">Unexpected Braking Maneuver Of Ego/non-ego-tp</rdfs:label>
        <rdfs:label xml:lang="de">unerwartetes Bremsmanöver von Ego/Non-Ego-TP</rdfs:label>
    </owl:Class>
    


    <!-- http://purl.org/auto/criticality_phenomena#CP_105 -->

    <owl:Class rdf:about="http://purl.org/auto/criticality_phenomena#CP_105">
        <rdfs:subClassOf rdf:resource="http://purl.org/auto/criticality_phenomena#CP_216"/>
        <rdfs:subClassOf rdf:resource="http://purl.org/auto/criticality_phenomena#Perfect_Perception_Criticality_Phenomenon"/>
        <dcterms:identifier rdf:datatype="http://www.w3.org/2001/XMLSchema#nonNegativeInteger">105</dcterms:identifier>
        <rdfs:comment xml:lang="en">ToDo: Reference for strong steering for (average) human drivers needed.

In the case of the Ego &apos;strong&apos; depends on the capabilities of the automated driving system.</rdfs:comment>
        <rdfs:label xml:lang="de">Starkes Lenkmanöver von Ego/Non-Ego-TP</rdfs:label>
        <rdfs:label xml:lang="en">Strong Steering Maneuver Of Ego/non-ego-tp</rdfs:label>
    </owl:Class>
    


    <!-- http://purl.org/auto/criticality_phenomena#CP_106 -->

    <owl:Class rdf:about="http://purl.org/auto/criticality_phenomena#CP_106">
        <rdfs:subClassOf rdf:resource="http://purl.org/auto/criticality_phenomena#CP_108"/>
        <rdfs:subClassOf rdf:resource="http://purl.org/auto/criticality_phenomena#Dynamical_Criticality_Phenomenon"/>
        <dcterms:identifier rdf:datatype="http://www.w3.org/2001/XMLSchema#nonNegativeInteger">106</dcterms:identifier>
        <rdfs:comment xml:lang="en">A TP which drives the opposite direction of ego cuts ego&apos;s lane due to an overtaking maneuver.</rdfs:comment>
        <rdfs:label xml:lang="de">Non-Ego-TP entgegenkommendes Fahrzeug schneidet Spur im Überholvorgang</rdfs:label>
        <rdfs:label xml:lang="en">Oncoming Overtaking Non-Ego-TP Cuts Lane</rdfs:label>
    </owl:Class>
    


    <!-- http://purl.org/auto/criticality_phenomena#CP_107 -->

    <owl:Class rdf:about="http://purl.org/auto/criticality_phenomena#CP_107">
        <rdfs:subClassOf rdf:resource="http://purl.org/auto/criticality_phenomena#CP_108"/>
        <dcterms:identifier rdf:datatype="http://www.w3.org/2001/XMLSchema#nonNegativeInteger">107</dcterms:identifier>
        <rdfs:comment xml:lang="en">A TP which drives the opposite direction of ego cuts ego&apos;s lane while driving in a curve.</rdfs:comment>
        <rdfs:label xml:lang="de">Non-Ego-TP entgegenkommendes Fahrzeug schneidet Fahrstreifen</rdfs:label>
        <rdfs:label xml:lang="en">Oncoming Turning Non-Ego-TP Cuts Lane</rdfs:label>
    </owl:Class>
    


    <!-- http://purl.org/auto/criticality_phenomena#CP_108 -->

    <owl:Class rdf:about="http://purl.org/auto/criticality_phenomena#CP_108">
        <rdfs:subClassOf rdf:resource="http://purl.org/auto/criticality_phenomena#CP_216"/>
        <rdfs:subClassOf rdf:resource="http://purl.org/auto/criticality_phenomena#Perfect_Perception_Criticality_Phenomenon"/>
        <dcterms:identifier rdf:datatype="http://www.w3.org/2001/XMLSchema#nonNegativeInteger">108</dcterms:identifier>
        <rdfs:comment xml:lang="en">Cutting into lane can occur during narrow passages or while performing a turn.

Large vehicle here means either at least 2,30m width or at least 6m length as to include busses, trucks, agricultural vehicles, etc. ToDo: Check these values.</rdfs:comment>
        <rdfs:label xml:lang="de">Entgegenkommendes großes Fahrzeug schneidet Spur</rdfs:label>
        <rdfs:label xml:lang="en">Oncoming Large Vehicle Cuts Into Lane</rdfs:label>
    </owl:Class>
    


    <!-- http://purl.org/auto/criticality_phenomena#CP_109 -->

    <owl:Class rdf:about="http://purl.org/auto/criticality_phenomena#CP_109">
        <rdfs:subClassOf rdf:resource="http://purl.org/auto/criticality_phenomena#CP_216"/>
        <rdfs:subClassOf rdf:resource="http://purl.org/auto/criticality_phenomena#Perfect_Perception_Criticality_Phenomenon"/>
        <dcterms:identifier rdf:datatype="http://www.w3.org/2001/XMLSchema#nonNegativeInteger">109</dcterms:identifier>
        <rdfs:comment xml:lang="en">A non-ego TP changes driving directions by turning on the road (e.g. a threeway turn or a U-turn).</rdfs:comment>
        <rdfs:label xml:lang="en">Non-Ego-TP Turning On Road</rdfs:label>
        <rdfs:label xml:lang="de">Non-Ego-TP Wenden auf der Straße</rdfs:label>
    </owl:Class>
    


    <!-- http://purl.org/auto/criticality_phenomena#CP_11 -->

    <owl:Class rdf:about="http://purl.org/auto/criticality_phenomena#CP_11">
        <rdfs:subClassOf rdf:resource="http://purl.org/auto/criticality_phenomena#CP_212"/>
        <rdfs:subClassOf rdf:resource="http://purl.org/auto/criticality_phenomena#Environmental_Criticality_Phenomenon"/>
        <rdfs:subClassOf rdf:resource="http://purl.org/auto/criticality_phenomena#Perfect_Perception_Criticality_Phenomenon"/>
        <dcterms:identifier rdf:datatype="http://www.w3.org/2001/XMLSchema#nonNegativeInteger">11</dcterms:identifier>
        <rdfs:comment xml:lang="en">A branch (meaning a bough, i.e. a large branch) is on the road. </rdfs:comment>
        <rdfs:label xml:lang="de">Ast auf der Straße</rdfs:label>
        <rdfs:label xml:lang="en">Branch On Road</rdfs:label>
    </owl:Class>
    


    <!-- http://purl.org/auto/criticality_phenomena#CP_110 -->

    <owl:Class rdf:about="http://purl.org/auto/criticality_phenomena#CP_110">
        <rdfs:subClassOf rdf:resource="http://purl.org/auto/criticality_phenomena#CP_109"/>
        <dcterms:identifier rdf:datatype="http://www.w3.org/2001/XMLSchema#nonNegativeInteger">110</dcterms:identifier>
        <rdfs:comment xml:lang="en">A non-ego TP performs a U-turn at a place where such a maneuver is not allowed.</rdfs:comment>
        <rdfs:label xml:lang="en">Illegitimate U-turn Of Non-Ego-TP</rdfs:label>
        <rdfs:label xml:lang="de">Non-Ego-TP Nichterlaubtes Wenden auf der Straße</rdfs:label>
    </owl:Class>
    


    <!-- http://purl.org/auto/criticality_phenomena#CP_111 -->

    <owl:Class rdf:about="http://purl.org/auto/criticality_phenomena#CP_111">
        <rdfs:subClassOf rdf:resource="http://purl.org/auto/criticality_phenomena#CP_216"/>
        <rdfs:subClassOf rdf:resource="http://purl.org/auto/criticality_phenomena#Perfect_Perception_Criticality_Phenomenon"/>
        <dcterms:identifier rdf:datatype="http://www.w3.org/2001/XMLSchema#nonNegativeInteger">111</dcterms:identifier>
        <rdfs:comment xml:lang="en">A TP is performing a parking maneuver to park its vehicle in a parking lot close to the road. Can disrupt traffic flow.</rdfs:comment>
        <rdfs:label xml:lang="en">Ego/non-ego-tp Parking In Near Lane</rdfs:label>
        <rdfs:label xml:lang="de">einparkendes Fahrzeug in Fahrstreifennähe</rdfs:label>
    </owl:Class>
    


    <!-- http://purl.org/auto/criticality_phenomena#CP_112 -->

    <owl:Class rdf:about="http://purl.org/auto/criticality_phenomena#CP_112">
        <rdfs:subClassOf rdf:resource="http://purl.org/auto/criticality_phenomena#CP_216"/>
        <rdfs:subClassOf rdf:resource="http://purl.org/auto/criticality_phenomena#Perfect_Perception_Criticality_Phenomenon"/>
        <dcterms:identifier rdf:datatype="http://www.w3.org/2001/XMLSchema#nonNegativeInteger">112</dcterms:identifier>
        <rdfs:comment xml:lang="en">A TP is performing a parking-out maneuver from a parking lot close to the road. Can disrupt traffic flow.</rdfs:comment>
        <rdfs:label xml:lang="en">Ego/non-ego-tp Parking Out Near Lane</rdfs:label>
        <rdfs:label xml:lang="de">ausparkendes Fahrzeug in Fahrstreifennähe</rdfs:label>
    </owl:Class>
    


    <!-- http://purl.org/auto/criticality_phenomena#CP_113 -->

    <owl:Class rdf:about="http://purl.org/auto/criticality_phenomena#CP_113">
        <rdfs:subClassOf rdf:resource="http://purl.org/auto/criticality_phenomena#Behavioral_Criticality_Phenomenon"/>
        <rdfs:subClassOf rdf:resource="http://purl.org/auto/criticality_phenomena#Criticality_Phenomenon"/>
        <rdfs:subClassOf rdf:resource="http://purl.org/auto/criticality_phenomena#Human_Criticality_Phenomenon"/>
        <rdfs:subClassOf rdf:resource="http://purl.org/auto/criticality_phenomena#Perfect_Perception_Criticality_Phenomenon"/>
        <rdfs:subClassOf rdf:resource="http://purl.org/auto/criticality_phenomena#Spatial_Criticality_Phenomenon"/>
        <rdfs:subClassOf rdf:resource="http://purl.org/auto/criticality_phenomena#Unpredictability_Criticality_Phenomenon"/>
        <dcterms:identifier rdf:datatype="http://www.w3.org/2001/XMLSchema#nonNegativeInteger">113</dcterms:identifier>
        <rdfs:comment xml:lang="en">A VRU is present in the scenario and has physical access to the road.</rdfs:comment>
        <rdfs:label xml:lang="en">Presence Of VRUs With Road Access</rdfs:label>
        <rdfs:label xml:lang="de">Präsenz von VRUs mit Fahrbahnzugang</rdfs:label>
    </owl:Class>
    


    <!-- http://purl.org/auto/criticality_phenomena#CP_114 -->

    <owl:Class rdf:about="http://purl.org/auto/criticality_phenomena#CP_114">
        <rdfs:subClassOf rdf:resource="http://purl.org/auto/criticality_phenomena#CP_113"/>
        <dcterms:identifier rdf:datatype="http://www.w3.org/2001/XMLSchema#nonNegativeInteger">114</dcterms:identifier>
        <rdfs:comment xml:lang="en">This refers to vulnerable road users whose ability to participate in traffic efficiently is impaired,
e.g. old/handicapped/blind pedestrians, wheel chairs</rdfs:comment>
        <rdfs:label xml:lang="de">Beeinträchtigte VRU mit Fahrbahnzugang</rdfs:label>
        <rdfs:label xml:lang="en">Impaired VRU With Road Access</rdfs:label>
    </owl:Class>
    


    <!-- http://purl.org/auto/criticality_phenomena#CP_115 -->

    <owl:Class rdf:about="http://purl.org/auto/criticality_phenomena#CP_115">
        <rdfs:subClassOf rdf:resource="http://purl.org/auto/criticality_phenomena#CP_275"/>
        <rdfs:subClassOf rdf:resource="http://purl.org/auto/criticality_phenomena#Perfect_Perception_Criticality_Phenomenon"/>
        <dcterms:identifier rdf:datatype="http://www.w3.org/2001/XMLSchema#nonNegativeInteger">115</dcterms:identifier>
        <rdfs:comment xml:lang="en">Some TP has a vehicle part which is deviating in its structural integrity. Examples include degraded tire profile, brakes, steering or lighting. Criticality depends on degree of degradation and vehicle part. </rdfs:comment>
        <rdfs:label xml:lang="en">Degraded Vehicle Parts</rdfs:label>
        <rdfs:label xml:lang="de">degradiert Fahrzeugteile</rdfs:label>
    </owl:Class>
    


    <!-- http://purl.org/auto/criticality_phenomena#CP_116 -->

    <owl:Class rdf:about="http://purl.org/auto/criticality_phenomena#CP_116">
        <rdfs:subClassOf rdf:resource="http://purl.org/auto/criticality_phenomena#CP_275"/>
        <rdfs:subClassOf rdf:resource="http://purl.org/auto/criticality_phenomena#Perfect_Perception_Criticality_Phenomenon"/>
        <dcterms:identifier rdf:datatype="http://www.w3.org/2001/XMLSchema#nonNegativeInteger">116</dcterms:identifier>
        <rdfs:comment xml:lang="en">Some TP has a vehicle part which is not able to perform its intended function. 
Examples include bursted tires, brakes, steering, wheels, engine, lighting, towing device, ... Criticality depends on defective vehicle part. </rdfs:comment>
        <rdfs:label xml:lang="en">Defective Vehicle Parts</rdfs:label>
        <rdfs:label xml:lang="de">Defekte Fahrzeugteile</rdfs:label>
    </owl:Class>
    


    <!-- http://purl.org/auto/criticality_phenomena#CP_117 -->

    <owl:Class rdf:about="http://purl.org/auto/criticality_phenomena#CP_117">
        <rdfs:subClassOf rdf:resource="http://purl.org/auto/criticality_phenomena#CP_255"/>
        <rdfs:subClassOf rdf:resource="http://purl.org/auto/criticality_phenomena#Dynamical_Criticality_Phenomenon"/>
        <rdfs:subClassOf rdf:resource="http://purl.org/auto/criticality_phenomena#Perfect_Perception_Criticality_Phenomenon"/>
        <rdfs:subClassOf rdf:resource="http://purl.org/auto/criticality_phenomena#Unpredictability_Criticality_Phenomenon"/>
        <dcterms:identifier rdf:datatype="http://www.w3.org/2001/XMLSchema#nonNegativeInteger">117</dcterms:identifier>
        <rdfs:comment xml:lang="en">Emergency vehicles how behavior like sirens which must be responded to.</rdfs:comment>
        <rdfs:label xml:lang="en">Behavior of Emergency Vehicles</rdfs:label>
        <rdfs:label xml:lang="de">Verhalten von Einsatzfahrzeugen</rdfs:label>
    </owl:Class>
    


    <!-- http://purl.org/auto/criticality_phenomena#CP_118 -->

    <owl:Class rdf:about="http://purl.org/auto/criticality_phenomena#CP_118">
        <rdfs:subClassOf rdf:resource="http://purl.org/auto/criticality_phenomena#CP_255"/>
        <rdfs:subClassOf rdf:resource="http://purl.org/auto/criticality_phenomena#Dynamical_Criticality_Phenomenon"/>
        <rdfs:subClassOf rdf:resource="http://purl.org/auto/criticality_phenomena#Perfect_Perception_Criticality_Phenomenon"/>
        <dcterms:identifier rdf:datatype="http://www.w3.org/2001/XMLSchema#nonNegativeInteger">118</dcterms:identifier>
        <rdfs:comment xml:lang="en">Service vehicles show special behaviour which must be responded to.</rdfs:comment>
        <rdfs:label xml:lang="en">Behaviour of service vehicles</rdfs:label>
        <rdfs:label xml:lang="de">Verhalten von Service Fahrzeugen</rdfs:label>
    </owl:Class>
    


    <!-- http://purl.org/auto/criticality_phenomena#CP_12 -->

    <owl:Class rdf:about="http://purl.org/auto/criticality_phenomena#CP_12">
        <rdfs:subClassOf rdf:resource="http://purl.org/auto/criticality_phenomena#CP_274"/>
        <rdfs:subClassOf rdf:resource="http://purl.org/auto/criticality_phenomena#Dynamical_Criticality_Phenomenon"/>
        <rdfs:subClassOf rdf:resource="http://purl.org/auto/criticality_phenomena#Real_Camera_Criticality_Phenomenon"/>
        <rdfs:subClassOf rdf:resource="http://purl.org/auto/criticality_phenomena#Real_Human_Criticality_Phenomenon"/>
        <rdfs:subClassOf rdf:resource="http://purl.org/auto/criticality_phenomena#Real_Lidar_Criticality_Phenomenon"/>
        <rdfs:subClassOf rdf:resource="http://purl.org/auto/criticality_phenomena#Real_Perception_Algorithm_Criticality_Phenomenon"/>
        <rdfs:subClassOf rdf:resource="http://purl.org/auto/criticality_phenomena#Real_Radar_Criticality_Phenomenon"/>
        <dcterms:identifier rdf:datatype="http://www.w3.org/2001/XMLSchema#nonNegativeInteger">12</dcterms:identifier>
        <rdfs:comment xml:lang="en">The road conditions on the surface, such as wet, (black) ice, snowy, aquaplaning, ...</rdfs:comment>
        <rdfs:label xml:lang="en">Deposited Precipitation</rdfs:label>
        <rdfs:label xml:lang="de">Flüssigkeitsablagerung auf der Straße</rdfs:label>
    </owl:Class>
    


    <!-- http://purl.org/auto/criticality_phenomena#CP_13 -->

    <owl:Class rdf:about="http://purl.org/auto/criticality_phenomena#CP_13">
        <rdfs:subClassOf rdf:resource="http://purl.org/auto/criticality_phenomena#CP_189"/>
        <rdfs:subClassOf rdf:resource="http://purl.org/auto/criticality_phenomena#CP_274"/>
        <rdfs:subClassOf rdf:resource="http://purl.org/auto/criticality_phenomena#Real_Lidar_Criticality_Phenomenon"/>
        <dcterms:identifier rdf:datatype="http://www.w3.org/2001/XMLSchema#nonNegativeInteger">13</dcterms:identifier>
        <rdfs:comment xml:lang="en">Fog is a visible aerosol consisting of tiny water droplets or ice crystals suspended in the air at or near the Earth&apos;s surface. Fog shows up when water vapor (water in its gaseous form) condenses. Fog can be considered a type of low-lying cloud usually resembling stratus, and is heavily influenced by nearby bodies of water, topography, and wind conditions.</rdfs:comment>
        <rdfs:label xml:lang="en">Fog</rdfs:label>
        <rdfs:label xml:lang="de">Nebel</rdfs:label>
    </owl:Class>
    


    <!-- http://purl.org/auto/criticality_phenomena#CP_138 -->

    <owl:Class rdf:about="http://purl.org/auto/criticality_phenomena#CP_138">
        <rdfs:subClassOf rdf:resource="http://purl.org/auto/criticality_phenomena#CP_142"/>
        <rdfs:subClassOf rdf:resource="http://purl.org/auto/criticality_phenomena#Human_Criticality_Phenomenon"/>
        <dcterms:identifier rdf:datatype="http://www.w3.org/2001/XMLSchema#nonNegativeInteger">138</dcterms:identifier>
        <rdfs:comment xml:lang="en">A distraction is an influencing factor deflecting the attention of the TP such that the TP is not able to conduct the driving task in a safely manner. This includes physical distractions (e.g. visual distraction by smarthpone or accident site) and cognitive distractions such as psychological stress or other emotions.</rdfs:comment>
        <rdfs:label xml:lang="en">Non-Ego-TP Distracted From Driving Task</rdfs:label>
        <rdfs:label xml:lang="de">Non-Ego-TP von Fahraufgabe abgelenkt</rdfs:label>
    </owl:Class>
    


    <!-- http://purl.org/auto/criticality_phenomena#CP_139 -->

    <owl:Class rdf:about="http://purl.org/auto/criticality_phenomena#CP_139">
        <rdfs:subClassOf rdf:resource="http://purl.org/auto/criticality_phenomena#CP_142"/>
        <dcterms:identifier rdf:datatype="http://www.w3.org/2001/XMLSchema#nonNegativeInteger">139</dcterms:identifier>
        <rdfs:comment xml:lang="en">An impairment is a state of the TP that leads to a reduced ability to safely navigate in traffic. Impairment may be temporarily, e.g. due to alcohol, drugs, medication, distraction or permanent to old age or handicap.</rdfs:comment>
        <rdfs:label xml:lang="de">Non-Ego-TP Beeinträchtigte Fahrfähigkeit</rdfs:label>
        <rdfs:label xml:lang="en">Non-Ego-TP Impaired Driving Ability</rdfs:label>
    </owl:Class>
    


    <!-- http://purl.org/auto/criticality_phenomena#CP_14 -->

    <owl:Class rdf:about="http://purl.org/auto/criticality_phenomena#CP_14">
        <rdfs:subClassOf rdf:resource="http://purl.org/auto/criticality_phenomena#CP_285"/>
        <rdfs:subClassOf rdf:resource="http://purl.org/auto/criticality_phenomena#Environmental_Criticality_Phenomenon"/>
        <rdfs:subClassOf rdf:resource="http://purl.org/auto/criticality_phenomena#Perfect_Perception_Criticality_Phenomenon"/>
        <dcterms:identifier rdf:datatype="http://www.w3.org/2001/XMLSchema#nonNegativeInteger">14</dcterms:identifier>
        <rdfs:comment xml:lang="en">The intensity and direction of the wind. </rdfs:comment>
        <rdfs:label xml:lang="de">Wind</rdfs:label>
        <rdfs:label xml:lang="en">Wind</rdfs:label>
    </owl:Class>
    


    <!-- http://purl.org/auto/criticality_phenomena#CP_140 -->

    <owl:Class rdf:about="http://purl.org/auto/criticality_phenomena#CP_140">
        <rdfs:subClassOf rdf:resource="http://purl.org/auto/criticality_phenomena#CP_141"/>
        <rdfs:subClassOf rdf:resource="http://purl.org/auto/criticality_phenomena#Dynamical_Criticality_Phenomenon"/>
        <dcterms:identifier rdf:datatype="http://www.w3.org/2001/XMLSchema#nonNegativeInteger">140</dcterms:identifier>
        <rdfs:comment xml:lang="en">Aggressive driving behavior is commonly defined as &quot;any behavior intended to physically, emotionally, or psychologically harm another within the driving environment.&quot;, e.g. for seeking excitement.</rdfs:comment>
        <rdfs:label xml:lang="en">Non-Ego-TP Aggressive Driving</rdfs:label>
        <rdfs:label xml:lang="de">Non-Ego-TP Aggressives Fahren</rdfs:label>
    </owl:Class>
    


    <!-- http://purl.org/auto/criticality_phenomena#CP_141 -->

    <owl:Class rdf:about="http://purl.org/auto/criticality_phenomena#CP_141">
        <rdfs:subClassOf rdf:resource="http://purl.org/auto/criticality_phenomena#CP_142"/>
        <rdfs:subClassOf rdf:resource="http://purl.org/auto/criticality_phenomena#Human_Criticality_Phenomenon"/>
        <dcterms:identifier rdf:datatype="http://www.w3.org/2001/XMLSchema#nonNegativeInteger">141</dcterms:identifier>
        <rdfs:comment xml:lang="en">Driving while experiencing egative emotions that affect the driving behavior of the TP, e.g. anger, fear, sadness, ...</rdfs:comment>
        <rdfs:label xml:lang="en">Non-Ego-TP Emotional Driving</rdfs:label>
        <rdfs:label xml:lang="de">Non-Ego-TP Emotionales Fahren</rdfs:label>
    </owl:Class>
    


    <!-- http://purl.org/auto/criticality_phenomena#CP_142 -->

    <owl:Class rdf:about="http://purl.org/auto/criticality_phenomena#CP_142">
        <rdfs:subClassOf rdf:resource="http://purl.org/auto/criticality_phenomena#CP_283"/>
        <rdfs:subClassOf rdf:resource="http://purl.org/auto/criticality_phenomena#Dynamical_Criticality_Phenomenon"/>
        <rdfs:subClassOf rdf:resource="http://purl.org/auto/criticality_phenomena#Perfect_Perception_Criticality_Phenomenon"/>
        <dcterms:identifier rdf:datatype="http://www.w3.org/2001/XMLSchema#nonNegativeInteger">142</dcterms:identifier>
        <rdfs:comment xml:lang="en">Behavior not according to expected norm behavior, e.g. a sudden left turn without indication or reduction in speed.</rdfs:comment>
        <rdfs:label xml:lang="de">Non-Ego-TP Unerwartetes Fahrverhalten</rdfs:label>
        <rdfs:label xml:lang="en">Non-Ego-TP Unexpected Driving</rdfs:label>
    </owl:Class>
    


    <!-- http://purl.org/auto/criticality_phenomena#CP_143 -->

    <owl:Class rdf:about="http://purl.org/auto/criticality_phenomena#CP_143">
        <rdfs:subClassOf rdf:resource="http://purl.org/auto/criticality_phenomena#CP_283"/>
        <rdfs:subClassOf rdf:resource="http://purl.org/auto/criticality_phenomena#Perfect_Perception_Criticality_Phenomenon"/>
        <dcterms:identifier rdf:datatype="http://www.w3.org/2001/XMLSchema#nonNegativeInteger">143</dcterms:identifier>
        <rdfs:comment xml:lang="en">Intentional or unintentional breaking of the traffic rules or norm behavior.</rdfs:comment>
        <rdfs:label xml:lang="de">Fehlverhalten</rdfs:label>
        <rdfs:label xml:lang="en">Misconduct</rdfs:label>
    </owl:Class>
    


    <!-- http://purl.org/auto/criticality_phenomena#CP_144 -->

    <owl:Class rdf:about="http://purl.org/auto/criticality_phenomena#CP_144">
        <rdfs:subClassOf rdf:resource="http://purl.org/auto/criticality_phenomena#CP_146"/>
        <rdfs:subClassOf rdf:resource="http://purl.org/auto/criticality_phenomena#Dynamical_Criticality_Phenomenon"/>
        <dcterms:identifier rdf:datatype="http://www.w3.org/2001/XMLSchema#nonNegativeInteger">144</dcterms:identifier>
        <rdfs:comment xml:lang="en">Failing to signalize the direction of driving in accordance to the traffic rules.</rdfs:comment>
        <rdfs:label xml:lang="en">Missing Indicator Signal Of Non-Ego-TP</rdfs:label>
        <rdfs:label xml:lang="de">Non-Ego-TP Fehlende Nutzung Fahrtrichtungsanzeiger</rdfs:label>
    </owl:Class>
    


    <!-- http://purl.org/auto/criticality_phenomena#CP_145 -->

    <owl:Class rdf:about="http://purl.org/auto/criticality_phenomena#CP_145">
        <rdfs:subClassOf rdf:resource="http://purl.org/auto/criticality_phenomena#CP_143"/>
        <rdfs:subClassOf rdf:resource="http://purl.org/auto/criticality_phenomena#Dynamical_Criticality_Phenomenon"/>
        <rdfs:subClassOf rdf:resource="http://purl.org/auto/criticality_phenomena#Human_Criticality_Phenomenon"/>
        <dcterms:identifier rdf:datatype="http://www.w3.org/2001/XMLSchema#nonNegativeInteger">145</dcterms:identifier>
        <rdfs:comment xml:lang="en">Missing indicator signal for the driving direction of a bicyclist.</rdfs:comment>
        <rdfs:label xml:lang="de">Fehlendes Blinken</rdfs:label>
        <rdfs:label xml:lang="en">Missing Indicator Signal Of Bicyclist</rdfs:label>
    </owl:Class>
    


    <!-- http://purl.org/auto/criticality_phenomena#CP_146 -->

    <owl:Class rdf:about="http://purl.org/auto/criticality_phenomena#CP_146">
        <rdfs:subClassOf rdf:resource="http://purl.org/auto/criticality_phenomena#CP_143"/>
        <dcterms:identifier rdf:datatype="http://www.w3.org/2001/XMLSchema#nonNegativeInteger">146</dcterms:identifier>
        <rdfs:comment xml:lang="en">Any missing signal of other TPs that could be of importance to the ego&apos;s situation interpretation. They can be either voluntary signals (e.g. hazard lights at traffic jam tail) or mandatory signals (e.g. indicator signal when making a turn).</rdfs:comment>
        <rdfs:label xml:lang="en">Missing Signal Of Non-Ego-TP</rdfs:label>
        <rdfs:label xml:lang="de">Non-Ego-TP Fehlendes Signal (nicht Fahrtrichtungsanzeige)</rdfs:label>
    </owl:Class>
    


    <!-- http://purl.org/auto/criticality_phenomena#CP_147 -->

    <owl:Class rdf:about="http://purl.org/auto/criticality_phenomena#CP_147">
        <rdfs:subClassOf rdf:resource="http://purl.org/auto/criticality_phenomena#CP_143"/>
        <dcterms:identifier rdf:datatype="http://www.w3.org/2001/XMLSchema#nonNegativeInteger">147</dcterms:identifier>
        <rdfs:comment xml:lang="en">The given signal of a traffic participant deviates from its intended message or the actual behavior.</rdfs:comment>
        <rdfs:label xml:lang="en">Errorneous Signal Of Non-Ego-TP</rdfs:label>
        <rdfs:label xml:lang="de">Non-Ego-TP Fehlerhaftes Signal</rdfs:label>
    </owl:Class>
    


    <!-- http://purl.org/auto/criticality_phenomena#CP_148 -->

    <owl:Class rdf:about="http://purl.org/auto/criticality_phenomena#CP_148">
        <rdfs:subClassOf rdf:resource="http://purl.org/auto/criticality_phenomena#Behavioral_Criticality_Phenomenon"/>
        <rdfs:subClassOf rdf:resource="http://purl.org/auto/criticality_phenomena#CP_29"/>
        <dcterms:identifier rdf:datatype="http://www.w3.org/2001/XMLSchema#nonNegativeInteger">148</dcterms:identifier>
        <rdfs:comment xml:lang="en">As defined by traffic rules, i.e. a TP who could drive faster, but is driving so slow that it hinders the traffic flow.</rdfs:comment>
        <rdfs:label xml:lang="en">Unnecessary Slow Driving Of TP</rdfs:label>
        <rdfs:label xml:lang="de">Unnötiges Langsamfahren</rdfs:label>
    </owl:Class>
    


    <!-- http://purl.org/auto/criticality_phenomena#CP_149 -->

    <owl:Class rdf:about="http://purl.org/auto/criticality_phenomena#CP_149">
        <rdfs:subClassOf rdf:resource="http://purl.org/auto/criticality_phenomena#Behavioral_Criticality_Phenomenon"/>
        <rdfs:subClassOf rdf:resource="http://purl.org/auto/criticality_phenomena#CP_39"/>
        <rdfs:subClassOf rdf:resource="http://purl.org/auto/criticality_phenomena#Real_Camera_Criticality_Phenomenon"/>
        <rdfs:subClassOf rdf:resource="http://purl.org/auto/criticality_phenomena#Unpredictability_Criticality_Phenomenon"/>
        <dcterms:identifier rdf:datatype="http://www.w3.org/2001/XMLSchema#nonNegativeInteger">149</dcterms:identifier>
        <rdfs:comment xml:lang="en">TP has wrongly interpreted a light signal, e.g. flashlight</rdfs:comment>
        <rdfs:label xml:lang="en">(mis/missing)-interpretation Of Light Signal</rdfs:label>
        <rdfs:label xml:lang="de">Fehlinterpretation eines Lichtsignals</rdfs:label>
    </owl:Class>
    


    <!-- http://purl.org/auto/criticality_phenomena#CP_15 -->

    <owl:Class rdf:about="http://purl.org/auto/criticality_phenomena#CP_15">
        <rdfs:subClassOf rdf:resource="http://purl.org/auto/criticality_phenomena#CP_274"/>
        <rdfs:subClassOf rdf:resource="http://purl.org/auto/criticality_phenomena#Dynamical_Criticality_Phenomenon"/>
        <rdfs:subClassOf rdf:resource="http://purl.org/auto/criticality_phenomena#Real_Camera_Criticality_Phenomenon"/>
        <rdfs:subClassOf rdf:resource="http://purl.org/auto/criticality_phenomena#Real_Human_Criticality_Phenomenon"/>
        <rdfs:subClassOf rdf:resource="http://purl.org/auto/criticality_phenomena#Real_Lidar_Criticality_Phenomenon"/>
        <rdfs:subClassOf rdf:resource="http://purl.org/auto/criticality_phenomena#Real_Perception_Algorithm_Criticality_Phenomenon"/>
        <rdfs:subClassOf rdf:resource="http://purl.org/auto/criticality_phenomena#Real_Radar_Criticality_Phenomenon"/>
        <dcterms:identifier rdf:datatype="http://www.w3.org/2001/XMLSchema#nonNegativeInteger">15</dcterms:identifier>
        <rdfs:comment xml:lang="en">The presence and intensity of snowfall or snow on the road.</rdfs:comment>
        <rdfs:label xml:lang="de">Schnee</rdfs:label>
        <rdfs:label xml:lang="en">Snow</rdfs:label>
    </owl:Class>
    


    <!-- http://purl.org/auto/criticality_phenomena#CP_150 -->

    <owl:Class rdf:about="http://purl.org/auto/criticality_phenomena#CP_150">
        <rdfs:subClassOf rdf:resource="http://purl.org/auto/criticality_phenomena#Criticality_Phenomenon"/>
        <rdfs:subClassOf rdf:resource="http://purl.org/auto/criticality_phenomena#Perfect_Perception_Criticality_Phenomenon"/>
        <rdfs:subClassOf rdf:resource="http://purl.org/auto/criticality_phenomena#Spatial_Criticality_Phenomenon"/>
        <dcterms:identifier rdf:datatype="http://www.w3.org/2001/XMLSchema#nonNegativeInteger">150</dcterms:identifier>
        <rdfs:comment xml:lang="en">A TP has a small distance to some object. We define small distance as being lower than the safe distance defined by RSS.</rdfs:comment>
        <rdfs:label xml:lang="en">Small Distance</rdfs:label>
        <rdfs:label xml:lang="de">geringer Abstand</rdfs:label>
    </owl:Class>
    


    <!-- http://purl.org/auto/criticality_phenomena#CP_151 -->

    <owl:Class rdf:about="http://purl.org/auto/criticality_phenomena#CP_151">
        <rdfs:subClassOf rdf:resource="http://purl.org/auto/criticality_phenomena#CP_36"/>
        <dcterms:identifier rdf:datatype="http://www.w3.org/2001/XMLSchema#nonNegativeInteger">151</dcterms:identifier>
        <rdfs:comment xml:lang="en">Unsafe longitudinal distance to the front, as defined by RSS</rdfs:comment>
        <rdfs:label xml:lang="en">Small Distance To Front</rdfs:label>
        <rdfs:label xml:lang="de">geringer Abstand zum vorderen Verkehrsteilnehmer</rdfs:label>
    </owl:Class>
    


    <!-- http://purl.org/auto/criticality_phenomena#CP_152 -->

    <owl:Class rdf:about="http://purl.org/auto/criticality_phenomena#CP_152">
        <rdfs:subClassOf rdf:resource="http://purl.org/auto/criticality_phenomena#CP_36"/>
        <dcterms:identifier rdf:datatype="http://www.w3.org/2001/XMLSchema#nonNegativeInteger">152</dcterms:identifier>
        <rdfs:comment xml:lang="en">Unsafe longitudinal distance to the back, as defined by RSS, e.g. caused by following TP</rdfs:comment>
        <rdfs:label xml:lang="en">Small Distance To Back</rdfs:label>
        <rdfs:label xml:lang="de">geringer Abstand zu hinteren Verkehrsteilnehmer</rdfs:label>
    </owl:Class>
    


    <!-- http://purl.org/auto/criticality_phenomena#CP_153 -->

    <owl:Class rdf:about="http://purl.org/auto/criticality_phenomena#CP_153">
        <rdfs:subClassOf rdf:resource="http://purl.org/auto/criticality_phenomena#CP_36"/>
        <dcterms:identifier rdf:datatype="http://www.w3.org/2001/XMLSchema#nonNegativeInteger">153</dcterms:identifier>
        <rdfs:comment xml:lang="en">Unsafe lateral distance as defined by RSS, e.g. to temporal lanes for construction sites</rdfs:comment>
        <rdfs:label xml:lang="en">Small Lateral Distance</rdfs:label>
        <rdfs:label xml:lang="de">geringer Seitenabstand zu anderem Verkehrsteilnehmer</rdfs:label>
    </owl:Class>
    


    <!-- http://purl.org/auto/criticality_phenomena#CP_154 -->

    <owl:Class rdf:about="http://purl.org/auto/criticality_phenomena#CP_154">
        <rdfs:subClassOf rdf:resource="http://purl.org/auto/criticality_phenomena#CP_284"/>
        <rdfs:subClassOf rdf:resource="http://purl.org/auto/criticality_phenomena#CP_293"/>
        <dcterms:identifier rdf:datatype="http://www.w3.org/2001/XMLSchema#nonNegativeInteger">154</dcterms:identifier>
        <rdfs:comment xml:lang="en"> The intended trajectories of at least two TPs intersect. Without direct action of the involved TPs, this would lead to a crash.</rdfs:comment>
        <rdfs:label xml:lang="en">Intersecting Planned Trajectories Of TPs</rdfs:label>
        <rdfs:label xml:lang="de">kreuzende geplante Fahrtrajektorien der Verkehrsteilnehmer</rdfs:label>
    </owl:Class>
    


    <!-- http://purl.org/auto/criticality_phenomena#CP_155 -->

    <owl:Class rdf:about="http://purl.org/auto/criticality_phenomena#CP_155">
        <rdfs:subClassOf rdf:resource="http://purl.org/auto/criticality_phenomena#CP_265"/>
        <rdfs:subClassOf rdf:resource="http://purl.org/auto/criticality_phenomena#Perfect_Camera_Criticality_Phenomenon"/>
        <rdfs:subClassOf rdf:resource="http://purl.org/auto/criticality_phenomena#Perfect_Human_Criticality_Phenomenon"/>
        <rdfs:subClassOf rdf:resource="http://purl.org/auto/criticality_phenomena#Perfect_Lidar_Criticality_Phenomenon"/>
        <rdfs:subClassOf rdf:resource="http://purl.org/auto/criticality_phenomena#Perfect_Radar_Criticality_Phenomenon"/>
        <dcterms:identifier rdf:datatype="http://www.w3.org/2001/XMLSchema#nonNegativeInteger">155</dcterms:identifier>
        <rdfs:comment xml:lang="en">The occluded entity is a (part of a) lane marking.</rdfs:comment>
        <rdfs:label xml:lang="en">Occluded Lane Markings</rdfs:label>
        <rdfs:label xml:lang="de">verdeckte Fahrstreifenmarkierungen</rdfs:label>
    </owl:Class>
    


    <!-- http://purl.org/auto/criticality_phenomena#CP_156 -->

    <owl:Class rdf:about="http://purl.org/auto/criticality_phenomena#CP_156">
        <rdfs:subClassOf rdf:resource="http://purl.org/auto/criticality_phenomena#CP_265"/>
        <rdfs:subClassOf rdf:resource="http://purl.org/auto/criticality_phenomena#Perfect_Camera_Criticality_Phenomenon"/>
        <rdfs:subClassOf rdf:resource="http://purl.org/auto/criticality_phenomena#Perfect_Human_Criticality_Phenomenon"/>
        <rdfs:subClassOf rdf:resource="http://purl.org/auto/criticality_phenomena#Perfect_Lidar_Criticality_Phenomenon"/>
        <rdfs:subClassOf rdf:resource="http://purl.org/auto/criticality_phenomena#Perfect_Radar_Criticality_Phenomenon"/>
        <dcterms:identifier rdf:datatype="http://www.w3.org/2001/XMLSchema#nonNegativeInteger">156</dcterms:identifier>
        <rdfs:comment xml:lang="en">The occluded entity is a (part of a) traffic sign. The criticality depends on traffic sign</rdfs:comment>
        <rdfs:label xml:lang="en">Occluded Traffic Sign</rdfs:label>
        <rdfs:label xml:lang="de">verdeckte Straßenschilder</rdfs:label>
    </owl:Class>
    


    <!-- http://purl.org/auto/criticality_phenomena#CP_157 -->

    <owl:Class rdf:about="http://purl.org/auto/criticality_phenomena#CP_157">
        <rdfs:subClassOf rdf:resource="http://purl.org/auto/criticality_phenomena#CP_25"/>
        <rdfs:subClassOf rdf:resource="http://purl.org/auto/criticality_phenomena#Human_Criticality_Phenomenon"/>
        <rdfs:subClassOf rdf:resource="http://purl.org/auto/criticality_phenomena#Unpredictability_Criticality_Phenomenon"/>
        <formalized rdf:datatype="http://www.w3.org/2001/XMLSchema#boolean">true</formalized>
        <dcterms:identifier rdf:datatype="http://www.w3.org/2001/XMLSchema#nonNegativeInteger">157</dcterms:identifier>
        <rdfs:comment xml:lang="en">The occluded entity is a pedestrian.</rdfs:comment>
        <rdfs:label xml:lang="en">Occluded Pedestrian</rdfs:label>
        <rdfs:label xml:lang="de">verdeckter Fußgänger</rdfs:label>
    </owl:Class>
    


    <!-- http://purl.org/auto/criticality_phenomena#CP_158 -->

    <owl:Class rdf:about="http://purl.org/auto/criticality_phenomena#CP_158">
        <rdfs:subClassOf rdf:resource="http://purl.org/auto/criticality_phenomena#CP_28"/>
        <rdfs:subClassOf rdf:resource="http://purl.org/auto/criticality_phenomena#Dynamical_Criticality_Phenomenon"/>
        <formalized rdf:datatype="http://www.w3.org/2001/XMLSchema#boolean">true</formalized>
        <dcterms:identifier rdf:datatype="http://www.w3.org/2001/XMLSchema#nonNegativeInteger">158</dcterms:identifier>
        <rdfs:comment xml:lang="en">The occluded entity is a vehicle whose planned trajectory intersects the currently planned trajectory of the ego.</rdfs:comment>
        <rdfs:label xml:lang="en">Occluded Intersecting Vehicle</rdfs:label>
        <rdfs:label xml:lang="de">verdecktes kreuzendes Fahrzeug</rdfs:label>
    </owl:Class>
    


    <!-- http://purl.org/auto/criticality_phenomena#CP_159 -->

    <owl:Class rdf:about="http://purl.org/auto/criticality_phenomena#CP_159">
        <rdfs:subClassOf rdf:resource="http://purl.org/auto/criticality_phenomena#CP_25"/>
        <dcterms:identifier rdf:datatype="http://www.w3.org/2001/XMLSchema#nonNegativeInteger">159</dcterms:identifier>
        <rdfs:comment xml:lang="en">Refers to objects for potential collisiohns,  e.g. parking vehicles</rdfs:comment>
        <rdfs:label xml:lang="en">Occluded Obstacle</rdfs:label>
        <rdfs:label xml:lang="de">verdecktes Hindernis</rdfs:label>
    </owl:Class>
    


    <!-- http://purl.org/auto/criticality_phenomena#CP_16 -->

    <owl:Class rdf:about="http://purl.org/auto/criticality_phenomena#CP_16">
        <rdfs:subClassOf rdf:resource="http://purl.org/auto/criticality_phenomena#CP_274"/>
        <rdfs:subClassOf rdf:resource="http://purl.org/auto/criticality_phenomena#Real_Camera_Criticality_Phenomenon"/>
        <rdfs:subClassOf rdf:resource="http://purl.org/auto/criticality_phenomena#Real_Human_Criticality_Phenomenon"/>
        <rdfs:subClassOf rdf:resource="http://purl.org/auto/criticality_phenomena#Real_Lidar_Criticality_Phenomenon"/>
        <rdfs:subClassOf rdf:resource="http://purl.org/auto/criticality_phenomena#Real_Perception_Algorithm_Criticality_Phenomenon"/>
        <rdfs:subClassOf rdf:resource="http://purl.org/auto/criticality_phenomena#Real_Radar_Criticality_Phenomenon"/>
        <dcterms:identifier rdf:datatype="http://www.w3.org/2001/XMLSchema#nonNegativeInteger">16</dcterms:identifier>
        <rdfs:comment xml:lang="en">The presence and intensity of hail.</rdfs:comment>
        <rdfs:label xml:lang="de">Hagel</rdfs:label>
        <rdfs:label xml:lang="en">Hail</rdfs:label>
    </owl:Class>
    


    <!-- http://purl.org/auto/criticality_phenomena#CP_160 -->

    <owl:Class rdf:about="http://purl.org/auto/criticality_phenomena#CP_160">
        <rdfs:subClassOf rdf:resource="http://purl.org/auto/criticality_phenomena#CP_25"/>
        <rdfs:subClassOf rdf:resource="http://purl.org/auto/criticality_phenomena#Human_Criticality_Phenomenon"/>
        <formalized rdf:datatype="http://www.w3.org/2001/XMLSchema#boolean">true</formalized>
        <dcterms:identifier rdf:datatype="http://www.w3.org/2001/XMLSchema#nonNegativeInteger">160</dcterms:identifier>
        <rdfs:comment xml:lang="en">The occluded entity is a bicyclist.</rdfs:comment>
        <rdfs:label xml:lang="en">Occluded Bicyclist</rdfs:label>
        <rdfs:label xml:lang="de">verdeckter Fahrradfahrer</rdfs:label>
    </owl:Class>
    


    <!-- http://purl.org/auto/criticality_phenomena#CP_161 -->

    <owl:Class rdf:about="http://purl.org/auto/criticality_phenomena#CP_161">
        <rdfs:subClassOf rdf:resource="http://purl.org/auto/criticality_phenomena#Behavioral_Criticality_Phenomenon"/>
        <rdfs:subClassOf rdf:resource="http://purl.org/auto/criticality_phenomena#CP_29"/>
        <dcterms:identifier rdf:datatype="http://www.w3.org/2001/XMLSchema#nonNegativeInteger">161</dcterms:identifier>
        <rdfs:comment xml:lang="en">TP has a speed which does is excessively higher than the normally expected speed.</rdfs:comment>
        <rdfs:label xml:lang="en">Excessive Speed Of Non-Ego-TP</rdfs:label>
        <rdfs:label xml:lang="de">Non-Ego-TP hat überhöhte Geschwindigkeit</rdfs:label>
    </owl:Class>
    


    <!-- http://purl.org/auto/criticality_phenomena#CP_162 -->

    <owl:Class rdf:about="http://purl.org/auto/criticality_phenomena#CP_162">
        <rdfs:subClassOf rdf:resource="http://purl.org/auto/criticality_phenomena#CP_286"/>
        <dcterms:identifier rdf:datatype="http://www.w3.org/2001/XMLSchema#nonNegativeInteger">162</dcterms:identifier>
        <rdfs:comment xml:lang="en">Refers to a road section which is not a straight road without any properties.</rdfs:comment>
        <rdfs:label xml:lang="en">Special road section</rdfs:label>
        <rdfs:label xml:lang="de">Spezieller Straßenabschnitt</rdfs:label>
    </owl:Class>
    


    <!-- http://purl.org/auto/criticality_phenomena#CP_163 -->

    <owl:Class rdf:about="http://purl.org/auto/criticality_phenomena#CP_163">
        <rdfs:subClassOf rdf:resource="http://purl.org/auto/criticality_phenomena#CP_29"/>
        <dcterms:identifier rdf:datatype="http://www.w3.org/2001/XMLSchema#nonNegativeInteger">163</dcterms:identifier>
        <rdfs:comment xml:lang="en">Two traffic participants in the scenario have a difference in speed which is unexpectedly high, e.g. TP in motion vs. TP at rest/slower TP</rdfs:comment>
        <rdfs:label xml:lang="en">High Relative Speed</rdfs:label>
        <rdfs:label xml:lang="de">hohe Relativgeschwindigkeit</rdfs:label>
    </owl:Class>
    


    <!-- http://purl.org/auto/criticality_phenomena#CP_164 -->

    <owl:Class rdf:about="http://purl.org/auto/criticality_phenomena#CP_164">
        <rdfs:subClassOf rdf:resource="http://purl.org/auto/criticality_phenomena#Criticality_Phenomenon"/>
        <rdfs:subClassOf rdf:resource="http://purl.org/auto/criticality_phenomena#Environmental_Criticality_Phenomenon"/>
        <rdfs:subClassOf rdf:resource="http://purl.org/auto/criticality_phenomena#Perfect_Perception_Criticality_Phenomenon"/>
        <dcterms:identifier rdf:datatype="http://www.w3.org/2001/XMLSchema#nonNegativeInteger">164</dcterms:identifier>
        <rdfs:comment xml:lang="en">An external force is applied to a traffic participant. Criticality depends on intensity. Examples: Storm, Accident, Someone Pushing a Pedestrian, ...</rdfs:comment>
        <rdfs:label xml:lang="en">External Force</rdfs:label>
        <rdfs:label xml:lang="de">Externe äußere Kraft (z.B. Wind)</rdfs:label>
    </owl:Class>
    


    <!-- http://purl.org/auto/criticality_phenomena#CP_165 -->

    <owl:Class rdf:about="http://purl.org/auto/criticality_phenomena#CP_165">
        <rdfs:subClassOf rdf:resource="http://purl.org/auto/criticality_phenomena#Behavioral_Criticality_Phenomenon"/>
        <rdfs:subClassOf rdf:resource="http://purl.org/auto/criticality_phenomena#CP_287"/>
        <rdfs:subClassOf rdf:resource="http://purl.org/auto/criticality_phenomena#Perfect_Perception_Criticality_Phenomenon"/>
        <dcterms:identifier rdf:datatype="http://www.w3.org/2001/XMLSchema#nonNegativeInteger">165</dcterms:identifier>
        <rdfs:comment xml:lang="en">A situation in which the right of way can not be solved through the application of the traffic rules. Communication of the TPs will be necessary.</rdfs:comment>
        <rdfs:label xml:lang="de">Nicht-auflösbare Vorfahrtssituation</rdfs:label>
        <rdfs:label xml:lang="en">Right-of-way Dead-lock</rdfs:label>
    </owl:Class>
    


    <!-- http://purl.org/auto/criticality_phenomena#CP_166 -->

    <owl:Class rdf:about="http://purl.org/auto/criticality_phenomena#CP_166">
        <rdfs:subClassOf rdf:resource="http://purl.org/auto/criticality_phenomena#CP_196"/>
        <rdfs:subClassOf rdf:resource="http://purl.org/auto/criticality_phenomena#Real_Camera_Criticality_Phenomenon"/>
        <rdfs:subClassOf rdf:resource="http://purl.org/auto/criticality_phenomena#Real_Human_Criticality_Phenomenon"/>
        <dcterms:identifier rdf:datatype="http://www.w3.org/2001/XMLSchema#nonNegativeInteger">166</dcterms:identifier>
        <rdfs:comment xml:lang="en">A TP has ist headlight set too high or its flash light permanently on such that other TPs will be blinded by the resulting glare.</rdfs:comment>
        <rdfs:label xml:lang="en">Glare Due To Non-Ego-TP Full Headlight</rdfs:label>
        <rdfs:label xml:lang="de">Non-Ego-TP blendet durch Aufblendlicht Ego</rdfs:label>
    </owl:Class>
    


    <!-- http://purl.org/auto/criticality_phenomena#CP_167 -->

    <owl:Class rdf:about="http://purl.org/auto/criticality_phenomena#CP_167">
        <rdfs:subClassOf rdf:resource="http://purl.org/auto/criticality_phenomena#CP_142"/>
        <dcterms:identifier rdf:datatype="http://www.w3.org/2001/XMLSchema#nonNegativeInteger">167</dcterms:identifier>
        <rdfs:comment xml:lang="en">Legitimate or illegitimate crossing of a red signal.</rdfs:comment>
        <rdfs:label xml:lang="en">Non-Ego-TP Running A Red Traffic Light</rdfs:label>
        <rdfs:label xml:lang="de">Non-Ego-TP überfährt eine rote Ampel</rdfs:label>
    </owl:Class>
    


    <!-- http://purl.org/auto/criticality_phenomena#CP_168 -->

    <owl:Class rdf:about="http://purl.org/auto/criticality_phenomena#CP_168">
        <rdfs:subClassOf rdf:resource="http://purl.org/auto/criticality_phenomena#CP_142"/>
        <dcterms:identifier rdf:datatype="http://www.w3.org/2001/XMLSchema#nonNegativeInteger">168</dcterms:identifier>
        <rdfs:comment xml:lang="en">Any violation of a right of way rule (can be indicated through lights, signs, or not at all) as defined by the traffic rules.</rdfs:comment>
        <rdfs:label xml:lang="en">Non-Ego-TP Violating Right Of Way</rdfs:label>
        <rdfs:label xml:lang="de">Non-Ego-TP missachtet die Vorfahrt</rdfs:label>
    </owl:Class>
    


    <!-- http://purl.org/auto/criticality_phenomena#CP_169 -->

    <owl:Class rdf:about="http://purl.org/auto/criticality_phenomena#CP_169">
        <rdfs:subClassOf rdf:resource="http://purl.org/auto/criticality_phenomena#CP_142"/>
        <dcterms:identifier rdf:datatype="http://www.w3.org/2001/XMLSchema#nonNegativeInteger">169</dcterms:identifier>
        <rdfs:comment xml:lang="en">A TP merges directly behind another TP without first letting the waiting vehicle pass, or a traffic participant is not letting another TP merge onto its lane.</rdfs:comment>
        <rdfs:label xml:lang="de">Missachtung des Reißverschlussverfahrens</rdfs:label>
        <rdfs:label xml:lang="en">Violation Of Zip Merging</rdfs:label>
    </owl:Class>
    


    <!-- http://purl.org/auto/criticality_phenomena#CP_17 -->

    <owl:Class rdf:about="http://purl.org/auto/criticality_phenomena#CP_17">
        <rdfs:subClassOf rdf:resource="http://purl.org/auto/criticality_phenomena#CP_274"/>
        <rdfs:subClassOf rdf:resource="http://purl.org/auto/criticality_phenomena#Dynamical_Criticality_Phenomenon"/>
        <rdfs:subClassOf rdf:resource="http://purl.org/auto/criticality_phenomena#Real_Camera_Criticality_Phenomenon"/>
        <rdfs:subClassOf rdf:resource="http://purl.org/auto/criticality_phenomena#Real_Human_Criticality_Phenomenon"/>
        <rdfs:subClassOf rdf:resource="http://purl.org/auto/criticality_phenomena#Real_Lidar_Criticality_Phenomenon"/>
        <rdfs:subClassOf rdf:resource="http://purl.org/auto/criticality_phenomena#Real_Perception_Algorithm_Criticality_Phenomenon"/>
        <rdfs:subClassOf rdf:resource="http://purl.org/auto/criticality_phenomena#Real_Radar_Criticality_Phenomenon"/>
        <formalized rdf:datatype="http://www.w3.org/2001/XMLSchema#boolean">true</formalized>
        <dcterms:identifier rdf:datatype="http://www.w3.org/2001/XMLSchema#nonNegativeInteger">17</dcterms:identifier>
        <rdfs:comment xml:lang="en">The presence and intensity of rain.</rdfs:comment>
        <rdfs:label xml:lang="en">Rain</rdfs:label>
        <rdfs:label xml:lang="de">Regen</rdfs:label>
    </owl:Class>
    


    <!-- http://purl.org/auto/criticality_phenomena#CP_170 -->

    <owl:Class rdf:about="http://purl.org/auto/criticality_phenomena#CP_170">
        <rdfs:subClassOf rdf:resource="http://purl.org/auto/criticality_phenomena#Behavioral_Criticality_Phenomenon"/>
        <rdfs:subClassOf rdf:resource="http://purl.org/auto/criticality_phenomena#CP_117"/>
        <dcterms:identifier rdf:datatype="http://www.w3.org/2001/XMLSchema#nonNegativeInteger">170</dcterms:identifier>
        <rdfs:comment xml:lang="en">Blue lights and siren signalize the priority of the emergency vehicle.</rdfs:comment>
        <rdfs:label xml:lang="de">Blaulicht und Sirene</rdfs:label>
        <rdfs:label xml:lang="en">Blue lights and siren</rdfs:label>
    </owl:Class>
    


    <!-- http://purl.org/auto/criticality_phenomena#CP_171 -->

    <owl:Class rdf:about="http://purl.org/auto/criticality_phenomena#CP_171">
        <rdfs:subClassOf rdf:resource="http://purl.org/auto/criticality_phenomena#CP_162"/>
        <rdfs:subClassOf rdf:resource="http://purl.org/auto/criticality_phenomena#Dynamical_Criticality_Phenomenon"/>
        <rdfs:subClassOf rdf:resource="http://purl.org/auto/criticality_phenomena#Perfect_Perception_Criticality_Phenomenon"/>
        <dcterms:identifier rdf:datatype="http://www.w3.org/2001/XMLSchema#nonNegativeInteger">171</dcterms:identifier>
        <rdfs:comment xml:lang="en">An incline that possibly endangers TPs if they do not adapt their behavior (e.g. through gear shifting). Can be indicated through a traffic sign.</rdfs:comment>
        <rdfs:label xml:lang="en">Incline Of Road</rdfs:label>
        <rdfs:label xml:lang="de">Straßensteigung</rdfs:label>
    </owl:Class>
    


    <!-- http://purl.org/auto/criticality_phenomena#CP_172 -->

    <owl:Class rdf:about="http://purl.org/auto/criticality_phenomena#CP_172">
        <rdfs:subClassOf rdf:resource="http://purl.org/auto/criticality_phenomena#CP_162"/>
        <rdfs:subClassOf rdf:resource="http://purl.org/auto/criticality_phenomena#Dynamical_Criticality_Phenomenon"/>
        <rdfs:subClassOf rdf:resource="http://purl.org/auto/criticality_phenomena#Perfect_Perception_Criticality_Phenomenon"/>
        <dcterms:identifier rdf:datatype="http://www.w3.org/2001/XMLSchema#nonNegativeInteger">172</dcterms:identifier>
        <rdfs:comment xml:lang="en">A decline that possibly endangers TPs if they do not adapt their behavior (e.g. through braking). Can be indicated through a traffic sign.</rdfs:comment>
        <rdfs:label xml:lang="en">Decline Of Road</rdfs:label>
        <rdfs:label xml:lang="de">Straßengefälle</rdfs:label>
    </owl:Class>
    


    <!-- http://purl.org/auto/criticality_phenomena#CP_173 -->

    <owl:Class rdf:about="http://purl.org/auto/criticality_phenomena#CP_173">
        <rdfs:subClassOf rdf:resource="http://purl.org/auto/criticality_phenomena#CP_162"/>
        <rdfs:subClassOf rdf:resource="http://purl.org/auto/criticality_phenomena#Dynamical_Criticality_Phenomenon"/>
        <rdfs:subClassOf rdf:resource="http://purl.org/auto/criticality_phenomena#Perfect_Perception_Criticality_Phenomenon"/>
        <dcterms:identifier rdf:datatype="http://www.w3.org/2001/XMLSchema#nonNegativeInteger">173</dcterms:identifier>
        <rdfs:comment xml:lang="en">Defined as the degree of curvature of a road (see civil engineering guidelines).</rdfs:comment>
        <rdfs:label xml:lang="en">Curvature Of Road</rdfs:label>
        <rdfs:label xml:lang="de">Kurvigkeit der Straße</rdfs:label>
    </owl:Class>
    


    <!-- http://purl.org/auto/criticality_phenomena#CP_174 -->

    <owl:Class rdf:about="http://purl.org/auto/criticality_phenomena#CP_174">
        <rdfs:subClassOf rdf:resource="http://purl.org/auto/criticality_phenomena#CP_173"/>
        <dcterms:identifier rdf:datatype="http://www.w3.org/2001/XMLSchema#nonNegativeInteger">174</dcterms:identifier>
        <rdfs:comment xml:lang="en">Typically, during curves, the decline is directed to the inside of the curve. This is the opposite case, where the decline is directed to the outside.</rdfs:comment>
        <rdfs:label xml:lang="en">Outside Decline Of Road During Turn</rdfs:label>
        <rdfs:label xml:lang="de">nach außen abfallende laterale Straßenneigung in Kurven</rdfs:label>
    </owl:Class>
    


    <!-- http://purl.org/auto/criticality_phenomena#CP_175 -->

    <owl:Class rdf:about="http://purl.org/auto/criticality_phenomena#CP_175">
        <rdfs:subClassOf rdf:resource="http://purl.org/auto/criticality_phenomena#CP_162"/>
        <rdfs:subClassOf rdf:resource="http://purl.org/auto/criticality_phenomena#Environmental_Criticality_Phenomenon"/>
        <rdfs:subClassOf rdf:resource="http://purl.org/auto/criticality_phenomena#Perfect_Perception_Criticality_Phenomenon"/>
        <dcterms:identifier rdf:datatype="http://www.w3.org/2001/XMLSchema#nonNegativeInteger">175</dcterms:identifier>
        <rdfs:comment xml:lang="en">The scenario contains a bridge.</rdfs:comment>
        <rdfs:label xml:lang="en">Bridge</rdfs:label>
        <rdfs:label xml:lang="de">Brücke</rdfs:label>
    </owl:Class>
    


    <!-- http://purl.org/auto/criticality_phenomena#CP_176 -->

    <owl:Class rdf:about="http://purl.org/auto/criticality_phenomena#CP_176">
        <rdfs:subClassOf rdf:resource="http://purl.org/auto/criticality_phenomena#CP_178"/>
        <rdfs:subClassOf rdf:resource="http://purl.org/auto/criticality_phenomena#Human_Criticality_Phenomenon"/>
        <dcterms:identifier rdf:datatype="http://www.w3.org/2001/XMLSchema#nonNegativeInteger">176</dcterms:identifier>
        <rdfs:comment xml:lang="en">The scenario contains a bicycle crossing.</rdfs:comment>
        <rdfs:label xml:lang="en">Bicycle Crossing</rdfs:label>
        <rdfs:label xml:lang="de">Radwegfurt</rdfs:label>
    </owl:Class>
    


    <!-- http://purl.org/auto/criticality_phenomena#CP_177 -->

    <owl:Class rdf:about="http://purl.org/auto/criticality_phenomena#CP_177">
        <rdfs:subClassOf rdf:resource="http://purl.org/auto/criticality_phenomena#CP_178"/>
        <rdfs:subClassOf rdf:resource="http://purl.org/auto/criticality_phenomena#Human_Criticality_Phenomenon"/>
        <formalized rdf:datatype="http://www.w3.org/2001/XMLSchema#boolean">true</formalized>
        <dcterms:identifier rdf:datatype="http://www.w3.org/2001/XMLSchema#nonNegativeInteger">177</dcterms:identifier>
        <rdfs:comment xml:lang="en">The scenario contains a pedestrian crossing (meaning both ford and crosswalk)</rdfs:comment>
        <rdfs:label xml:lang="de">Fußgängerfurt/-überweg</rdfs:label>
        <rdfs:label xml:lang="en">Pedestrian Crossing / Ford</rdfs:label>
    </owl:Class>
    


    <!-- http://purl.org/auto/criticality_phenomena#CP_178 -->

    <owl:Class rdf:about="http://purl.org/auto/criticality_phenomena#CP_178">
        <rdfs:subClassOf rdf:resource="http://purl.org/auto/criticality_phenomena#CP_286"/>
        <rdfs:subClassOf rdf:resource="http://purl.org/auto/criticality_phenomena#Perfect_Perception_Criticality_Phenomenon"/>
        <rdfs:subClassOf rdf:resource="http://purl.org/auto/criticality_phenomena#Spatial_Criticality_Phenomenon"/>
        <dcterms:identifier rdf:datatype="http://www.w3.org/2001/XMLSchema#nonNegativeInteger">178</dcterms:identifier>
        <rdfs:comment xml:lang="en">Increased probability of Intersecting Trajectories</rdfs:comment>
        <rdfs:label xml:lang="en">Intersection</rdfs:label>
        <rdfs:label xml:lang="de">Kreuzung</rdfs:label>
    </owl:Class>
    


    <!-- http://purl.org/auto/criticality_phenomena#CP_179 -->

    <owl:Class rdf:about="http://purl.org/auto/criticality_phenomena#CP_179">
        <rdfs:subClassOf rdf:resource="http://purl.org/auto/criticality_phenomena#CP_162"/>
        <rdfs:subClassOf rdf:resource="http://purl.org/auto/criticality_phenomena#Environmental_Criticality_Phenomenon"/>
        <rdfs:subClassOf rdf:resource="http://purl.org/auto/criticality_phenomena#Perfect_Perception_Criticality_Phenomenon"/>
        <dcterms:identifier rdf:datatype="http://www.w3.org/2001/XMLSchema#nonNegativeInteger">179</dcterms:identifier>
        <rdfs:comment xml:lang="en">A road covered with trees to both sides</rdfs:comment>
        <rdfs:label xml:lang="de">Allee</rdfs:label>
        <rdfs:label xml:lang="en">Avenue</rdfs:label>
    </owl:Class>
    


    <!-- http://purl.org/auto/criticality_phenomena#CP_18 -->

    <owl:Class rdf:about="http://purl.org/auto/criticality_phenomena#CP_18">
        <rdfs:subClassOf rdf:resource="http://purl.org/auto/criticality_phenomena#CP_273"/>
        <rdfs:subClassOf rdf:resource="http://purl.org/auto/criticality_phenomena#Real_Camera_Criticality_Phenomenon"/>
        <rdfs:subClassOf rdf:resource="http://purl.org/auto/criticality_phenomena#Real_Human_Criticality_Phenomenon"/>
        <rdfs:subClassOf rdf:resource="http://purl.org/auto/criticality_phenomena#Real_Perception_Algorithm_Criticality_Phenomenon"/>
        <dcterms:identifier rdf:datatype="http://www.w3.org/2001/XMLSchema#nonNegativeInteger">18</dcterms:identifier>
        <rdfs:comment xml:lang="en">Whether the global illumination source of the scenery is being limited. This includes dawn, twilight and night. Criticality depends on intensity/artificial light sources/sensor capability</rdfs:comment>
        <rdfs:label xml:lang="de">Eingeschränkte globale Lichtquelle</rdfs:label>
        <rdfs:label xml:lang="en">Reduced Global Light Source</rdfs:label>
    </owl:Class>
    


    <!-- http://purl.org/auto/criticality_phenomena#CP_180 -->

    <owl:Class rdf:about="http://purl.org/auto/criticality_phenomena#CP_180">
        <rdfs:subClassOf rdf:resource="http://purl.org/auto/criticality_phenomena#CP_212"/>
        <rdfs:subClassOf rdf:resource="http://purl.org/auto/criticality_phenomena#Environmental_Criticality_Phenomenon"/>
        <rdfs:subClassOf rdf:resource="http://purl.org/auto/criticality_phenomena#Perfect_Perception_Criticality_Phenomenon"/>
        <dcterms:identifier rdf:datatype="http://www.w3.org/2001/XMLSchema#nonNegativeInteger">180</dcterms:identifier>
        <rdfs:comment xml:lang="en">Water bodies such as lakes and rivers to the side of the road. Can increase the probablity of fog.</rdfs:comment>
        <rdfs:label xml:lang="de">Gewässer in Straßennähe</rdfs:label>
        <rdfs:label xml:lang="en">Water Bodies Near Road</rdfs:label>
    </owl:Class>
    


    <!-- http://purl.org/auto/criticality_phenomena#CP_181 -->

    <owl:Class rdf:about="http://purl.org/auto/criticality_phenomena#CP_181">
        <rdfs:subClassOf rdf:resource="http://purl.org/auto/criticality_phenomena#CP_286"/>
        <rdfs:subClassOf rdf:resource="http://purl.org/auto/criticality_phenomena#Human_Criticality_Phenomenon"/>
        <rdfs:subClassOf rdf:resource="http://purl.org/auto/criticality_phenomena#Perfect_Perception_Criticality_Phenomenon"/>
        <rdfs:subClassOf rdf:resource="http://purl.org/auto/criticality_phenomena#Unpredictability_Criticality_Phenomenon"/>
        <dcterms:identifier rdf:datatype="http://www.w3.org/2001/XMLSchema#nonNegativeInteger">181</dcterms:identifier>
        <rdfs:comment xml:lang="en">A building exists in proximity to the road in which a larger number of URUs is present, e.g. kindergarden, school, retirement home, disabled home.</rdfs:comment>
        <rdfs:label xml:lang="en">Building For URUs Near Road</rdfs:label>
        <rdfs:label xml:lang="de">Gebäude für URUs an der Straße</rdfs:label>
    </owl:Class>
    


    <!-- http://purl.org/auto/criticality_phenomena#CP_182 -->

    <owl:Class rdf:about="http://purl.org/auto/criticality_phenomena#CP_182">
        <rdfs:subClassOf rdf:resource="http://purl.org/auto/criticality_phenomena#CP_208"/>
        <rdfs:subClassOf rdf:resource="http://purl.org/auto/criticality_phenomena#Perfect_Perception_Criticality_Phenomenon"/>
        <dcterms:identifier rdf:datatype="http://www.w3.org/2001/XMLSchema#nonNegativeInteger">182</dcterms:identifier>
        <rdfs:comment xml:lang="en">Any advertisements (digital, analog, ...) close to the road. They can lead to False Positives in Object Recognition.</rdfs:comment>
        <rdfs:label xml:lang="en">Advertising Space Near Road</rdfs:label>
        <rdfs:label xml:lang="de">Werbefläche an der Straße</rdfs:label>
    </owl:Class>
    


    <!-- http://purl.org/auto/criticality_phenomena#CP_183 -->

    <owl:Class rdf:about="http://purl.org/auto/criticality_phenomena#CP_183">
        <rdfs:subClassOf rdf:resource="http://purl.org/auto/criticality_phenomena#CP_208"/>
        <rdfs:subClassOf rdf:resource="http://purl.org/auto/criticality_phenomena#Perfect_Perception_Criticality_Phenomenon"/>
        <dcterms:identifier rdf:datatype="http://www.w3.org/2001/XMLSchema#nonNegativeInteger">183</dcterms:identifier>
        <rdfs:comment xml:lang="en">Deviation from the norm state of a road, e.g. through potholes, tar joint, lane grooves. Criticality depends on type and degree of degradation.</rdfs:comment>
        <rdfs:label xml:lang="en">Degraded Road Quality</rdfs:label>
        <rdfs:label xml:lang="de">Degradierte Straßenqualität</rdfs:label>
    </owl:Class>
    


    <!-- http://purl.org/auto/criticality_phenomena#CP_184 -->

    <owl:Class rdf:about="http://purl.org/auto/criticality_phenomena#CP_184">
        <rdfs:subClassOf rdf:resource="http://purl.org/auto/criticality_phenomena#CP_208"/>
        <rdfs:subClassOf rdf:resource="http://purl.org/auto/criticality_phenomena#Perfect_Perception_Criticality_Phenomenon"/>
        <dcterms:identifier rdf:datatype="http://www.w3.org/2001/XMLSchema#nonNegativeInteger">184</dcterms:identifier>
        <rdfs:comment xml:lang="en">A road surface material which reduces the driving quality, e.g. cobblestones, setts, bitumen, ...</rdfs:comment>
        <rdfs:label xml:lang="en">Bad Road Surface</rdfs:label>
        <rdfs:label xml:lang="de">Schlechter Straßenbelag</rdfs:label>
    </owl:Class>
    


    <!-- http://purl.org/auto/criticality_phenomena#CP_185 -->

    <owl:Class rdf:about="http://purl.org/auto/criticality_phenomena#CP_185">
        <rdfs:subClassOf rdf:resource="http://purl.org/auto/criticality_phenomena#CP_208"/>
        <rdfs:subClassOf rdf:resource="http://purl.org/auto/criticality_phenomena#Perfect_Perception_Criticality_Phenomenon"/>
        <dcterms:identifier rdf:datatype="http://www.w3.org/2001/XMLSchema#nonNegativeInteger">185</dcterms:identifier>
        <rdfs:comment xml:lang="en">Meaning the friction between tires and road. The criticality depends on degree of reduction.</rdfs:comment>
        <rdfs:label xml:lang="en">Reduced Friction On Road</rdfs:label>
        <rdfs:label xml:lang="de">verminderte Straßenhaftung</rdfs:label>
    </owl:Class>
    


    <!-- http://purl.org/auto/criticality_phenomena#CP_186 -->

    <owl:Class rdf:about="http://purl.org/auto/criticality_phenomena#CP_186">
        <rdfs:subClassOf rdf:resource="http://purl.org/auto/criticality_phenomena#CP_18"/>
        <rdfs:subClassOf rdf:resource="http://purl.org/auto/criticality_phenomena#Environmental_Criticality_Phenomenon"/>
        <dcterms:identifier rdf:datatype="http://www.w3.org/2001/XMLSchema#nonNegativeInteger">186</dcterms:identifier>
        <rdfs:comment xml:lang="en">There is little global light at night. Therefore, light-dependent sensors such as the camera can be affected.</rdfs:comment>
        <rdfs:label xml:lang="de">Nacht</rdfs:label>
        <rdfs:label xml:lang="en">Night</rdfs:label>
    </owl:Class>
    


    <!-- http://purl.org/auto/criticality_phenomena#CP_187 -->

    <owl:Class rdf:about="http://purl.org/auto/criticality_phenomena#CP_187">
        <rdfs:subClassOf rdf:resource="http://purl.org/auto/criticality_phenomena#CP_18"/>
        <rdfs:subClassOf rdf:resource="http://purl.org/auto/criticality_phenomena#Environmental_Criticality_Phenomenon"/>
        <dcterms:identifier rdf:datatype="http://www.w3.org/2001/XMLSchema#nonNegativeInteger">187</dcterms:identifier>
        <rdfs:comment xml:lang="en">Dusk is the time of the beginning of twilight after sundown. It is related to scattered, diffused light. Therefore it might affect the capabilitiy of light sensitive sensors.</rdfs:comment>
        <rdfs:label xml:lang="de">Abenddämmerung</rdfs:label>
        <rdfs:label xml:lang="en">Dusk</rdfs:label>
    </owl:Class>
    


    <!-- http://purl.org/auto/criticality_phenomena#CP_188 -->

    <owl:Class rdf:about="http://purl.org/auto/criticality_phenomena#CP_188">
        <rdfs:subClassOf rdf:resource="http://purl.org/auto/criticality_phenomena#CP_18"/>
        <rdfs:subClassOf rdf:resource="http://purl.org/auto/criticality_phenomena#Environmental_Criticality_Phenomenon"/>
        <dcterms:identifier rdf:datatype="http://www.w3.org/2001/XMLSchema#nonNegativeInteger">188</dcterms:identifier>
        <rdfs:comment xml:lang="en">Dawn is the time of the beginning of twilight before sunrise. It is related to scattered, diffused light. Therefore it might affect the capabilitiy of light sensitive sensors.</rdfs:comment>
        <rdfs:label xml:lang="en">Dawn</rdfs:label>
        <rdfs:label xml:lang="de">Morgendämmerung</rdfs:label>
    </owl:Class>
    


    <!-- http://purl.org/auto/criticality_phenomena#CP_189 -->

    <owl:Class rdf:about="http://purl.org/auto/criticality_phenomena#CP_189">
        <rdfs:subClassOf rdf:resource="http://purl.org/auto/criticality_phenomena#CP_273"/>
        <rdfs:subClassOf rdf:resource="http://purl.org/auto/criticality_phenomena#Perfect_Camera_Criticality_Phenomenon"/>
        <rdfs:subClassOf rdf:resource="http://purl.org/auto/criticality_phenomena#Perfect_Human_Criticality_Phenomenon"/>
        <rdfs:subClassOf rdf:resource="http://purl.org/auto/criticality_phenomena#Perfect_Lidar_Criticality_Phenomenon"/>
        <dcterms:identifier rdf:datatype="http://www.w3.org/2001/XMLSchema#nonNegativeInteger">189</dcterms:identifier>
        <rdfs:comment xml:lang="en">Air particles are microscopic particles of solid or liquid matter suspended in the air. They might affect the capability of sensors to return the right data.</rdfs:comment>
        <rdfs:label xml:lang="en">Air Particle</rdfs:label>
        <rdfs:label xml:lang="de">Luftpartikel</rdfs:label>
    </owl:Class>
    


    <!-- http://purl.org/auto/criticality_phenomena#CP_19 -->

    <owl:Class rdf:about="http://purl.org/auto/criticality_phenomena#CP_19">
        <rdfs:subClassOf rdf:resource="http://purl.org/auto/criticality_phenomena#CP_273"/>
        <rdfs:subClassOf rdf:resource="http://purl.org/auto/criticality_phenomena#Real_Camera_Criticality_Phenomenon"/>
        <rdfs:subClassOf rdf:resource="http://purl.org/auto/criticality_phenomena#Real_Human_Criticality_Phenomenon"/>
        <rdfs:subClassOf rdf:resource="http://purl.org/auto/criticality_phenomena#Real_Perception_Algorithm_Criticality_Phenomenon"/>
        <dcterms:identifier rdf:datatype="http://www.w3.org/2001/XMLSchema#nonNegativeInteger">19</dcterms:identifier>
        <rdfs:comment xml:lang="en">The brightness condition alternates over time or space, e.g. disco effect driving through avenues, entering/exiting tunnels, fast partial clouds.</rdfs:comment>
        <rdfs:label xml:lang="en">Alternating/changing Brightness</rdfs:label>
        <rdfs:label xml:lang="de">Änderung / wechselnde Helligkeit</rdfs:label>
    </owl:Class>
    


    <!-- http://purl.org/auto/criticality_phenomena#CP_190 -->

    <owl:Class rdf:about="http://purl.org/auto/criticality_phenomena#CP_190">
        <rdfs:subClassOf rdf:resource="http://purl.org/auto/criticality_phenomena#CP_189"/>
        <rdfs:subClassOf rdf:resource="http://purl.org/auto/criticality_phenomena#CP_274"/>
        <dcterms:identifier rdf:datatype="http://www.w3.org/2001/XMLSchema#nonNegativeInteger">190</dcterms:identifier>
        <rdfs:comment xml:lang="en">Dust particles in the surrounding air. Might affect sensor data.</rdfs:comment>
        <rdfs:label xml:lang="en">Dust</rdfs:label>
        <rdfs:label xml:lang="de">Staub</rdfs:label>
    </owl:Class>
    


    <!-- http://purl.org/auto/criticality_phenomena#CP_191 -->

    <owl:Class rdf:about="http://purl.org/auto/criticality_phenomena#CP_191">
        <rdfs:subClassOf rdf:resource="http://purl.org/auto/criticality_phenomena#CP_189"/>
        <rdfs:subClassOf rdf:resource="http://purl.org/auto/criticality_phenomena#Dynamical_Criticality_Phenomenon"/>
        <dcterms:identifier rdf:datatype="http://www.w3.org/2001/XMLSchema#nonNegativeInteger">191</dcterms:identifier>
        <rdfs:comment xml:lang="en">Sandparticle in the surrounding air. Might affect sensor data.</rdfs:comment>
        <rdfs:label xml:lang="de">Sand</rdfs:label>
        <rdfs:label xml:lang="en">Sand</rdfs:label>
    </owl:Class>
    


    <!-- http://purl.org/auto/criticality_phenomena#CP_192 -->

    <owl:Class rdf:about="http://purl.org/auto/criticality_phenomena#CP_192">
        <rdfs:subClassOf rdf:resource="http://purl.org/auto/criticality_phenomena#CP_56"/>
        <rdfs:subClassOf rdf:resource="http://purl.org/auto/criticality_phenomena#Perfect_Camera_Criticality_Phenomenon"/>
        <rdfs:subClassOf rdf:resource="http://purl.org/auto/criticality_phenomena#Perfect_Human_Criticality_Phenomenon"/>
        <rdfs:subClassOf rdf:resource="http://purl.org/auto/criticality_phenomena#Unpredictability_Criticality_Phenomenon"/>
        <dcterms:identifier rdf:datatype="http://www.w3.org/2001/XMLSchema#nonNegativeInteger">192</dcterms:identifier>
        <rdfs:comment xml:lang="en">A road user is blinded by the high beam of another road user. In the case of a human driver, this can have an impact on driving behavior. In the case of an automated vehicle, light-sensing sensors such as the camera or lidar can be affected.</rdfs:comment>
        <rdfs:label xml:lang="de">Blendung durch Fernlicht eines anderen TPs</rdfs:label>
        <rdfs:label xml:lang="en">Glare Due To High Beam Of Non-Ego-TP</rdfs:label>
    </owl:Class>
    


    <!-- http://purl.org/auto/criticality_phenomena#CP_193 -->

    <owl:Class rdf:about="http://purl.org/auto/criticality_phenomena#CP_193">
        <rdfs:subClassOf rdf:resource="http://purl.org/auto/criticality_phenomena#CP_185"/>
        <rdfs:subClassOf rdf:resource="http://purl.org/auto/criticality_phenomena#Environmental_Criticality_Phenomenon"/>
        <dcterms:identifier rdf:datatype="http://www.w3.org/2001/XMLSchema#nonNegativeInteger">193</dcterms:identifier>
        <rdfs:comment xml:lang="en">A layer of water builds between the wheels of the vehicle and the road surface. This leads to loss of traction which then leads to the vehicle not responding to control.</rdfs:comment>
        <rdfs:label xml:lang="de">Aquaplaning</rdfs:label>
        <rdfs:label xml:lang="en">Aquaplaning</rdfs:label>
    </owl:Class>
    


    <!-- http://purl.org/auto/criticality_phenomena#CP_194 -->

    <owl:Class rdf:about="http://purl.org/auto/criticality_phenomena#CP_194">
        <rdfs:subClassOf rdf:resource="http://purl.org/auto/criticality_phenomena#CP_272"/>
        <rdfs:subClassOf rdf:resource="http://purl.org/auto/criticality_phenomena#Perfect_Lidar_Criticality_Phenomenon"/>
        <rdfs:subClassOf rdf:resource="http://purl.org/auto/criticality_phenomena#Real_Camera_Criticality_Phenomenon"/>
        <rdfs:subClassOf rdf:resource="http://purl.org/auto/criticality_phenomena#Real_Human_Criticality_Phenomenon"/>
        <rdfs:subClassOf rdf:resource="http://purl.org/auto/criticality_phenomena#Real_Perception_Algorithm_Criticality_Phenomenon"/>
        <dcterms:identifier rdf:datatype="http://www.w3.org/2001/XMLSchema#nonNegativeInteger">194</dcterms:identifier>
        <rdfs:comment xml:lang="en">Perception of an entity that does not exist in reality. Contains existence uncertainty, false positives.
- Example: Perception of a pedestrian on the road side which does not exist.</rdfs:comment>
        <rdfs:label xml:lang="de">Geisterobjekt</rdfs:label>
        <rdfs:label xml:lang="en">Ghost Perception</rdfs:label>
    </owl:Class>
    


    <!-- http://purl.org/auto/criticality_phenomena#CP_195 -->

    <owl:Class rdf:about="http://purl.org/auto/criticality_phenomena#CP_195">
        <rdfs:subClassOf rdf:resource="http://purl.org/auto/criticality_phenomena#CP_272"/>
        <dcterms:identifier rdf:datatype="http://www.w3.org/2001/XMLSchema#nonNegativeInteger">195</dcterms:identifier>
        <rdfs:comment xml:lang="en">Missing perception of an existing entity. Contains existence uncertainty, false negatives.
- Example: Pedestrian exists in reality, but is not perceived (e.g. due to occlusion)</rdfs:comment>
        <rdfs:label xml:lang="de">Keine Perzeption</rdfs:label>
        <rdfs:label xml:lang="en">No Perception</rdfs:label>
    </owl:Class>
    


    <!-- http://purl.org/auto/criticality_phenomena#CP_196 -->

    <owl:Class rdf:about="http://purl.org/auto/criticality_phenomena#CP_196">
        <rdfs:subClassOf rdf:resource="http://purl.org/auto/criticality_phenomena#CP_272"/>
        <dcterms:identifier rdf:datatype="http://www.w3.org/2001/XMLSchema#nonNegativeInteger">196</dcterms:identifier>
        <rdfs:comment xml:lang="en">Relevant properties are only partially perceived.
- Example: &quot;velocity&quot; of a vehicle is perceived, but property &quot;acceleration&quot; is not perceived.</rdfs:comment>
        <rdfs:label xml:lang="en">Partial Perception</rdfs:label>
        <rdfs:label xml:lang="de">Teilperzeption</rdfs:label>
    </owl:Class>
    


    <!-- http://purl.org/auto/criticality_phenomena#CP_197 -->

    <owl:Class rdf:about="http://purl.org/auto/criticality_phenomena#CP_197">
        <rdfs:subClassOf rdf:resource="http://purl.org/auto/criticality_phenomena#CP_272"/>
        <rdfs:subClassOf rdf:resource="http://purl.org/auto/criticality_phenomena#Real_Camera_Criticality_Phenomenon"/>
        <rdfs:subClassOf rdf:resource="http://purl.org/auto/criticality_phenomena#Real_Human_Criticality_Phenomenon"/>
        <rdfs:subClassOf rdf:resource="http://purl.org/auto/criticality_phenomena#Real_Lidar_Criticality_Phenomenon"/>
        <rdfs:subClassOf rdf:resource="http://purl.org/auto/criticality_phenomena#Real_Perception_Algorithm_Criticality_Phenomenon"/>
        <rdfs:subClassOf rdf:resource="http://purl.org/auto/criticality_phenomena#Real_Radar_Criticality_Phenomenon"/>
        <dcterms:identifier rdf:datatype="http://www.w3.org/2001/XMLSchema#nonNegativeInteger">197</dcterms:identifier>
        <rdfs:comment xml:lang="en">Correctly perceived existence and classification, but classification and properties are too abstract, imprecise or uncertain to aid in decision making. Includes state uncertainty.
- Example: Classification of a stinger as &quot;small object&quot;.
- Example 2:  Assignment of property &quot;v&quot; to some vehicle with &quot;v in [1,100] km/h&quot;
- Example 3: Assignment of property &quot;dist = 10 m&quot; to some vehicle in front with &quot;95% confidence interval = [5,50] m&quot;</rdfs:comment>
        <rdfs:label xml:lang="en">Imprecise Perception</rdfs:label>
        <rdfs:label xml:lang="de">Ungenaue Perzeption</rdfs:label>
    </owl:Class>
    


    <!-- http://purl.org/auto/criticality_phenomena#CP_198 -->

    <owl:Class rdf:about="http://purl.org/auto/criticality_phenomena#CP_198">
        <rdfs:subClassOf rdf:resource="http://purl.org/auto/criticality_phenomena#CP_272"/>
        <rdfs:subClassOf rdf:resource="http://purl.org/auto/criticality_phenomena#Real_Camera_Criticality_Phenomenon"/>
        <rdfs:subClassOf rdf:resource="http://purl.org/auto/criticality_phenomena#Real_Human_Criticality_Phenomenon"/>
        <rdfs:subClassOf rdf:resource="http://purl.org/auto/criticality_phenomena#Real_Lidar_Criticality_Phenomenon"/>
        <rdfs:subClassOf rdf:resource="http://purl.org/auto/criticality_phenomena#Real_Perception_Algorithm_Criticality_Phenomenon"/>
        <rdfs:subClassOf rdf:resource="http://purl.org/auto/criticality_phenomena#Real_Radar_Criticality_Phenomenon"/>
        <dcterms:identifier rdf:datatype="http://www.w3.org/2001/XMLSchema#nonNegativeInteger">198</dcterms:identifier>
        <rdfs:comment xml:lang="en">Correctly perceived existence, but wrong attributation, e.g. class label or property of entity. Can include classification uncertainty.
- Example 1: Classification of a pedestrian as a bicyclist
- Example 2: Assignment of property &quot;v = 100km/h&quot; with 95% confidence interval = [99,101] km/h to a 10 km/h fast vehicle</rdfs:comment>
        <rdfs:label xml:lang="de">Fehlperzeption</rdfs:label>
        <rdfs:label xml:lang="en">Mis-perception</rdfs:label>
    </owl:Class>
    


    <!-- http://purl.org/auto/criticality_phenomena#CP_199 -->

    <owl:Class rdf:about="http://purl.org/auto/criticality_phenomena#CP_199">
        <rdfs:subClassOf rdf:resource="http://purl.org/auto/criticality_phenomena#CP_196"/>
        <dcterms:identifier rdf:datatype="http://www.w3.org/2001/XMLSchema#nonNegativeInteger">199</dcterms:identifier>
        <rdfs:comment xml:lang="en">Bird shit, plastic bag, mud, frost, ...</rdfs:comment>
        <rdfs:label xml:lang="en">Physically Blocked Sensor</rdfs:label>
        <rdfs:label xml:lang="de">Physikalisch blockierter Sensor</rdfs:label>
    </owl:Class>
    


    <!-- http://purl.org/auto/criticality_phenomena#CP_2 -->

    <owl:Class rdf:about="http://purl.org/auto/criticality_phenomena#CP_2">
        <rdfs:subClassOf rdf:resource="http://purl.org/auto/criticality_phenomena#CP_216"/>
        <rdfs:subClassOf rdf:resource="http://purl.org/auto/criticality_phenomena#Perfect_Perception_Criticality_Phenomenon"/>
        <dcterms:identifier rdf:datatype="http://www.w3.org/2001/XMLSchema#nonNegativeInteger">2</dcterms:identifier>
        <rdfs:comment xml:lang="en">A VRU has a planned trajectory that intersects with the planned trajectory of the ego. Standard situation at urban intersections.</rdfs:comment>
        <rdfs:label xml:lang="en">Intersecting VRU During Right Turn</rdfs:label>
        <rdfs:label xml:lang="de">Kreuzender VRU beim Rechts abbiegen</rdfs:label>
    </owl:Class>
    


    <!-- http://purl.org/auto/criticality_phenomena#CP_20 -->

    <owl:Class rdf:about="http://purl.org/auto/criticality_phenomena#CP_20">
        <rdfs:subClassOf rdf:resource="http://purl.org/auto/criticality_phenomena#CP_56"/>
        <rdfs:subClassOf rdf:resource="http://purl.org/auto/criticality_phenomena#Environmental_Criticality_Phenomenon"/>
        <dcterms:identifier rdf:datatype="http://www.w3.org/2001/XMLSchema#nonNegativeInteger">20</dcterms:identifier>
        <rdfs:comment xml:lang="en">Glare directly from the sun, through reflections (e.g. buildings, water, ...), </rdfs:comment>
        <rdfs:label xml:lang="de">Blendung durch Sonnenlicht</rdfs:label>
        <rdfs:label xml:lang="en">Glare Due To Sunlight</rdfs:label>
    </owl:Class>
    


    <!-- http://purl.org/auto/criticality_phenomena#CP_200 -->

    <owl:Class rdf:about="http://purl.org/auto/criticality_phenomena#CP_200">
        <rdfs:subClassOf rdf:resource="http://purl.org/auto/criticality_phenomena#CP_215"/>
        <dcterms:identifier rdf:datatype="http://www.w3.org/2001/XMLSchema#nonNegativeInteger">200</dcterms:identifier>
        <rdfs:comment xml:lang="en">Undirected reflection of a part of the electromagnetic spectrum.</rdfs:comment>
        <rdfs:label xml:lang="de">Diffus reflektierende Oberflächen</rdfs:label>
        <rdfs:label xml:lang="en">Diffuse-reflecting Surfaces</rdfs:label>
    </owl:Class>
    


    <!-- http://purl.org/auto/criticality_phenomena#CP_201 -->

    <owl:Class rdf:about="http://purl.org/auto/criticality_phenomena#CP_201">
        <rdfs:subClassOf rdf:resource="http://purl.org/auto/criticality_phenomena#CP_200"/>
        <dcterms:identifier rdf:datatype="http://www.w3.org/2001/XMLSchema#nonNegativeInteger">201</dcterms:identifier>
        <rdfs:comment xml:lang="en">Pedestriants wearing a fur coat are less likely recognized by lidar sensors.</rdfs:comment>
        <rdfs:label xml:lang="en">Fur Coat</rdfs:label>
        <rdfs:label xml:lang="de">Pelzmantel</rdfs:label>
    </owl:Class>
    


    <!-- http://purl.org/auto/criticality_phenomena#CP_202 -->

    <owl:Class rdf:about="http://purl.org/auto/criticality_phenomena#CP_202">
        <rdfs:subClassOf rdf:resource="http://purl.org/auto/criticality_phenomena#CP_12"/>
        <dcterms:identifier rdf:datatype="http://www.w3.org/2001/XMLSchema#nonNegativeInteger">202</dcterms:identifier>
        <rdfs:comment xml:lang="en">A wet road is a road whose surface is wetted with a liquid. This can lead to a loss of road friction.</rdfs:comment>
        <rdfs:label xml:lang="de">Nasse Straße</rdfs:label>
        <rdfs:label xml:lang="en">Wet Road</rdfs:label>
    </owl:Class>
    


    <!-- http://purl.org/auto/criticality_phenomena#CP_203 -->

    <owl:Class rdf:about="http://purl.org/auto/criticality_phenomena#CP_203">
        <rdfs:subClassOf rdf:resource="http://purl.org/auto/criticality_phenomena#CP_274"/>
        <rdfs:subClassOf rdf:resource="http://purl.org/auto/criticality_phenomena#Dynamical_Criticality_Phenomenon"/>
        <dcterms:identifier rdf:datatype="http://www.w3.org/2001/XMLSchema#nonNegativeInteger">203</dcterms:identifier>
        <rdfs:comment xml:lang="en">An icy road is covered with a film of ice. This affects road friction and the response to steering and braking maneuvers as well as the response to acceleration.</rdfs:comment>
        <rdfs:label xml:lang="en">Icy Road</rdfs:label>
        <rdfs:label xml:lang="de">Vereiste Straße</rdfs:label>
    </owl:Class>
    


    <!-- http://purl.org/auto/criticality_phenomena#CP_204 -->

    <owl:Class rdf:about="http://purl.org/auto/criticality_phenomena#CP_204">
        <rdfs:subClassOf rdf:resource="http://purl.org/auto/criticality_phenomena#CP_12"/>
        <dcterms:identifier rdf:datatype="http://www.w3.org/2001/XMLSchema#nonNegativeInteger">204</dcterms:identifier>
        <rdfs:comment xml:lang="en">Camera Lense</rdfs:comment>
        <rdfs:label xml:lang="de">Frost</rdfs:label>
        <rdfs:label xml:lang="en">Frost</rdfs:label>
    </owl:Class>
    


    <!-- http://purl.org/auto/criticality_phenomena#CP_206 -->

    <owl:Class rdf:about="http://purl.org/auto/criticality_phenomena#CP_206">
        <rdfs:subClassOf rdf:resource="http://purl.org/auto/criticality_phenomena#CP_215"/>
        <rdfs:subClassOf rdf:resource="http://purl.org/auto/criticality_phenomena#Real_Human_Criticality_Phenomenon"/>
        <rdfs:subClassOf rdf:resource="http://purl.org/auto/criticality_phenomena#Real_Perception_Algorithm_Criticality_Phenomenon"/>
        <dcterms:identifier rdf:datatype="http://www.w3.org/2001/XMLSchema#nonNegativeInteger">206</dcterms:identifier>
        <rdfs:comment xml:lang="en">Objects in near reflecting surfaces appear twice in the environment according to light source angle, distance and position relative to reflecting surface.</rdfs:comment>
        <rdfs:label xml:lang="en">Mirroring</rdfs:label>
        <rdfs:label xml:lang="de">Spiegelung</rdfs:label>
    </owl:Class>
    


    <!-- http://purl.org/auto/criticality_phenomena#CP_207 -->

    <owl:Class rdf:about="http://purl.org/auto/criticality_phenomena#CP_207">
        <rdfs:subClassOf rdf:resource="http://purl.org/auto/criticality_phenomena#CP_212"/>
        <rdfs:subClassOf rdf:resource="http://purl.org/auto/criticality_phenomena#Unpredictability_Criticality_Phenomenon"/>
        <dcterms:identifier rdf:datatype="http://www.w3.org/2001/XMLSchema#nonNegativeInteger">207</dcterms:identifier>
        <rdfs:comment xml:lang="en">ToDo</rdfs:comment>
        <rdfs:label xml:lang="en">Miscellaneaous Object On Road</rdfs:label>
        <rdfs:label xml:lang="de">Sonstiges Objekt auf der Straße</rdfs:label>
    </owl:Class>
    


    <!-- http://purl.org/auto/criticality_phenomena#CP_208 -->

    <owl:Class rdf:about="http://purl.org/auto/criticality_phenomena#CP_208">
        <rdfs:subClassOf rdf:resource="http://purl.org/auto/criticality_phenomena#CP_276"/>
        <rdfs:subClassOf rdf:resource="http://purl.org/auto/criticality_phenomena#Dynamical_Criticality_Phenomenon"/>
        <rdfs:subClassOf rdf:resource="http://purl.org/auto/criticality_phenomena#Environmental_Criticality_Phenomenon"/>
        <rdfs:subClassOf rdf:resource="http://purl.org/auto/criticality_phenomena#Spatial_Criticality_Phenomenon"/>
        <dcterms:identifier rdf:datatype="http://www.w3.org/2001/XMLSchema#nonNegativeInteger">208</dcterms:identifier>
        <rdfs:comment xml:lang="en">The condition of the road is in an abnormal condition. This could be due to temporal change or wear.</rdfs:comment>
        <rdfs:label xml:lang="de">Abnormaler Straßenzustand</rdfs:label>
        <rdfs:label xml:lang="en">Special Road Condition</rdfs:label>
    </owl:Class>
    


    <!-- http://purl.org/auto/criticality_phenomena#CP_209 -->

    <owl:Class rdf:about="http://purl.org/auto/criticality_phenomena#CP_209">
        <rdfs:subClassOf rdf:resource="http://purl.org/auto/criticality_phenomena#CP_208"/>
        <rdfs:subClassOf rdf:resource="http://purl.org/auto/criticality_phenomena#CP_276"/>
        <dcterms:identifier rdf:datatype="http://www.w3.org/2001/XMLSchema#nonNegativeInteger">209</dcterms:identifier>
        <rdfs:comment xml:lang="en">Lane markings are in an abnormal state. This might be temporary or permanent.</rdfs:comment>
        <rdfs:label xml:lang="de">Abnormale Straßenmarkierung</rdfs:label>
        <rdfs:label xml:lang="en">Special Lane Markings</rdfs:label>
    </owl:Class>
    


    <!-- http://purl.org/auto/criticality_phenomena#CP_21 -->

    <owl:Class rdf:about="http://purl.org/auto/criticality_phenomena#CP_21">
        <rdfs:subClassOf rdf:resource="http://purl.org/auto/criticality_phenomena#CP_274"/>
        <rdfs:subClassOf rdf:resource="http://purl.org/auto/criticality_phenomena#Real_Camera_Criticality_Phenomenon"/>
        <rdfs:subClassOf rdf:resource="http://purl.org/auto/criticality_phenomena#Real_Human_Criticality_Phenomenon"/>
        <rdfs:subClassOf rdf:resource="http://purl.org/auto/criticality_phenomena#Real_Lidar_Criticality_Phenomenon"/>
        <rdfs:subClassOf rdf:resource="http://purl.org/auto/criticality_phenomena#Real_Radar_Criticality_Phenomenon"/>
        <dcterms:identifier rdf:datatype="http://www.w3.org/2001/XMLSchema#nonNegativeInteger">21</dcterms:identifier>
        <rdfs:comment xml:lang="en">A change in temperature during a scenario, e.g. direct sun exposure of vehicle parts in hot climates. Criticality depends on intensity and degraded functionality of system components.</rdfs:comment>
        <rdfs:label xml:lang="en">Extreme (change In) Temperature</rdfs:label>
        <rdfs:label xml:lang="de">extreme (Veränderung der) Temperaturen</rdfs:label>
    </owl:Class>
    


    <!-- http://purl.org/auto/criticality_phenomena#CP_210 -->

    <owl:Class rdf:about="http://purl.org/auto/criticality_phenomena#CP_210">
        <rdfs:subClassOf rdf:resource="http://purl.org/auto/criticality_phenomena#CP_234"/>
        <rdfs:subClassOf rdf:resource="http://purl.org/auto/criticality_phenomena#Real_Camera_Criticality_Phenomenon"/>
        <rdfs:subClassOf rdf:resource="http://purl.org/auto/criticality_phenomena#Real_Human_Criticality_Phenomenon"/>
        <rdfs:subClassOf rdf:resource="http://purl.org/auto/criticality_phenomena#Real_Lidar_Criticality_Phenomenon"/>
        <dcterms:identifier rdf:datatype="http://www.w3.org/2001/XMLSchema#nonNegativeInteger">210</dcterms:identifier>
        <rdfs:comment xml:lang="en">Wikipedia: Temporal light interference (TLI) is an unacceptable degradation of the performance of an equipment or system that has an optical input for its intended functioning and is caused by a temporal light modulation disturbance.</rdfs:comment>
        <rdfs:label xml:lang="en">Temporal Light Effects</rdfs:label>
        <rdfs:label xml:lang="de">Temporäre Licht Effekte</rdfs:label>
    </owl:Class>
    


    <!-- http://purl.org/auto/criticality_phenomena#CP_211 -->

    <owl:Class rdf:about="http://purl.org/auto/criticality_phenomena#CP_211">
        <rdfs:subClassOf rdf:resource="http://purl.org/auto/criticality_phenomena#Behavioral_Criticality_Phenomenon"/>
        <rdfs:subClassOf rdf:resource="http://purl.org/auto/criticality_phenomena#CP_276"/>
        <dcterms:identifier rdf:datatype="http://www.w3.org/2001/XMLSchema#nonNegativeInteger">211</dcterms:identifier>
        <rdfs:comment xml:lang="en">Signs are in an abnormal state. This might be temporary or permanent.</rdfs:comment>
        <rdfs:label xml:lang="de">Abnormale Beschilderung</rdfs:label>
        <rdfs:label xml:lang="en">Special Signage</rdfs:label>
    </owl:Class>
    


    <!-- http://purl.org/auto/criticality_phenomena#CP_212 -->

    <owl:Class rdf:about="http://purl.org/auto/criticality_phenomena#CP_212">
        <rdfs:subClassOf rdf:resource="http://purl.org/auto/criticality_phenomena#CP_278"/>
        <rdfs:subClassOf rdf:resource="http://purl.org/auto/criticality_phenomena#Dynamical_Criticality_Phenomenon"/>
        <rdfs:subClassOf rdf:resource="http://purl.org/auto/criticality_phenomena#Perception_Criticality_Phenomenon"/>
        <dcterms:identifier rdf:datatype="http://www.w3.org/2001/XMLSchema#nonNegativeInteger">212</dcterms:identifier>
        <rdfs:comment xml:lang="en">There is an object on the road surface. This object might be a TP or anything other like e.g. a ball.</rdfs:comment>
        <rdfs:label xml:lang="en">Entity On Road</rdfs:label>
        <rdfs:label xml:lang="de">Objekt auf der Straße</rdfs:label>
    </owl:Class>
    


    <!-- http://purl.org/auto/criticality_phenomena#CP_213 -->

    <owl:Class rdf:about="http://purl.org/auto/criticality_phenomena#CP_213">
        <rdfs:subClassOf rdf:resource="http://purl.org/auto/criticality_phenomena#CP_278"/>
        <rdfs:subClassOf rdf:resource="http://purl.org/auto/criticality_phenomena#Perception_Criticality_Phenomenon"/>
        <rdfs:subClassOf rdf:resource="http://purl.org/auto/criticality_phenomena#Unpredictability_Criticality_Phenomenon"/>
        <dcterms:identifier rdf:datatype="http://www.w3.org/2001/XMLSchema#nonNegativeInteger">213</dcterms:identifier>
        <rdfs:comment xml:lang="en">There is an object near the road surface. This object might be a TP or anything other like e.g. a ball.</rdfs:comment>
        <rdfs:label xml:lang="en">Entity Near Road</rdfs:label>
        <rdfs:label xml:lang="de">Objekt nahe der Straße</rdfs:label>
    </owl:Class>
    


    <!-- http://purl.org/auto/criticality_phenomena#CP_214 -->

    <owl:Class rdf:about="http://purl.org/auto/criticality_phenomena#CP_214">
        <rdfs:subClassOf rdf:resource="http://purl.org/auto/criticality_phenomena#Behavioral_Criticality_Phenomenon"/>
        <rdfs:subClassOf rdf:resource="http://purl.org/auto/criticality_phenomena#CP_118"/>
        <dcterms:identifier rdf:datatype="http://www.w3.org/2001/XMLSchema#nonNegativeInteger">214</dcterms:identifier>
        <rdfs:comment xml:lang="en">An additional traffic sign can be set on a pickup truck. Its rules have to be followed.</rdfs:comment>
        <rdfs:label xml:lang="en">Additional traffic sign on pickup truck</rdfs:label>
        <rdfs:label xml:lang="de">Zusätzliches Verkehrszeichen auf Pickup</rdfs:label>
    </owl:Class>
    


    <!-- http://purl.org/auto/criticality_phenomena#CP_215 -->

    <owl:Class rdf:about="http://purl.org/auto/criticality_phenomena#CP_215">
        <rdfs:subClassOf rdf:resource="http://purl.org/auto/criticality_phenomena#CP_230"/>
        <dcterms:identifier rdf:datatype="http://www.w3.org/2001/XMLSchema#nonNegativeInteger">215</dcterms:identifier>
        <rdfs:comment xml:lang="en">Refers to specular and diffuse reflection or back-scattering of light by a material.</rdfs:comment>
        <rdfs:label xml:lang="de">Remission</rdfs:label>
        <rdfs:label xml:lang="en">Remission</rdfs:label>
    </owl:Class>
    


    <!-- http://purl.org/auto/criticality_phenomena#CP_216 -->

    <owl:Class rdf:about="http://purl.org/auto/criticality_phenomena#CP_216">
        <rdfs:subClassOf rdf:resource="http://purl.org/auto/criticality_phenomena#CP_284"/>
        <rdfs:subClassOf rdf:resource="http://purl.org/auto/criticality_phenomena#Dynamical_Criticality_Phenomenon"/>
        <rdfs:subClassOf rdf:resource="http://purl.org/auto/criticality_phenomena#Human_Criticality_Phenomenon"/>
        <rdfs:subClassOf rdf:resource="http://purl.org/auto/criticality_phenomena#Perception_Criticality_Phenomenon"/>
        <rdfs:subClassOf rdf:resource="http://purl.org/auto/criticality_phenomena#Spatial_Criticality_Phenomenon"/>
        <rdfs:subClassOf rdf:resource="http://purl.org/auto/criticality_phenomena#Temporal_Criticality_Phenomenon"/>
        <rdfs:subClassOf rdf:resource="http://purl.org/auto/criticality_phenomena#Unpredictability_Criticality_Phenomenon"/>
        <dcterms:identifier rdf:datatype="http://www.w3.org/2001/XMLSchema#nonNegativeInteger">216</dcterms:identifier>
        <rdfs:comment xml:lang="en">A TP performs a maneuver. This might be a e.g. a turn or a breaking maneuver</rdfs:comment>
        <rdfs:label xml:lang="en">Maneuver Of TP</rdfs:label>
        <rdfs:label xml:lang="de">Manöver eines TPs</rdfs:label>
    </owl:Class>
    


    <!-- http://purl.org/auto/criticality_phenomena#CP_217 -->

    <owl:Class rdf:about="http://purl.org/auto/criticality_phenomena#CP_217">
        <rdfs:subClassOf rdf:resource="http://purl.org/auto/criticality_phenomena#CP_194"/>
        <rdfs:subClassOf rdf:resource="http://purl.org/auto/criticality_phenomena#CP_212"/>
        <rdfs:subClassOf rdf:resource="http://purl.org/auto/criticality_phenomena#Real_Radar_Criticality_Phenomenon"/>
        <dcterms:identifier rdf:datatype="http://www.w3.org/2001/XMLSchema#nonNegativeInteger">217</dcterms:identifier>
        <rdfs:comment xml:lang="en">Metallic objects can reflect Radar waves and thus trigger FPs.</rdfs:comment>
        <rdfs:label xml:lang="de">Metallenes Objekt auf der Straße</rdfs:label>
        <rdfs:label xml:lang="en">Metallic Object On Road</rdfs:label>
    </owl:Class>
    


    <!-- http://purl.org/auto/criticality_phenomena#CP_218 -->

    <owl:Class rdf:about="http://purl.org/auto/criticality_phenomena#CP_218">
        <rdfs:subClassOf rdf:resource="http://purl.org/auto/criticality_phenomena#CP_217"/>
        <dcterms:identifier rdf:datatype="http://www.w3.org/2001/XMLSchema#nonNegativeInteger">218</dcterms:identifier>
        <rdfs:comment xml:lang="en">Highly reflective surface on the ground may be regarded as an obstacle by Radar sensor.</rdfs:comment>
        <rdfs:label xml:lang="de">Gullydeckel</rdfs:label>
        <rdfs:label xml:lang="en">Manhole Cover</rdfs:label>
    </owl:Class>
    


    <!-- http://purl.org/auto/criticality_phenomena#CP_219 -->

    <owl:Class rdf:about="http://purl.org/auto/criticality_phenomena#CP_219">
        <rdfs:subClassOf rdf:resource="http://purl.org/auto/criticality_phenomena#CP_197"/>
        <dcterms:identifier rdf:datatype="http://www.w3.org/2001/XMLSchema#nonNegativeInteger">219</dcterms:identifier>
        <rdfs:comment xml:lang="en">When multiple targets are located within one resolution cell, they appear as one (Holder et al.).</rdfs:comment>
        <rdfs:label xml:lang="en">Insufficient Separation Capability Of Radar</rdfs:label>
        <rdfs:label xml:lang="de">Unzureichende Trennschärfe von Radar</rdfs:label>
    </owl:Class>
    


    <!-- http://purl.org/auto/criticality_phenomena#CP_22 -->

    <owl:Class rdf:about="http://purl.org/auto/criticality_phenomena#CP_22">
        <rdfs:subClassOf rdf:resource="http://purl.org/auto/criticality_phenomena#CP_189"/>
        <rdfs:subClassOf rdf:resource="http://purl.org/auto/criticality_phenomena#Real_Lidar_Criticality_Phenomenon"/>
        <dcterms:identifier rdf:datatype="http://www.w3.org/2001/XMLSchema#nonNegativeInteger">22</dcterms:identifier>
        <rdfs:comment xml:lang="en">Presence of smoke where smoke is a collection of airborne particles and gases emitted when a material undergoes combustion or pyrolysis. E.g. smoke coming from a nearby burning car.</rdfs:comment>
        <rdfs:label xml:lang="de">Rauch</rdfs:label>
        <rdfs:label xml:lang="en">Smoke</rdfs:label>
    </owl:Class>
    


    <!-- http://purl.org/auto/criticality_phenomena#CP_220 -->

    <owl:Class rdf:about="http://purl.org/auto/criticality_phenomena#CP_220">
        <rdfs:subClassOf rdf:resource="http://purl.org/auto/criticality_phenomena#CP_195"/>
        <rdfs:subClassOf rdf:resource="http://purl.org/auto/criticality_phenomena#Real_Radar_Criticality_Phenomenon"/>
        <dcterms:identifier rdf:datatype="http://www.w3.org/2001/XMLSchema#nonNegativeInteger">220</dcterms:identifier>
        <rdfs:comment xml:lang="en">Objects with low radar cross section (depending again on volume, shape, material, ...) are invisible to RADAR sensor.</rdfs:comment>
        <rdfs:label xml:lang="en">Object With Low Radar Cross Section (rcs)</rdfs:label>
        <rdfs:label xml:lang="de">Objekt mit niedrigem Radarquerschnitt</rdfs:label>
    </owl:Class>
    


    <!-- http://purl.org/auto/criticality_phenomena#CP_221 -->

    <owl:Class rdf:about="http://purl.org/auto/criticality_phenomena#CP_221">
        <rdfs:subClassOf rdf:resource="http://purl.org/auto/criticality_phenomena#CP_195"/>
        <rdfs:subClassOf rdf:resource="http://purl.org/auto/criticality_phenomena#Perfect_Camera_Criticality_Phenomenon"/>
        <rdfs:subClassOf rdf:resource="http://purl.org/auto/criticality_phenomena#Perfect_Lidar_Criticality_Phenomenon"/>
        <rdfs:subClassOf rdf:resource="http://purl.org/auto/criticality_phenomena#Perfect_Radar_Criticality_Phenomenon"/>
        <dcterms:identifier rdf:datatype="http://www.w3.org/2001/XMLSchema#nonNegativeInteger">221</dcterms:identifier>
        <rdfs:comment xml:lang="en">Objects out of the recognition area of sensor may not be recognized by the sensor.</rdfs:comment>
        <rdfs:label xml:lang="en">Object Out Of Recognition Area Of Sensor</rdfs:label>
        <rdfs:label xml:lang="de">Objekt außerhalb des Erkennungsbereich des Sensors</rdfs:label>
    </owl:Class>
    


    <!-- http://purl.org/auto/criticality_phenomena#CP_222 -->

    <owl:Class rdf:about="http://purl.org/auto/criticality_phenomena#CP_222">
        <rdfs:subClassOf rdf:resource="http://purl.org/auto/criticality_phenomena#CP_221"/>
        <dcterms:identifier rdf:datatype="http://www.w3.org/2001/XMLSchema#nonNegativeInteger">222</dcterms:identifier>
        <rdfs:comment xml:lang="en">Objects out of the field of view may not be recognized by the sensor.</rdfs:comment>
        <rdfs:label xml:lang="en">Object Out Of Field Of View</rdfs:label>
        <rdfs:label xml:lang="de">Objekt außerhalb des Sichtfelds (Winkel horizontal &amp; vertikal)</rdfs:label>
    </owl:Class>
    


    <!-- http://purl.org/auto/criticality_phenomena#CP_223 -->

    <owl:Class rdf:about="http://purl.org/auto/criticality_phenomena#CP_223">
        <rdfs:subClassOf rdf:resource="http://purl.org/auto/criticality_phenomena#CP_195"/>
        <rdfs:subClassOf rdf:resource="http://purl.org/auto/criticality_phenomena#Perfect_Camera_Criticality_Phenomenon"/>
        <rdfs:subClassOf rdf:resource="http://purl.org/auto/criticality_phenomena#Perfect_Lidar_Criticality_Phenomenon"/>
        <rdfs:subClassOf rdf:resource="http://purl.org/auto/criticality_phenomena#Perfect_Radar_Criticality_Phenomenon"/>
        <rdfs:subClassOf rdf:resource="http://purl.org/auto/criticality_phenomena#Real_Human_Criticality_Phenomenon"/>
        <dcterms:identifier rdf:datatype="http://www.w3.org/2001/XMLSchema#nonNegativeInteger">223</dcterms:identifier>
        <rdfs:comment xml:lang="en">Objects with high transmission or absorption may not be recognized by the sensor</rdfs:comment>
        <rdfs:label xml:lang="en">Object With High Transmission Or Absorption Regarding Electromagnetic Wave Spectrum Of Sensor</rdfs:label>
        <rdfs:label xml:lang="de">Objekt mit hoher Transmission oder Absorption im elektromagnetischen Spektrum des entsprechenden Sensors</rdfs:label>
    </owl:Class>
    


    <!-- http://purl.org/auto/criticality_phenomena#CP_224 -->

    <owl:Class rdf:about="http://purl.org/auto/criticality_phenomena#CP_224">
        <rdfs:subClassOf rdf:resource="http://purl.org/auto/criticality_phenomena#CP_221"/>
        <rdfs:subClassOf rdf:resource="http://purl.org/auto/criticality_phenomena#Real_Camera_Criticality_Phenomenon"/>
        <rdfs:subClassOf rdf:resource="http://purl.org/auto/criticality_phenomena#Real_Lidar_Criticality_Phenomenon"/>
        <rdfs:subClassOf rdf:resource="http://purl.org/auto/criticality_phenomena#Real_Radar_Criticality_Phenomenon"/>
        <dcterms:identifier rdf:datatype="http://www.w3.org/2001/XMLSchema#nonNegativeInteger">224</dcterms:identifier>
        <rdfs:comment xml:lang="en">Objects out of the range may not be recognized by the sensor.</rdfs:comment>
        <rdfs:label xml:lang="en">Object Out Of Sensor Range</rdfs:label>
        <rdfs:label xml:lang="de">Objekt außerhalb der Reichweite des Sensors</rdfs:label>
    </owl:Class>
    


    <!-- http://purl.org/auto/criticality_phenomena#CP_225 -->

    <owl:Class rdf:about="http://purl.org/auto/criticality_phenomena#CP_225">
        <rdfs:subClassOf rdf:resource="http://purl.org/auto/criticality_phenomena#CP_197"/>
        <rdfs:subClassOf rdf:resource="http://purl.org/auto/criticality_phenomena#Perfect_Camera_Criticality_Phenomenon"/>
        <dcterms:identifier rdf:datatype="http://www.w3.org/2001/XMLSchema#nonNegativeInteger">225</dcterms:identifier>
        <rdfs:comment xml:lang="en">Objects out of the plane of focus of the camera may appear blurred.</rdfs:comment>
        <rdfs:label xml:lang="en">Object Out Of Plane Of Focus Of Camera</rdfs:label>
        <rdfs:label xml:lang="de">Objekt außerhalb der Schärfeebene der Kamera</rdfs:label>
    </owl:Class>
    


    <!-- http://purl.org/auto/criticality_phenomena#CP_226 -->

    <owl:Class rdf:about="http://purl.org/auto/criticality_phenomena#CP_226">
        <rdfs:subClassOf rdf:resource="http://purl.org/auto/criticality_phenomena#CP_195"/>
        <rdfs:subClassOf rdf:resource="http://purl.org/auto/criticality_phenomena#Perfect_Camera_Criticality_Phenomenon"/>
        <rdfs:subClassOf rdf:resource="http://purl.org/auto/criticality_phenomena#Perfect_Human_Criticality_Phenomenon"/>
        <rdfs:subClassOf rdf:resource="http://purl.org/auto/criticality_phenomena#Perfect_Lidar_Criticality_Phenomenon"/>
        <rdfs:subClassOf rdf:resource="http://purl.org/auto/criticality_phenomena#Perfect_Radar_Criticality_Phenomenon"/>
        <dcterms:identifier rdf:datatype="http://www.w3.org/2001/XMLSchema#nonNegativeInteger">226</dcterms:identifier>
        <rdfs:comment xml:lang="en">Existence of highly reflective or absorptive object between relevant object and sensor.</rdfs:comment>
        <rdfs:label xml:lang="en">Blockage Of Relevant Electromagnetic Waves For Sensor By Another Object</rdfs:label>
        <rdfs:label xml:lang="de">Blockierung von relevanten elektromagnetischen Wellen für Sensor durch ein weiteres Objekt</rdfs:label>
    </owl:Class>
    


    <!-- http://purl.org/auto/criticality_phenomena#CP_227 -->

    <owl:Class rdf:about="http://purl.org/auto/criticality_phenomena#CP_227">
        <rdfs:subClassOf rdf:resource="http://purl.org/auto/criticality_phenomena#CP_223"/>
        <dcterms:identifier rdf:datatype="http://www.w3.org/2001/XMLSchema#nonNegativeInteger">227</dcterms:identifier>
        <rdfs:comment xml:lang="en">Objects with high transparency may not be recognized by camera or LIDAR</rdfs:comment>
        <rdfs:label xml:lang="en">Object With High Transmission Or Absorption In Optical Spectrum</rdfs:label>
        <rdfs:label xml:lang="de">Objekt mit hoher Transparenz</rdfs:label>
    </owl:Class>
    


    <!-- http://purl.org/auto/criticality_phenomena#CP_228 -->

    <owl:Class rdf:about="http://purl.org/auto/criticality_phenomena#CP_228">
        <rdfs:subClassOf rdf:resource="http://purl.org/auto/criticality_phenomena#CP_227"/>
        <rdfs:subClassOf rdf:resource="http://purl.org/auto/criticality_phenomena#Real_Human_Criticality_Phenomenon"/>
        <dcterms:identifier rdf:datatype="http://www.w3.org/2001/XMLSchema#nonNegativeInteger">228</dcterms:identifier>
        <rdfs:comment xml:lang="en">Glas may not be recognized by sensors.</rdfs:comment>
        <rdfs:label xml:lang="en">Glas Objects</rdfs:label>
        <rdfs:label xml:lang="de">Glasobjekte</rdfs:label>
    </owl:Class>
    


    <!-- http://purl.org/auto/criticality_phenomena#CP_229 -->

    <owl:Class rdf:about="http://purl.org/auto/criticality_phenomena#CP_229">
        <rdfs:subClassOf rdf:resource="http://purl.org/auto/criticality_phenomena#CP_226"/>
        <rdfs:subClassOf rdf:resource="http://purl.org/auto/criticality_phenomena#Real_Camera_Criticality_Phenomenon"/>
        <rdfs:subClassOf rdf:resource="http://purl.org/auto/criticality_phenomena#Real_Lidar_Criticality_Phenomenon"/>
        <rdfs:subClassOf rdf:resource="http://purl.org/auto/criticality_phenomena#Real_Radar_Criticality_Phenomenon"/>
        <dcterms:identifier rdf:datatype="http://www.w3.org/2001/XMLSchema#nonNegativeInteger">229</dcterms:identifier>
        <rdfs:comment xml:lang="en">Layers on sensor cover such as: dirt, snow, ice, water, salt, ...</rdfs:comment>
        <rdfs:label xml:lang="en">Layer On Sensor Cover Or Lens</rdfs:label>
        <rdfs:label xml:lang="de">Schicht auf der Sensorabdeckung oder -linse</rdfs:label>
    </owl:Class>
    


    <!-- http://purl.org/auto/criticality_phenomena#CP_23 -->

    <owl:Class rdf:about="http://purl.org/auto/criticality_phenomena#CP_23">
        <rdfs:subClassOf rdf:resource="http://purl.org/auto/criticality_phenomena#CP_195"/>
        <rdfs:subClassOf rdf:resource="http://purl.org/auto/criticality_phenomena#Spatial_Criticality_Phenomenon"/>
        <dcterms:identifier rdf:datatype="http://www.w3.org/2001/XMLSchema#nonNegativeInteger">23</dcterms:identifier>
        <rdfs:comment xml:lang="en">Loss/restriction of planning ability due to potential disconnect from e.g. digital maps.</rdfs:comment>
        <rdfs:label xml:lang="en">Dead Spot</rdfs:label>
        <rdfs:label xml:lang="de">Funkloch</rdfs:label>
    </owl:Class>
    


    <!-- http://purl.org/auto/criticality_phenomena#CP_230 -->

    <owl:Class rdf:about="http://purl.org/auto/criticality_phenomena#CP_230">
        <rdfs:subClassOf rdf:resource="http://purl.org/auto/criticality_phenomena#CP_197"/>
        <rdfs:subClassOf rdf:resource="http://purl.org/auto/criticality_phenomena#Perfect_Camera_Criticality_Phenomenon"/>
        <rdfs:subClassOf rdf:resource="http://purl.org/auto/criticality_phenomena#Perfect_Lidar_Criticality_Phenomenon"/>
        <rdfs:subClassOf rdf:resource="http://purl.org/auto/criticality_phenomena#Perfect_Radar_Criticality_Phenomenon"/>
        <dcterms:identifier rdf:datatype="http://www.w3.org/2001/XMLSchema#nonNegativeInteger">230</dcterms:identifier>
        <rdfs:comment xml:lang="en">Deviation of electromagnetic waves from their straight trajectory.</rdfs:comment>
        <rdfs:label xml:lang="en">Scattering</rdfs:label>
        <rdfs:label xml:lang="de">Streuung</rdfs:label>
    </owl:Class>
    


    <!-- http://purl.org/auto/criticality_phenomena#CP_231 -->

    <owl:Class rdf:about="http://purl.org/auto/criticality_phenomena#CP_231">
        <rdfs:subClassOf rdf:resource="http://purl.org/auto/criticality_phenomena#CP_197"/>
        <dcterms:identifier rdf:datatype="http://www.w3.org/2001/XMLSchema#nonNegativeInteger">231</dcterms:identifier>
        <rdfs:comment xml:lang="en">Sensor may vibrate leading to high measurement errors if sensitive hardware (e.g. mirrors, lenses) are used.</rdfs:comment>
        <rdfs:label xml:lang="de">Vibrationen des Sensors</rdfs:label>
        <rdfs:label xml:lang="en">Vibrations Of The Sensor</rdfs:label>
    </owl:Class>
    


    <!-- http://purl.org/auto/criticality_phenomena#CP_232 -->

    <owl:Class rdf:about="http://purl.org/auto/criticality_phenomena#CP_232">
        <rdfs:subClassOf rdf:resource="http://purl.org/auto/criticality_phenomena#CP_208"/>
        <dcterms:identifier rdf:datatype="http://www.w3.org/2001/XMLSchema#nonNegativeInteger">232</dcterms:identifier>
        <rdfs:comment xml:lang="en">May lead to reduced controllability, but also affects sensor vibrations.</rdfs:comment>
        <rdfs:label xml:lang="en">Rough Road Surface</rdfs:label>
        <rdfs:label xml:lang="de">Unebene Straßenoberfläche</rdfs:label>
    </owl:Class>
    


    <!-- http://purl.org/auto/criticality_phenomena#CP_233 -->

    <owl:Class rdf:about="http://purl.org/auto/criticality_phenomena#CP_233">
        <rdfs:subClassOf rdf:resource="http://purl.org/auto/criticality_phenomena#CP_197"/>
        <dcterms:identifier rdf:datatype="http://www.w3.org/2001/XMLSchema#nonNegativeInteger">233</dcterms:identifier>
        <rdfs:comment xml:lang="en">Moving objects can be (motion) blurred due to high relative speeds, esp. for slow shutter speeds.</rdfs:comment>
        <rdfs:label xml:lang="en">Moving Objects W.r.t Relative Speed</rdfs:label>
        <rdfs:label xml:lang="de">Sich bewegende Objekte in Bezug auf die Relativgeschwindigkeit</rdfs:label>
    </owl:Class>
    


    <!-- http://purl.org/auto/criticality_phenomena#CP_234 -->

    <owl:Class rdf:about="http://purl.org/auto/criticality_phenomena#CP_234">
        <rdfs:subClassOf rdf:resource="http://purl.org/auto/criticality_phenomena#CP_197"/>
        <rdfs:subClassOf rdf:resource="http://purl.org/auto/criticality_phenomena#Perfect_Camera_Criticality_Phenomenon"/>
        <rdfs:subClassOf rdf:resource="http://purl.org/auto/criticality_phenomena#Perfect_Lidar_Criticality_Phenomenon"/>
        <rdfs:subClassOf rdf:resource="http://purl.org/auto/criticality_phenomena#Perfect_Radar_Criticality_Phenomenon"/>
        <dcterms:identifier rdf:datatype="http://www.w3.org/2001/XMLSchema#nonNegativeInteger">234</dcterms:identifier>
        <rdfs:comment xml:lang="en">Electromagnetic interference (EMI) is a disturbance generated by an external source that affects an electrical circuit by electromagnetic induction, electrostatic coupling, or conduction. The disturbance may degrade the performance of the circuit or even stop it from functioning. In the case of a data path, these effects can range from an increase in error rate to a total loss of the data. May be caused by some entity like other active sensors, lasr pointers, ...</rdfs:comment>
        <rdfs:label xml:lang="en">Electromagnetic Interference</rdfs:label>
        <rdfs:label xml:lang="de">Elektromagnetische Interferenz</rdfs:label>
    </owl:Class>
    


    <!-- http://purl.org/auto/criticality_phenomena#CP_235 -->

    <owl:Class rdf:about="http://purl.org/auto/criticality_phenomena#CP_235">
        <rdfs:subClassOf rdf:resource="http://purl.org/auto/criticality_phenomena#CP_234"/>
        <dcterms:identifier rdf:datatype="http://www.w3.org/2001/XMLSchema#nonNegativeInteger">235</dcterms:identifier>
        <rdfs:comment xml:lang="en">Intereference between electromagnetic waves of sensors of ego and other vehicles.</rdfs:comment>
        <rdfs:label xml:lang="en">Sensor Crosstalk</rdfs:label>
        <rdfs:label xml:lang="de">Sensorüberlagerung</rdfs:label>
    </owl:Class>
    


    <!-- http://purl.org/auto/criticality_phenomena#CP_236 -->

    <owl:Class rdf:about="http://purl.org/auto/criticality_phenomena#CP_236">
        <rdfs:subClassOf rdf:resource="http://purl.org/auto/criticality_phenomena#CP_230"/>
        <dcterms:identifier rdf:datatype="http://www.w3.org/2001/XMLSchema#nonNegativeInteger">236</dcterms:identifier>
        <rdfs:comment xml:lang="en">Particles in air (e.g. fog, snow, rain, dust,...) may lead to backscattering which may lead to low signal to noise ratio and false positives.</rdfs:comment>
        <rdfs:label xml:lang="en">Backscattering Of Electromagnetic Waves</rdfs:label>
        <rdfs:label xml:lang="de">Rückstreuung von elektromagnetischer Strahlung</rdfs:label>
    </owl:Class>
    


    <!-- http://purl.org/auto/criticality_phenomena#CP_237 -->

    <owl:Class rdf:about="http://purl.org/auto/criticality_phenomena#CP_237">
        <rdfs:subClassOf rdf:resource="http://purl.org/auto/criticality_phenomena#CP_234"/>
        <rdfs:subClassOf rdf:resource="http://purl.org/auto/criticality_phenomena#Real_Lidar_Criticality_Phenomenon"/>
        <dcterms:identifier rdf:datatype="http://www.w3.org/2001/XMLSchema#nonNegativeInteger">237</dcterms:identifier>
        <rdfs:comment xml:lang="en">Photosensor of camera or LIDAR is disturbed by light directed at it (e.g. laser pointer).</rdfs:comment>
        <rdfs:label xml:lang="de">Lichtstörung</rdfs:label>
        <rdfs:label xml:lang="en">Light Disturbance</rdfs:label>
    </owl:Class>
    


    <!-- http://purl.org/auto/criticality_phenomena#CP_238 -->

    <owl:Class rdf:about="http://purl.org/auto/criticality_phenomena#CP_238">
        <rdfs:subClassOf rdf:resource="http://purl.org/auto/criticality_phenomena#CP_230"/>
        <dcterms:identifier rdf:datatype="http://www.w3.org/2001/XMLSchema#nonNegativeInteger">238</dcterms:identifier>
        <rdfs:comment xml:lang="en">Optical distortion might affect the capability to detect entities correctly.</rdfs:comment>
        <rdfs:label xml:lang="en">Optical Distortion Of Objects</rdfs:label>
        <rdfs:label xml:lang="de">Optische Verzerrung von Objekten</rdfs:label>
    </owl:Class>
    


    <!-- http://purl.org/auto/criticality_phenomena#CP_239 -->

    <owl:Class rdf:about="http://purl.org/auto/criticality_phenomena#CP_239">
        <rdfs:subClassOf rdf:resource="http://purl.org/auto/criticality_phenomena#CP_198"/>
        <dcterms:identifier rdf:datatype="http://www.w3.org/2001/XMLSchema#nonNegativeInteger">239</dcterms:identifier>
        <rdfs:comment xml:lang="en">Extraordinary clothes may not be recognized by a perception algorithm depending on the employed training data.</rdfs:comment>
        <rdfs:label xml:lang="de">Außergewöhnlich gekleidete Personen in Straßennähe</rdfs:label>
        <rdfs:label xml:lang="en">Extraordinarily Dressed Persons Near Road</rdfs:label>
    </owl:Class>
    


    <!-- http://purl.org/auto/criticality_phenomena#CP_24 -->

    <owl:Class rdf:about="http://purl.org/auto/criticality_phenomena#CP_24">
        <rdfs:subClassOf rdf:resource="http://purl.org/auto/criticality_phenomena#CP_212"/>
        <rdfs:subClassOf rdf:resource="http://purl.org/auto/criticality_phenomena#Complexity_Criticality_Phenomenon"/>
        <rdfs:subClassOf rdf:resource="http://purl.org/auto/criticality_phenomena#Human_Criticality_Phenomenon"/>
        <rdfs:subClassOf rdf:resource="http://purl.org/auto/criticality_phenomena#Perfect_Perception_Criticality_Phenomenon"/>
        <rdfs:subClassOf rdf:resource="http://purl.org/auto/criticality_phenomena#Unpredictability_Criticality_Phenomenon"/>
        <dcterms:identifier rdf:datatype="http://www.w3.org/2001/XMLSchema#nonNegativeInteger">24</dcterms:identifier>
        <rdfs:comment xml:lang="en">An accident has happened on the road.</rdfs:comment>
        <rdfs:label xml:lang="en">Accident Site</rdfs:label>
        <rdfs:label xml:lang="de">Unfallstelle</rdfs:label>
    </owl:Class>
    


    <!-- http://purl.org/auto/criticality_phenomena#CP_240 -->

    <owl:Class rdf:about="http://purl.org/auto/criticality_phenomena#CP_240">
        <rdfs:subClassOf rdf:resource="http://purl.org/auto/criticality_phenomena#CP_239"/>
        <rdfs:subClassOf rdf:resource="http://purl.org/auto/criticality_phenomena#Complexity_Criticality_Phenomenon"/>
        <dcterms:identifier rdf:datatype="http://www.w3.org/2001/XMLSchema#nonNegativeInteger">240</dcterms:identifier>
        <rdfs:comment xml:lang="en">Carnival implies persons may dress up, which may lead to misclassification of humans.</rdfs:comment>
        <rdfs:label xml:lang="en">Carnival</rdfs:label>
        <rdfs:label xml:lang="de">Karneval</rdfs:label>
    </owl:Class>
    


    <!-- http://purl.org/auto/criticality_phenomena#CP_241 -->

    <owl:Class rdf:about="http://purl.org/auto/criticality_phenomena#CP_241">
        <rdfs:subClassOf rdf:resource="http://purl.org/auto/criticality_phenomena#CP_238"/>
        <rdfs:subClassOf rdf:resource="http://purl.org/auto/criticality_phenomena#Real_Camera_Criticality_Phenomenon"/>
        <dcterms:identifier rdf:datatype="http://www.w3.org/2001/XMLSchema#nonNegativeInteger">241</dcterms:identifier>
        <rdfs:comment xml:lang="en">E.g. wide angle lenses</rdfs:comment>
        <rdfs:label xml:lang="en">Optical Distortion Of Objects Due To Optical Properties Of Sensor</rdfs:label>
        <rdfs:label xml:lang="de">Optische Verzerrung von Objekten durch Eigenschaften des Sensors</rdfs:label>
    </owl:Class>
    


    <!-- http://purl.org/auto/criticality_phenomena#CP_242 -->

    <owl:Class rdf:about="http://purl.org/auto/criticality_phenomena#CP_242">
        <rdfs:subClassOf rdf:resource="http://purl.org/auto/criticality_phenomena#CP_238"/>
        <dcterms:identifier rdf:datatype="http://www.w3.org/2001/XMLSchema#nonNegativeInteger">242</dcterms:identifier>
        <rdfs:comment xml:lang="en">E.g. rain</rdfs:comment>
        <rdfs:label xml:lang="en">Optical Distortion Of Objects Due To Environmental Factors</rdfs:label>
        <rdfs:label xml:lang="de">Optische Verzerrung von Objekten durch Umweltfaktoren</rdfs:label>
    </owl:Class>
    


    <!-- http://purl.org/auto/criticality_phenomena#CP_243 -->

    <owl:Class rdf:about="http://purl.org/auto/criticality_phenomena#CP_243">
        <rdfs:subClassOf rdf:resource="http://purl.org/auto/criticality_phenomena#CP_197"/>
        <rdfs:subClassOf rdf:resource="http://purl.org/auto/criticality_phenomena#CP_198"/>
        <dcterms:identifier rdf:datatype="http://www.w3.org/2001/XMLSchema#nonNegativeInteger">243</dcterms:identifier>
        <rdfs:comment xml:lang="en">Objects without an ontological equivalent can not be &apos;understood&apos; by the perception algorithm and may be labeled falsely or too abstractly.</rdfs:comment>
        <rdfs:label xml:lang="en">Object Without Ontological Representation In Scene</rdfs:label>
        <rdfs:label xml:lang="de">Objekt ohne ontologische Darstelling in Szene</rdfs:label>
    </owl:Class>
    


    <!-- http://purl.org/auto/criticality_phenomena#CP_244 -->

    <owl:Class rdf:about="http://purl.org/auto/criticality_phenomena#CP_244">
        <rdfs:subClassOf rdf:resource="http://purl.org/auto/criticality_phenomena#CP_198"/>
        <dcterms:identifier rdf:datatype="http://www.w3.org/2001/XMLSchema#nonNegativeInteger">244</dcterms:identifier>
        <rdfs:comment xml:lang="en">Wrong perceived height due to small vertical opening angle of Radar may lead to erroneous decisions.</rdfs:comment>
        <rdfs:label xml:lang="de">Falsche Höhenklassifizierung von bauliche Strukturen über der Straße</rdfs:label>
        <rdfs:label xml:lang="en">Wrong Height Classification Of Overhead Structure</rdfs:label>
    </owl:Class>
    


    <!-- http://purl.org/auto/criticality_phenomena#CP_245 -->

    <owl:Class rdf:about="http://purl.org/auto/criticality_phenomena#CP_245">
        <rdfs:subClassOf rdf:resource="http://purl.org/auto/criticality_phenomena#CP_286"/>
        <rdfs:subClassOf rdf:resource="http://purl.org/auto/criticality_phenomena#Real_Radar_Criticality_Phenomenon"/>
        <dcterms:identifier rdf:datatype="http://www.w3.org/2001/XMLSchema#nonNegativeInteger">245</dcterms:identifier>
        <rdfs:comment xml:lang="en">Overhead structures (esp. with metal) may reflect radar waves such that ghost objects are recognized by a radar.</rdfs:comment>
        <rdfs:label xml:lang="de">Bauliche Strukturen über der Straße</rdfs:label>
        <rdfs:label xml:lang="en">Presence Of Overhead Structures</rdfs:label>
    </owl:Class>
    


    <!-- http://purl.org/auto/criticality_phenomena#CP_246 -->

    <owl:Class rdf:about="http://purl.org/auto/criticality_phenomena#CP_246">
        <rdfs:subClassOf rdf:resource="http://purl.org/auto/criticality_phenomena#CP_198"/>
        <dcterms:identifier rdf:datatype="http://www.w3.org/2001/XMLSchema#nonNegativeInteger">246</dcterms:identifier>
        <rdfs:comment xml:lang="en">Interleaving of sampling rates with signal frequencies of emitting objects in scene (e.g. traffic lights) may lead to not identifying the correct state indicated by the signal.</rdfs:comment>
        <rdfs:label xml:lang="de">Abtastrateneffekt präsent</rdfs:label>
        <rdfs:label xml:lang="en">Sampling Rate Effect Present</rdfs:label>
    </owl:Class>
    


    <!-- http://purl.org/auto/criticality_phenomena#CP_247 -->

    <owl:Class rdf:about="http://purl.org/auto/criticality_phenomena#CP_247">
        <rdfs:subClassOf rdf:resource="http://purl.org/auto/criticality_phenomena#CP_175"/>
        <rdfs:subClassOf rdf:resource="http://purl.org/auto/criticality_phenomena#CP_245"/>
        <dcterms:identifier rdf:datatype="http://www.w3.org/2001/XMLSchema#nonNegativeInteger">247</dcterms:identifier>
        <rdfs:comment xml:lang="en">Ego is driving below a bridge. This might amplify sensor phenomenons.</rdfs:comment>
        <rdfs:label xml:lang="en">Driving Below Bridge</rdfs:label>
        <rdfs:label xml:lang="de">Unter einer Brücke hindurch fahren</rdfs:label>
    </owl:Class>
    


    <!-- http://purl.org/auto/criticality_phenomena#CP_248 -->

    <owl:Class rdf:about="http://purl.org/auto/criticality_phenomena#CP_248">
        <rdfs:subClassOf rdf:resource="http://purl.org/auto/criticality_phenomena#CP_194"/>
        <rdfs:subClassOf rdf:resource="http://purl.org/auto/criticality_phenomena#CP_198"/>
        <rdfs:subClassOf rdf:resource="http://purl.org/auto/criticality_phenomena#Perfect_Camera_Criticality_Phenomenon"/>
        <rdfs:subClassOf rdf:resource="http://purl.org/auto/criticality_phenomena#Perfect_Radar_Criticality_Phenomenon"/>
        <dcterms:identifier rdf:datatype="http://www.w3.org/2001/XMLSchema#nonNegativeInteger">248</dcterms:identifier>
        <rdfs:comment xml:lang="en">Electromagnetic waves may reach the sensor by more than one path leading to spurious signals.</rdfs:comment>
        <rdfs:label xml:lang="de">Mehrwegeempfang</rdfs:label>
        <rdfs:label xml:lang="en">Multipath Propagation</rdfs:label>
    </owl:Class>
    


    <!-- http://purl.org/auto/criticality_phenomena#CP_249 -->

    <owl:Class rdf:about="http://purl.org/auto/criticality_phenomena#CP_249">
        <rdfs:subClassOf rdf:resource="http://purl.org/auto/criticality_phenomena#CP_175"/>
        <dcterms:identifier rdf:datatype="http://www.w3.org/2001/XMLSchema#nonNegativeInteger">249</dcterms:identifier>
        <rdfs:comment xml:lang="en">Driving on a bridge might amplify phenomenons like external force.</rdfs:comment>
        <rdfs:label xml:lang="en">Driving On Bridge</rdfs:label>
        <rdfs:label xml:lang="de">Fahren auf einer Brücke</rdfs:label>
    </owl:Class>
    


    <!-- http://purl.org/auto/criticality_phenomena#CP_25 -->

    <owl:Class rdf:about="http://purl.org/auto/criticality_phenomena#CP_25">
        <rdfs:subClassOf rdf:resource="http://purl.org/auto/criticality_phenomena#CP_226"/>
        <rdfs:subClassOf rdf:resource="http://purl.org/auto/criticality_phenomena#Spatial_Criticality_Phenomenon"/>
        <formalized rdf:datatype="http://www.w3.org/2001/XMLSchema#boolean">true</formalized>
        <dcterms:identifier rdf:datatype="http://www.w3.org/2001/XMLSchema#nonNegativeInteger">25</dcterms:identifier>
        <rdfs:comment xml:lang="en">For a perceiving TP, occlusion is the visual obstruction of some entity through some opaque object such that the obstructed entity can not or only partially be perceived by the TP.</rdfs:comment>
        <rdfs:label xml:lang="en">Occlusion</rdfs:label>
        <rdfs:label xml:lang="de">Sichtverdeckung</rdfs:label>
    </owl:Class>
    


    <!-- http://purl.org/auto/criticality_phenomena#CP_250 -->

    <owl:Class rdf:about="http://purl.org/auto/criticality_phenomena#CP_250">
        <rdfs:subClassOf rdf:resource="http://purl.org/auto/criticality_phenomena#CP_286"/>
        <rdfs:subClassOf rdf:resource="http://purl.org/auto/criticality_phenomena#Perfect_Camera_Criticality_Phenomenon"/>
        <rdfs:subClassOf rdf:resource="http://purl.org/auto/criticality_phenomena#Perfect_Lidar_Criticality_Phenomenon"/>
        <rdfs:subClassOf rdf:resource="http://purl.org/auto/criticality_phenomena#Perfect_Radar_Criticality_Phenomenon"/>
        <dcterms:identifier rdf:datatype="http://www.w3.org/2001/XMLSchema#nonNegativeInteger">250</dcterms:identifier>
        <rdfs:comment xml:lang="en">Roadside structures (especially metal) may lead to multipath propagation.</rdfs:comment>
        <rdfs:label xml:lang="de">Anwesenheit von Straßenbebauung</rdfs:label>
        <rdfs:label xml:lang="en">Presence Of Roadside Structures</rdfs:label>
    </owl:Class>
    


    <!-- http://purl.org/auto/criticality_phenomena#CP_251 -->

    <owl:Class rdf:about="http://purl.org/auto/criticality_phenomena#CP_251">
        <rdfs:subClassOf rdf:resource="http://purl.org/auto/criticality_phenomena#CP_116"/>
        <rdfs:subClassOf rdf:resource="http://purl.org/auto/criticality_phenomena#Real_Camera_Criticality_Phenomenon"/>
        <rdfs:subClassOf rdf:resource="http://purl.org/auto/criticality_phenomena#Real_Lidar_Criticality_Phenomenon"/>
        <rdfs:subClassOf rdf:resource="http://purl.org/auto/criticality_phenomena#Real_Radar_Criticality_Phenomenon"/>
        <dcterms:identifier rdf:datatype="http://www.w3.org/2001/XMLSchema#nonNegativeInteger">251</dcterms:identifier>
        <rdfs:comment xml:lang="en">The sensor cover may be damaged, includes the plastic, metal, glass etc. surfaces containing all sensor technologies.</rdfs:comment>
        <rdfs:label xml:lang="en">Mechanical Defect Of Sensor Cover</rdfs:label>
        <rdfs:label xml:lang="de">Mechanischer Defekt der Sensorabdeckung oder -linse</rdfs:label>
    </owl:Class>
    


    <!-- http://purl.org/auto/criticality_phenomena#CP_252 -->

    <owl:Class rdf:about="http://purl.org/auto/criticality_phenomena#CP_252">
        <rdfs:subClassOf rdf:resource="http://purl.org/auto/criticality_phenomena#CP_251"/>
        <dcterms:identifier rdf:datatype="http://www.w3.org/2001/XMLSchema#nonNegativeInteger">252</dcterms:identifier>
        <rdfs:comment xml:lang="en">e.g. lens is missing.</rdfs:comment>
        <rdfs:label xml:lang="de">Fehlende Sensorabdeckung</rdfs:label>
        <rdfs:label xml:lang="en">Missing Sensor Cover</rdfs:label>
    </owl:Class>
    


    <!-- http://purl.org/auto/criticality_phenomena#CP_253 -->

    <owl:Class rdf:about="http://purl.org/auto/criticality_phenomena#CP_253">
        <rdfs:subClassOf rdf:resource="http://purl.org/auto/criticality_phenomena#CP_251"/>
        <dcterms:identifier rdf:datatype="http://www.w3.org/2001/XMLSchema#nonNegativeInteger">253</dcterms:identifier>
        <rdfs:comment xml:lang="en">e.g. scratch, hole, crack in cover or deformation of whole cover due to high temperatures.</rdfs:comment>
        <rdfs:label xml:lang="de">Beschädigte Sensorabdeckung</rdfs:label>
        <rdfs:label xml:lang="en">Damaged Sensor Cover</rdfs:label>
    </owl:Class>
    


    <!-- http://purl.org/auto/criticality_phenomena#CP_254 -->

    <owl:Class rdf:about="http://purl.org/auto/criticality_phenomena#CP_254">
        <rdfs:subClassOf rdf:resource="http://purl.org/auto/criticality_phenomena#CP_204"/>
        <dcterms:identifier rdf:datatype="http://www.w3.org/2001/XMLSchema#nonNegativeInteger">254</dcterms:identifier>
        <rdfs:comment xml:lang="en">Unremoved ice sheets on truck roofs may fall down and cause severe accidents, as they usually hit the road 20-50m behind the truck.</rdfs:comment>
        <rdfs:label xml:lang="de">Eisplatten auf LKW Dach</rdfs:label>
        <rdfs:label xml:lang="en">Ice Sheets On Truck Roof</rdfs:label>
    </owl:Class>
    


    <!-- http://purl.org/auto/criticality_phenomena#CP_255 -->

    <owl:Class rdf:about="http://purl.org/auto/criticality_phenomena#CP_255">
        <rdfs:subClassOf rdf:resource="http://purl.org/auto/criticality_phenomena#Criticality_Phenomenon"/>
        <dcterms:identifier rdf:datatype="http://www.w3.org/2001/XMLSchema#nonNegativeInteger">255</dcterms:identifier>
        <rdfs:comment xml:lang="en">Special vehicles like police cars etc. show special behaviour which must be responded to.</rdfs:comment>
        <rdfs:label xml:lang="en">Behaviour of special TP</rdfs:label>
        <rdfs:label xml:lang="de">Verhalten Spezieller TP</rdfs:label>
    </owl:Class>
    


    <!-- http://purl.org/auto/criticality_phenomena#CP_256 -->

    <owl:Class rdf:about="http://purl.org/auto/criticality_phenomena#CP_256">
        <rdfs:subClassOf rdf:resource="http://purl.org/auto/criticality_phenomena#CP_210"/>
        <dcterms:identifier rdf:datatype="http://www.w3.org/2001/XMLSchema#nonNegativeInteger">256</dcterms:identifier>
        <rdfs:comment xml:lang="en">Wikipedia: In many cases temporal light modulationss may cause unacceptable annoying effects such as flicker or stroboscopic effect that can directly be perceived by humans. These effects are categorized as temporal light artefacts.</rdfs:comment>
        <rdfs:label xml:lang="en">Temporal Light Artefacts</rdfs:label>
        <rdfs:label xml:lang="de">Temporäre Licht Artefakte</rdfs:label>
    </owl:Class>
    


    <!-- http://purl.org/auto/criticality_phenomena#CP_257 -->

    <owl:Class rdf:about="http://purl.org/auto/criticality_phenomena#CP_257">
        <rdfs:subClassOf rdf:resource="http://purl.org/auto/criticality_phenomena#CP_256"/>
        <dcterms:identifier rdf:datatype="http://www.w3.org/2001/XMLSchema#nonNegativeInteger">257</dcterms:identifier>
        <rdfs:comment xml:lang="en">Wikipedia: Flicker refers to unacceptable (irritating) light variation of a light source that is perceived by an average person, either directly or via a reflecting surface.</rdfs:comment>
        <rdfs:label xml:lang="de">Flackern</rdfs:label>
        <rdfs:label xml:lang="en">Flicker</rdfs:label>
    </owl:Class>
    


    <!-- http://purl.org/auto/criticality_phenomena#CP_258 -->

    <owl:Class rdf:about="http://purl.org/auto/criticality_phenomena#CP_258">
        <rdfs:subClassOf rdf:resource="http://purl.org/auto/criticality_phenomena#CP_210"/>
        <dcterms:identifier rdf:datatype="http://www.w3.org/2001/XMLSchema#nonNegativeInteger">258</dcterms:identifier>
        <rdfs:comment xml:lang="en">Wikipedia: Temporal light interference (TLI) is an unacceptable degradation of the performance of an equipment or system that has an optical input for its intended functioning and is caused by a temporal light modulation disturbance.</rdfs:comment>
        <rdfs:label xml:lang="en">Temporal Light Interference</rdfs:label>
        <rdfs:label xml:lang="de">Temporäre Licht Interferenz</rdfs:label>
    </owl:Class>
    


    <!-- http://purl.org/auto/criticality_phenomena#CP_26 -->

    <owl:Class rdf:about="http://purl.org/auto/criticality_phenomena#CP_26">
        <rdfs:subClassOf rdf:resource="http://purl.org/auto/criticality_phenomena#CP_265"/>
        <rdfs:subClassOf rdf:resource="http://purl.org/auto/criticality_phenomena#Perfect_Camera_Criticality_Phenomenon"/>
        <rdfs:subClassOf rdf:resource="http://purl.org/auto/criticality_phenomena#Perfect_Human_Criticality_Phenomenon"/>
        <rdfs:subClassOf rdf:resource="http://purl.org/auto/criticality_phenomena#Perfect_Lidar_Criticality_Phenomenon"/>
        <rdfs:subClassOf rdf:resource="http://purl.org/auto/criticality_phenomena#Perfect_Radar_Criticality_Phenomenon"/>
        <dcterms:identifier rdf:datatype="http://www.w3.org/2001/XMLSchema#nonNegativeInteger">26</dcterms:identifier>
        <rdfs:comment xml:lang="en">The occluded entity is a (part of a) traffic light.</rdfs:comment>
        <rdfs:label xml:lang="en">Occluded Traffic Light</rdfs:label>
        <rdfs:label xml:lang="de">verdeckte Ampel</rdfs:label>
    </owl:Class>
    


    <!-- http://purl.org/auto/criticality_phenomena#CP_265 -->

    <owl:Class rdf:about="http://purl.org/auto/criticality_phenomena#CP_265">
        <rdfs:subClassOf rdf:resource="http://purl.org/auto/criticality_phenomena#CP_25"/>
        <rdfs:subClassOf rdf:resource="http://purl.org/auto/criticality_phenomena#Complexity_Criticality_Phenomenon"/>
        <rdfs:subClassOf rdf:resource="http://purl.org/auto/criticality_phenomena#Dynamical_Criticality_Phenomenon"/>
        <rdfs:subClassOf rdf:resource="http://purl.org/auto/criticality_phenomena#Perfect_Perception_Criticality_Phenomenon"/>
        <rdfs:subClassOf rdf:resource="http://purl.org/auto/criticality_phenomena#Temporal_Criticality_Phenomenon"/>
        <dcterms:identifier rdf:datatype="http://www.w3.org/2001/XMLSchema#nonNegativeInteger">265</dcterms:identifier>
        <rdfs:comment xml:lang="en">Some entity which belongs to the traffic infrastructure is occluded.</rdfs:comment>
        <rdfs:label xml:lang="en">Occluded Traffic Infrastructure</rdfs:label>
        <rdfs:label xml:lang="de">Verdeckte Verkehrsinfrastruktur</rdfs:label>
    </owl:Class>
    


    <!-- http://purl.org/auto/criticality_phenomena#CP_266 -->

    <owl:Class rdf:about="http://purl.org/auto/criticality_phenomena#CP_266">
        <rdfs:subClassOf rdf:resource="http://purl.org/auto/criticality_phenomena#CP_265"/>
        <dcterms:identifier rdf:datatype="http://www.w3.org/2001/XMLSchema#nonNegativeInteger">266</dcterms:identifier>
        <rdfs:comment xml:lang="en">A lane is occluded.</rdfs:comment>
        <rdfs:label xml:lang="en">Occluded Lane</rdfs:label>
        <rdfs:label xml:lang="de">Verdeckter Fahrstreifen</rdfs:label>
    </owl:Class>
    


    <!-- http://purl.org/auto/criticality_phenomena#CP_27 -->

    <owl:Class rdf:about="http://purl.org/auto/criticality_phenomena#CP_27">
        <rdfs:subClassOf rdf:resource="http://purl.org/auto/criticality_phenomena#CP_178"/>
        <dcterms:identifier rdf:datatype="http://www.w3.org/2001/XMLSchema#nonNegativeInteger">27</dcterms:identifier>
        <rdfs:comment xml:lang="en">Drivable traffic space intersects with tram driving space (e.g. tram is driving on car lanes).</rdfs:comment>
        <rdfs:label xml:lang="en">Intersecting Tram Rails</rdfs:label>
        <rdfs:label xml:lang="de">Kreuzende Straßenbahnschienen</rdfs:label>
    </owl:Class>
    


    <!-- http://purl.org/auto/criticality_phenomena#CP_272 -->

    <owl:Class rdf:about="http://purl.org/auto/criticality_phenomena#CP_272">
        <rdfs:subClassOf rdf:resource="http://purl.org/auto/criticality_phenomena#Criticality_Phenomenon"/>
        <rdfs:subClassOf rdf:resource="http://purl.org/auto/criticality_phenomena#Perfect_Perception_Criticality_Phenomenon"/>
        <rdfs:subClassOf rdf:resource="http://purl.org/auto/criticality_phenomena#Unpredictability_Criticality_Phenomenon"/>
        <dcterms:identifier rdf:datatype="http://www.w3.org/2001/XMLSchema#nonNegativeInteger">272</dcterms:identifier>
        <rdfs:comment xml:lang="en">Areas of perception are limited, altered or defective.</rdfs:comment>
        <rdfs:label xml:lang="de">Abnormale Perzeption</rdfs:label>
        <rdfs:label xml:lang="en">Special Perception</rdfs:label>
    </owl:Class>
    


    <!-- http://purl.org/auto/criticality_phenomena#CP_273 -->

    <owl:Class rdf:about="http://purl.org/auto/criticality_phenomena#CP_273">
        <rdfs:subClassOf rdf:resource="http://purl.org/auto/criticality_phenomena#CP_274"/>
        <dcterms:identifier rdf:datatype="http://www.w3.org/2001/XMLSchema#nonNegativeInteger">273</dcterms:identifier>
        <rdfs:comment xml:lang="en">Visibility is affected by e.g. air particles or light conditions.</rdfs:comment>
        <rdfs:label xml:lang="en">Adverse Visibility Condition</rdfs:label>
        <rdfs:label xml:lang="de">Schlechte Sichtverhältnisse</rdfs:label>
    </owl:Class>
    


    <!-- http://purl.org/auto/criticality_phenomena#CP_274 -->

    <owl:Class rdf:about="http://purl.org/auto/criticality_phenomena#CP_274">
        <rdfs:subClassOf rdf:resource="http://purl.org/auto/criticality_phenomena#Criticality_Phenomenon"/>
        <rdfs:subClassOf rdf:resource="http://purl.org/auto/criticality_phenomena#Environmental_Criticality_Phenomenon"/>
        <rdfs:subClassOf rdf:resource="http://purl.org/auto/criticality_phenomena#Perfect_Perception_Criticality_Phenomenon"/>
        <dcterms:identifier rdf:datatype="http://www.w3.org/2001/XMLSchema#nonNegativeInteger">274</dcterms:identifier>
        <rdfs:comment xml:lang="en">Driving is affected by environmental conditions.</rdfs:comment>
        <rdfs:label xml:lang="en">Adverse Environmental Condition</rdfs:label>
        <rdfs:label xml:lang="de">Widrige Umweltbedingungen</rdfs:label>
    </owl:Class>
    


    <!-- http://purl.org/auto/criticality_phenomena#CP_275 -->

    <owl:Class rdf:about="http://purl.org/auto/criticality_phenomena#CP_275">
        <rdfs:subClassOf rdf:resource="http://purl.org/auto/criticality_phenomena#Criticality_Phenomenon"/>
        <rdfs:subClassOf rdf:resource="http://purl.org/auto/criticality_phenomena#Dynamical_Criticality_Phenomenon"/>
        <rdfs:subClassOf rdf:resource="http://purl.org/auto/criticality_phenomena#Unpredictability_Criticality_Phenomenon"/>
        <dcterms:identifier rdf:datatype="http://www.w3.org/2001/XMLSchema#nonNegativeInteger">275</dcterms:identifier>
        <rdfs:comment xml:lang="en">Parts of the vehicle are changed, broken or damaged.</rdfs:comment>
        <rdfs:label xml:lang="de">Abnormaler Fahrzeugzustand</rdfs:label>
        <rdfs:label xml:lang="en">Special Vehicle State</rdfs:label>
    </owl:Class>
    


    <!-- http://purl.org/auto/criticality_phenomena#CP_276 -->

    <owl:Class rdf:about="http://purl.org/auto/criticality_phenomena#CP_276">
        <rdfs:subClassOf rdf:resource="http://purl.org/auto/criticality_phenomena#CP_286"/>
        <rdfs:subClassOf rdf:resource="http://purl.org/auto/criticality_phenomena#Perfect_Perception_Criticality_Phenomenon"/>
        <rdfs:subClassOf rdf:resource="http://purl.org/auto/criticality_phenomena#Unpredictability_Criticality_Phenomenon"/>
        <dcterms:identifier rdf:datatype="http://www.w3.org/2001/XMLSchema#nonNegativeInteger">276</dcterms:identifier>
        <rdfs:comment xml:lang="en">Parts of the traffic infrastructure contain special features.</rdfs:comment>
        <rdfs:label xml:lang="de">Anormale Verkehrsinfrastruktur</rdfs:label>
        <rdfs:label xml:lang="en">Special Traffic Infrastructure</rdfs:label>
    </owl:Class>
    


    <!-- http://purl.org/auto/criticality_phenomena#CP_277 -->

    <owl:Class rdf:about="http://purl.org/auto/criticality_phenomena#CP_277">
        <rdfs:subClassOf rdf:resource="http://purl.org/auto/criticality_phenomena#CP_216"/>
        <rdfs:subClassOf rdf:resource="http://purl.org/auto/criticality_phenomena#Perfect_Perception_Criticality_Phenomenon"/>
        <dcterms:identifier rdf:datatype="http://www.w3.org/2001/XMLSchema#nonNegativeInteger">277</dcterms:identifier>
        <rdfs:comment xml:lang="en">Refers to a cyclist who push-to-front between or next to waiting vehicles, e.g. at a closed railroad crossing, a red traffic light or in a traffic jam.</rdfs:comment>
        <rdfs:label xml:lang="de">(Vor-)drängelnder Fahrradfahrer</rdfs:label>
        <rdfs:label xml:lang="en">Push-to-front Of Cyclist</rdfs:label>
    </owl:Class>
    


    <!-- http://purl.org/auto/criticality_phenomena#CP_278 -->

    <owl:Class rdf:about="http://purl.org/auto/criticality_phenomena#CP_278">
        <rdfs:subClassOf rdf:resource="http://purl.org/auto/criticality_phenomena#Criticality_Phenomenon"/>
        <rdfs:subClassOf rdf:resource="http://purl.org/auto/criticality_phenomena#Spatial_Criticality_Phenomenon"/>
        <dcterms:identifier rdf:datatype="http://www.w3.org/2001/XMLSchema#nonNegativeInteger">278</dcterms:identifier>
        <rdfs:comment xml:lang="en">There is an entity in the szene which might affect criticality.</rdfs:comment>
        <rdfs:label xml:lang="en">Entitiy In Scene</rdfs:label>
        <rdfs:label xml:lang="de">Existenz einer Entität in einer Szene</rdfs:label>
    </owl:Class>
    


    <!-- http://purl.org/auto/criticality_phenomena#CP_279 -->

    <owl:Class rdf:about="http://purl.org/auto/criticality_phenomena#CP_279">
        <rdfs:subClassOf rdf:resource="http://purl.org/auto/criticality_phenomena#CP_216"/>
        <dcterms:identifier rdf:datatype="http://www.w3.org/2001/XMLSchema#nonNegativeInteger">279</dcterms:identifier>
        <rdfs:comment xml:lang="en">An entity is passed by ego.</rdfs:comment>
        <rdfs:label xml:lang="de">Passieren eines Objekts</rdfs:label>
        <rdfs:label xml:lang="en">Passing Of Object</rdfs:label>
    </owl:Class>
    


    <!-- http://purl.org/auto/criticality_phenomena#CP_28 -->

    <owl:Class rdf:about="http://purl.org/auto/criticality_phenomena#CP_28">
        <rdfs:subClassOf rdf:resource="http://purl.org/auto/criticality_phenomena#CP_25"/>
        <formalized rdf:datatype="http://www.w3.org/2001/XMLSchema#boolean">true</formalized>
        <dcterms:identifier rdf:datatype="http://www.w3.org/2001/XMLSchema#nonNegativeInteger">28</dcterms:identifier>
        <rdfs:comment xml:lang="en">The occluded entity is a vehicle.</rdfs:comment>
        <rdfs:label xml:lang="en">Occluded Vehicle</rdfs:label>
        <rdfs:label xml:lang="de">verdecktes Fahrzeug</rdfs:label>
    </owl:Class>
    


    <!-- http://purl.org/auto/criticality_phenomena#CP_280 -->

    <owl:Class rdf:about="http://purl.org/auto/criticality_phenomena#CP_280">
        <rdfs:subClassOf rdf:resource="http://purl.org/auto/criticality_phenomena#CP_143"/>
        <rdfs:subClassOf rdf:resource="http://purl.org/auto/criticality_phenomena#Dynamical_Criticality_Phenomenon"/>
        <rdfs:subClassOf rdf:resource="http://purl.org/auto/criticality_phenomena#Spatial_Criticality_Phenomenon"/>
        <dcterms:identifier rdf:datatype="http://www.w3.org/2001/XMLSchema#nonNegativeInteger">280</dcterms:identifier>
        <rdfs:comment xml:lang="en">An entity is pushing in traffic.</rdfs:comment>
        <rdfs:label xml:lang="de">Drängeln</rdfs:label>
        <rdfs:label xml:lang="en">Pushing</rdfs:label>
    </owl:Class>
    


    <!-- http://purl.org/auto/criticality_phenomena#CP_281 -->

    <owl:Class rdf:about="http://purl.org/auto/criticality_phenomena#CP_281">
        <rdfs:subClassOf rdf:resource="http://purl.org/auto/criticality_phenomena#CP_47"/>
        <dcterms:identifier rdf:datatype="http://www.w3.org/2001/XMLSchema#nonNegativeInteger">281</dcterms:identifier>
        <rdfs:comment xml:lang="en">Load of a non-ego-TP is not secured.</rdfs:comment>
        <rdfs:label xml:lang="en">Insecured Load Of Non-Ego-TP</rdfs:label>
        <rdfs:label xml:lang="de">Ungesicherte Ladung von Non-Ego-TP</rdfs:label>
    </owl:Class>
    


    <!-- http://purl.org/auto/criticality_phenomena#CP_282 -->

    <owl:Class rdf:about="http://purl.org/auto/criticality_phenomena#CP_282">
        <rdfs:subClassOf rdf:resource="http://purl.org/auto/criticality_phenomena#CP_47"/>
        <dcterms:identifier rdf:datatype="http://www.w3.org/2001/XMLSchema#nonNegativeInteger">282</dcterms:identifier>
        <rdfs:comment xml:lang="en">A non-ego-TP is overloaded by more than 10%.</rdfs:comment>
        <rdfs:label xml:lang="en">Overloaded  Non-Ego-TP</rdfs:label>
        <rdfs:label xml:lang="de">Überlasteter Non-Ego-TP</rdfs:label>
    </owl:Class>
    


    <!-- http://purl.org/auto/criticality_phenomena#CP_283 -->

    <owl:Class rdf:about="http://purl.org/auto/criticality_phenomena#CP_283">
        <rdfs:subClassOf rdf:resource="http://purl.org/auto/criticality_phenomena#CP_284"/>
        <rdfs:subClassOf rdf:resource="http://purl.org/auto/criticality_phenomena#Unpredictability_Criticality_Phenomenon"/>
        <dcterms:identifier rdf:datatype="http://www.w3.org/2001/XMLSchema#nonNegativeInteger">283</dcterms:identifier>
        <rdfs:comment xml:lang="en">TP behaves wrong or unexpected.</rdfs:comment>
        <rdfs:label xml:lang="de">Abnormales Verhalten von TP</rdfs:label>
        <rdfs:label xml:lang="en">Special Behavior Of TP</rdfs:label>
    </owl:Class>
    


    <!-- http://purl.org/auto/criticality_phenomena#CP_284 -->

    <owl:Class rdf:about="http://purl.org/auto/criticality_phenomena#CP_284">
        <rdfs:subClassOf rdf:resource="http://purl.org/auto/criticality_phenomena#Behavioral_Criticality_Phenomenon"/>
        <rdfs:subClassOf rdf:resource="http://purl.org/auto/criticality_phenomena#Criticality_Phenomenon"/>
        <dcterms:identifier rdf:datatype="http://www.w3.org/2001/XMLSchema#nonNegativeInteger">284</dcterms:identifier>
        <rdfs:comment xml:lang="en">TP behaves in a safety critical way.</rdfs:comment>
        <rdfs:label xml:lang="en">Behavior Of TP</rdfs:label>
        <rdfs:label xml:lang="de">Verhalten von TP</rdfs:label>
    </owl:Class>
    


    <!-- http://purl.org/auto/criticality_phenomena#CP_285 -->

    <owl:Class rdf:about="http://purl.org/auto/criticality_phenomena#CP_285">
        <rdfs:subClassOf rdf:resource="http://purl.org/auto/criticality_phenomena#CP_164"/>
        <rdfs:subClassOf rdf:resource="http://purl.org/auto/criticality_phenomena#Dynamical_Criticality_Phenomenon"/>
        <dcterms:identifier rdf:datatype="http://www.w3.org/2001/XMLSchema#nonNegativeInteger">285</dcterms:identifier>
        <rdfs:comment xml:lang="en">Refers to environmental force like wind which may lead to changed dynamics.</rdfs:comment>
        <rdfs:label xml:lang="en">Environmental Force</rdfs:label>
        <rdfs:label xml:lang="de">Umgebungskraft</rdfs:label>
    </owl:Class>
    


    <!-- http://purl.org/auto/criticality_phenomena#CP_286 -->

    <owl:Class rdf:about="http://purl.org/auto/criticality_phenomena#CP_286">
        <rdfs:subClassOf rdf:resource="http://purl.org/auto/criticality_phenomena#Criticality_Phenomenon"/>
        <rdfs:subClassOf rdf:resource="http://purl.org/auto/criticality_phenomena#Dynamical_Criticality_Phenomenon"/>
        <dcterms:identifier rdf:datatype="http://www.w3.org/2001/XMLSchema#nonNegativeInteger">286</dcterms:identifier>
        <rdfs:comment xml:lang="en">The road network might have special structures like intersections or might be in a special state.</rdfs:comment>
        <rdfs:label xml:lang="de">Besondere bauliche Gegebenheiten</rdfs:label>
        <rdfs:label xml:lang="en">Special structural circumstances</rdfs:label>
    </owl:Class>
    


    <!-- http://purl.org/auto/criticality_phenomena#CP_287 -->

    <owl:Class rdf:about="http://purl.org/auto/criticality_phenomena#CP_287">
        <rdfs:subClassOf rdf:resource="http://purl.org/auto/criticality_phenomena#Criticality_Phenomenon"/>
        <rdfs:subClassOf rdf:resource="http://purl.org/auto/criticality_phenomena#Unpredictability_Criticality_Phenomenon"/>
        <dcterms:identifier rdf:datatype="http://www.w3.org/2001/XMLSchema#nonNegativeInteger">287</dcterms:identifier>
        <rdfs:comment xml:lang="en">Refers to states of traffic which occure less often like traffic jam or collective misconduct.</rdfs:comment>
        <rdfs:label xml:lang="de">Besondere Verkehrskonstellation</rdfs:label>
        <rdfs:label xml:lang="en">Special Traffic Constellation</rdfs:label>
    </owl:Class>
    


    <!-- http://purl.org/auto/criticality_phenomena#CP_288 -->

    <owl:Class rdf:about="http://purl.org/auto/criticality_phenomena#CP_288">
        <rdfs:subClassOf rdf:resource="http://purl.org/auto/criticality_phenomena#CP_287"/>
        <rdfs:subClassOf rdf:resource="http://purl.org/auto/criticality_phenomena#Dynamical_Criticality_Phenomenon"/>
        <dcterms:identifier rdf:datatype="http://www.w3.org/2001/XMLSchema#nonNegativeInteger">288</dcterms:identifier>
        <rdfs:comment xml:lang="en">A line or lines of stationary or very slow-moving traffic, caused by roadworks, an accident, or heavy congestion.</rdfs:comment>
        <rdfs:label xml:lang="de">Stau</rdfs:label>
        <rdfs:label xml:lang="en">Traffic Jam</rdfs:label>
    </owl:Class>
    


    <!-- http://purl.org/auto/criticality_phenomena#CP_29 -->

    <owl:Class rdf:about="http://purl.org/auto/criticality_phenomena#CP_29">
        <rdfs:subClassOf rdf:resource="http://purl.org/auto/criticality_phenomena#CP_283"/>
        <rdfs:subClassOf rdf:resource="http://purl.org/auto/criticality_phenomena#Dynamical_Criticality_Phenomenon"/>
        <rdfs:subClassOf rdf:resource="http://purl.org/auto/criticality_phenomena#Perfect_Perception_Criticality_Phenomenon"/>
        <dcterms:identifier rdf:datatype="http://www.w3.org/2001/XMLSchema#nonNegativeInteger">29</dcterms:identifier>
        <rdfs:comment xml:lang="en">TP has a speed which is not adapted to the current situation. May still be lower than the speed limit.</rdfs:comment>
        <rdfs:label xml:lang="en">Inappropriate Speed Of Non-Ego-TP</rdfs:label>
        <rdfs:label xml:lang="de">Non-Ego-TP hat nicht angepasste Geschwindigkeit</rdfs:label>
    </owl:Class>
    


    <!-- http://purl.org/auto/criticality_phenomena#CP_291 -->

    <owl:Class rdf:about="http://purl.org/auto/criticality_phenomena#CP_291">
        <rdfs:subClassOf rdf:resource="http://purl.org/auto/criticality_phenomena#CP_297"/>
        <dcterms:identifier rdf:datatype="http://www.w3.org/2001/XMLSchema#nonNegativeInteger">291</dcterms:identifier>
        <rdfs:comment xml:lang="en">The rescue alley has been collectively formed on wrong side.</rdfs:comment>
        <rdfs:label xml:lang="en">Rescue alley formed on wrong side</rdfs:label>
        <rdfs:label xml:lang="de">Rettungsgasse auf falscher Seite gebildet</rdfs:label>
    </owl:Class>
    


    <!-- http://purl.org/auto/criticality_phenomena#CP_292 -->

    <owl:Class rdf:about="http://purl.org/auto/criticality_phenomena#CP_292">
        <rdfs:subClassOf rdf:resource="http://purl.org/auto/criticality_phenomena#CP_297"/>
        <dcterms:identifier rdf:datatype="http://www.w3.org/2001/XMLSchema#nonNegativeInteger">292</dcterms:identifier>
        <rdfs:comment xml:lang="en">The lane assignment is not taken into account by traffic.</rdfs:comment>
        <rdfs:label xml:lang="de">Fahrstreifenzuordnung wird nicht vom Verkehr berücksichtigt</rdfs:label>
        <rdfs:label xml:lang="en">Lane assignment is not taken into account by traffic</rdfs:label>
    </owl:Class>
    


    <!-- http://purl.org/auto/criticality_phenomena#CP_293 -->

    <owl:Class rdf:about="http://purl.org/auto/criticality_phenomena#CP_293">
        <rdfs:subClassOf rdf:resource="http://purl.org/auto/criticality_phenomena#Criticality_Phenomenon"/>
        <rdfs:subClassOf rdf:resource="http://purl.org/auto/criticality_phenomena#Dynamical_Criticality_Phenomenon"/>
        <rdfs:subClassOf rdf:resource="http://purl.org/auto/criticality_phenomena#Perfect_Perception_Criticality_Phenomenon"/>
        <rdfs:subClassOf rdf:resource="http://purl.org/auto/criticality_phenomena#Spatial_Criticality_Phenomenon"/>
        <rdfs:subClassOf rdf:resource="http://purl.org/auto/criticality_phenomena#Temporal_Criticality_Phenomenon"/>
        <dcterms:identifier rdf:datatype="http://www.w3.org/2001/XMLSchema#nonNegativeInteger">293</dcterms:identifier>
        <rdfs:comment xml:lang="en">The intended paths of at least two TPs intersect, i.e. they are not driving parallel or away from each other.</rdfs:comment>
        <rdfs:label xml:lang="en">Intersecting Planned Paths Of TPs</rdfs:label>
        <rdfs:label xml:lang="de">kreuzende geplante Fahrpfade der Verkehrsteilnehmer</rdfs:label>
    </owl:Class>
    


    <!-- http://purl.org/auto/criticality_phenomena#CP_294 -->

    <owl:Class rdf:about="http://purl.org/auto/criticality_phenomena#CP_294">
        <rdfs:subClassOf rdf:resource="http://purl.org/auto/criticality_phenomena#CP_274"/>
        <rdfs:subClassOf rdf:resource="http://purl.org/auto/criticality_phenomena#Unpredictability_Criticality_Phenomenon"/>
        <dcterms:identifier rdf:datatype="http://www.w3.org/2001/XMLSchema#nonNegativeInteger">294</dcterms:identifier>
        <rdfs:comment xml:lang="en">Air temperature is at or below 0 degrees Celsius.</rdfs:comment>
        <rdfs:label xml:lang="de">Eiskalte Temperaturen</rdfs:label>
        <rdfs:label xml:lang="en">Freezing Temperatures</rdfs:label>
    </owl:Class>
    


    <!-- http://purl.org/auto/criticality_phenomena#CP_295 -->

    <owl:Class rdf:about="http://purl.org/auto/criticality_phenomena#CP_295">
        <rdfs:subClassOf rdf:resource="http://purl.org/auto/criticality_phenomena#CP_17"/>
        <dcterms:identifier rdf:datatype="http://www.w3.org/2001/XMLSchema#nonNegativeInteger">295</dcterms:identifier>
        <rdfs:comment xml:lang="en">Rain that has an intensity of over or equal to 10 mm/h.</rdfs:comment>
        <rdfs:label xml:lang="en">Heavy Rain</rdfs:label>
        <rdfs:label xml:lang="de">Starkregen</rdfs:label>
    </owl:Class>
    


    <!-- http://purl.org/auto/criticality_phenomena#CP_296 -->

    <owl:Class rdf:about="http://purl.org/auto/criticality_phenomena#CP_296">
        <rdfs:subClassOf rdf:resource="http://purl.org/auto/criticality_phenomena#CP_143"/>
        <dcterms:identifier rdf:datatype="http://www.w3.org/2001/XMLSchema#nonNegativeInteger">296</dcterms:identifier>
        <rdfs:comment xml:lang="en">Not turning on the low beam or back lights in darkness (e.g. during night).</rdfs:comment>
        <rdfs:label xml:lang="de">Fehlende Beleuchtung in Dunkelheit</rdfs:label>
        <rdfs:label xml:lang="en">No Vehicle Lights in Darkness</rdfs:label>
    </owl:Class>
    


    <!-- http://purl.org/auto/criticality_phenomena#CP_297 -->

    <owl:Class rdf:about="http://purl.org/auto/criticality_phenomena#CP_297">
        <rdfs:subClassOf rdf:resource="http://purl.org/auto/criticality_phenomena#Behavioral_Criticality_Phenomenon"/>
        <rdfs:subClassOf rdf:resource="http://purl.org/auto/criticality_phenomena#CP_287"/>
        <dcterms:identifier rdf:datatype="http://www.w3.org/2001/XMLSchema#nonNegativeInteger">297</dcterms:identifier>
        <rdfs:comment xml:lang="en">Several road users act wrongly but collectively.</rdfs:comment>
        <rdfs:label xml:lang="en">Collaborative Misconduct</rdfs:label>
        <rdfs:label xml:lang="de">Gemeinschaftliches Fehlverhalten</rdfs:label>
    </owl:Class>
    


    <!-- http://purl.org/auto/criticality_phenomena#CP_298 -->

    <owl:Class rdf:about="http://purl.org/auto/criticality_phenomena#CP_298">
        <rdfs:subClassOf rdf:resource="http://purl.org/auto/criticality_phenomena#CP_288"/>
        <dcterms:identifier rdf:datatype="http://www.w3.org/2001/XMLSchema#nonNegativeInteger">298</dcterms:identifier>
        <rdfs:comment xml:lang="en">Refers to the existence of traffic jam on slip roads.</rdfs:comment>
        <rdfs:label xml:lang="de">Stau auf Autobahnauffahrten </rdfs:label>
        <rdfs:label xml:lang="en">Traffic jam on slip roads</rdfs:label>
    </owl:Class>
    


    <!-- http://purl.org/auto/criticality_phenomena#CP_299 -->

    <owl:Class rdf:about="http://purl.org/auto/criticality_phenomena#CP_299">
        <rdfs:subClassOf rdf:resource="http://purl.org/auto/criticality_phenomena#CP_288"/>
        <dcterms:identifier rdf:datatype="http://www.w3.org/2001/XMLSchema#nonNegativeInteger">299</dcterms:identifier>
        <rdfs:comment xml:lang="en">Refers to the existence of traffic jam on motorway exits.</rdfs:comment>
        <rdfs:label xml:lang="de">Stau auf Autobahnabfahrten</rdfs:label>
        <rdfs:label xml:lang="en">Traffic jam on motorway exit</rdfs:label>
    </owl:Class>
    


    <!-- http://purl.org/auto/criticality_phenomena#CP_3 -->

    <owl:Class rdf:about="http://purl.org/auto/criticality_phenomena#CP_3">
        <rdfs:subClassOf rdf:resource="http://purl.org/auto/criticality_phenomena#CP_216"/>
        <rdfs:subClassOf rdf:resource="http://purl.org/auto/criticality_phenomena#Complexity_Criticality_Phenomenon"/>
        <rdfs:subClassOf rdf:resource="http://purl.org/auto/criticality_phenomena#Perfect_Perception_Criticality_Phenomenon"/>
        <dcterms:identifier rdf:datatype="http://www.w3.org/2001/XMLSchema#nonNegativeInteger">3</dcterms:identifier>
        <rdfs:comment xml:lang="en">A oncoming vehicle has a planned trajectory that intersects with the planned left turn trajectory of ego. Standard situation at urban intersections.</rdfs:comment>
        <rdfs:label xml:lang="de">Gegenverkehr beim Linksabbiegen</rdfs:label>
        <rdfs:label xml:lang="en">Intersecting Oncoming Traffic During Left Turn</rdfs:label>
    </owl:Class>
    


    <!-- http://purl.org/auto/criticality_phenomena#CP_30 -->

    <owl:Class rdf:about="http://purl.org/auto/criticality_phenomena#CP_30">
        <rdfs:subClassOf rdf:resource="http://purl.org/auto/criticality_phenomena#CP_211"/>
        <rdfs:subClassOf rdf:resource="http://purl.org/auto/criticality_phenomena#Real_Camera_Criticality_Phenomenon"/>
        <rdfs:subClassOf rdf:resource="http://purl.org/auto/criticality_phenomena#Real_Human_Criticality_Phenomenon"/>
        <rdfs:subClassOf rdf:resource="http://purl.org/auto/criticality_phenomena#Real_Lidar_Criticality_Phenomenon"/>
        <rdfs:subClassOf rdf:resource="http://purl.org/auto/criticality_phenomena#Real_Perception_Algorithm_Criticality_Phenomenon"/>
        <rdfs:subClassOf rdf:resource="http://purl.org/auto/criticality_phenomena#Real_Radar_Criticality_Phenomenon"/>
        <dcterms:identifier rdf:datatype="http://www.w3.org/2001/XMLSchema#nonNegativeInteger">30</dcterms:identifier>
        <rdfs:comment xml:lang="en">Any sign that is not an official sign and not a traffic sign, such as advertisement board, election posters, corporate signposts, ...</rdfs:comment>
        <rdfs:label xml:lang="en">Unofficial Non-traffic Signs</rdfs:label>
        <rdfs:label xml:lang="de">inoffizielles Beschilderung</rdfs:label>
    </owl:Class>
    


    <!-- http://purl.org/auto/criticality_phenomena#CP_300 -->

    <owl:Class rdf:about="http://purl.org/auto/criticality_phenomena#CP_300">
        <rdfs:subClassOf rdf:resource="http://purl.org/auto/criticality_phenomena#CP_288"/>
        <dcterms:identifier rdf:datatype="http://www.w3.org/2001/XMLSchema#nonNegativeInteger">300</dcterms:identifier>
        <rdfs:comment xml:lang="en">Refers to the existence of traffic jam on specific lanes.</rdfs:comment>
        <rdfs:label xml:lang="en">Partial traffic jam</rdfs:label>
        <rdfs:label xml:lang="de">Partieller Stau</rdfs:label>
    </owl:Class>
    


    <!-- http://purl.org/auto/criticality_phenomena#CP_301 -->

    <owl:Class rdf:about="http://purl.org/auto/criticality_phenomena#CP_301">
        <rdfs:subClassOf rdf:resource="http://purl.org/auto/criticality_phenomena#CP_287"/>
        <rdfs:subClassOf rdf:resource="http://purl.org/auto/criticality_phenomena#Dynamical_Criticality_Phenomenon"/>
        <dcterms:identifier rdf:datatype="http://www.w3.org/2001/XMLSchema#nonNegativeInteger">301</dcterms:identifier>
        <rdfs:comment xml:lang="en">In specific times a higher amount of traffic is present.</rdfs:comment>
        <rdfs:label xml:lang="de">Hohe Verkehrsdichte</rdfs:label>
        <rdfs:label xml:lang="en">Rush Hour</rdfs:label>
    </owl:Class>
    


    <!-- http://purl.org/auto/criticality_phenomena#CP_302 -->

    <owl:Class rdf:about="http://purl.org/auto/criticality_phenomena#CP_302">
        <rdfs:subClassOf rdf:resource="http://purl.org/auto/criticality_phenomena#CP_287"/>
        <rdfs:subClassOf rdf:resource="http://purl.org/auto/criticality_phenomena#Dynamical_Criticality_Phenomenon"/>
        <dcterms:identifier rdf:datatype="http://www.w3.org/2001/XMLSchema#nonNegativeInteger">302</dcterms:identifier>
        <rdfs:comment xml:lang="en">Collars drive under specific rules which are different than the normal rules for driving (e.g. run red traffic lights).</rdfs:comment>
        <rdfs:label xml:lang="en">Collars</rdfs:label>
        <rdfs:label xml:lang="de">Kolonnen</rdfs:label>
    </owl:Class>
    


    <!-- http://purl.org/auto/criticality_phenomena#CP_303 -->

    <owl:Class rdf:about="http://purl.org/auto/criticality_phenomena#CP_303">
        <rdfs:subClassOf rdf:resource="http://purl.org/auto/criticality_phenomena#CP_287"/>
        <rdfs:subClassOf rdf:resource="http://purl.org/auto/criticality_phenomena#Dynamical_Criticality_Phenomenon"/>
        <dcterms:identifier rdf:datatype="http://www.w3.org/2001/XMLSchema#nonNegativeInteger">303</dcterms:identifier>
        <rdfs:comment xml:lang="en">Motorcades might act different than normal traffic.</rdfs:comment>
        <rdfs:label xml:lang="de">Autokorso</rdfs:label>
        <rdfs:label xml:lang="en">Motorcade</rdfs:label>
    </owl:Class>
    


    <!-- http://purl.org/auto/criticality_phenomena#CP_304 -->

    <owl:Class rdf:about="http://purl.org/auto/criticality_phenomena#CP_304">
        <rdfs:subClassOf rdf:resource="http://purl.org/auto/criticality_phenomena#CP_297"/>
        <rdfs:subClassOf rdf:resource="http://purl.org/auto/criticality_phenomena#Complexity_Criticality_Phenomenon"/>
        <rdfs:subClassOf rdf:resource="http://purl.org/auto/criticality_phenomena#Unpredictability_Criticality_Phenomenon"/>
        <dcterms:identifier rdf:datatype="http://www.w3.org/2001/XMLSchema#nonNegativeInteger">304</dcterms:identifier>
        <rdfs:comment xml:lang="en">Community driving through a traffic circle in the wrong direction. Might be due to an accident.</rdfs:comment>
        <rdfs:label xml:lang="en">Community driving through a traffic circle in the wrong direction</rdfs:label>
        <rdfs:label xml:lang="de">Kreisverkehr in falscher Richtung durchfahren</rdfs:label>
    </owl:Class>
    


    <!-- http://purl.org/auto/criticality_phenomena#CP_305 -->

    <owl:Class rdf:about="http://purl.org/auto/criticality_phenomena#CP_305">
        <rdfs:subClassOf rdf:resource="http://purl.org/auto/criticality_phenomena#CP_275"/>
        <rdfs:subClassOf rdf:resource="http://purl.org/auto/criticality_phenomena#Perception_Criticality_Phenomenon"/>
        <dcterms:identifier rdf:datatype="http://www.w3.org/2001/XMLSchema#nonNegativeInteger">305</dcterms:identifier>
        <rdfs:comment xml:lang="en">TP drives with an open trunk. Might be due to cargo.</rdfs:comment>
        <rdfs:label xml:lang="de">Offener Kofferraum</rdfs:label>
        <rdfs:label xml:lang="en">Open trunk</rdfs:label>
    </owl:Class>
    


    <!-- http://purl.org/auto/criticality_phenomena#CP_306 -->

    <owl:Class rdf:about="http://purl.org/auto/criticality_phenomena#CP_306">
        <rdfs:subClassOf rdf:resource="http://purl.org/auto/criticality_phenomena#CP_275"/>
        <rdfs:subClassOf rdf:resource="http://purl.org/auto/criticality_phenomena#Perception_Criticality_Phenomenon"/>
        <dcterms:identifier rdf:datatype="http://www.w3.org/2001/XMLSchema#nonNegativeInteger">306</dcterms:identifier>
        <rdfs:comment xml:lang="en">TP drives with overhanging load e.g on top of a car.</rdfs:comment>
        <rdfs:label xml:lang="en">Overhanging load</rdfs:label>
        <rdfs:label xml:lang="de">Überhängende Beladung</rdfs:label>
    </owl:Class>
    


    <!-- http://purl.org/auto/criticality_phenomena#CP_307 -->

    <owl:Class rdf:about="http://purl.org/auto/criticality_phenomena#CP_307">
        <rdfs:subClassOf rdf:resource="http://purl.org/auto/criticality_phenomena#CP_275"/>
        <rdfs:subClassOf rdf:resource="http://purl.org/auto/criticality_phenomena#Perception_Criticality_Phenomenon"/>
        <dcterms:identifier rdf:datatype="http://www.w3.org/2001/XMLSchema#nonNegativeInteger">307</dcterms:identifier>
        <rdfs:comment xml:lang="en">TP has an open door. Might be during parking or driving.</rdfs:comment>
        <rdfs:label xml:lang="de">Offene Tür eines TP</rdfs:label>
        <rdfs:label xml:lang="en">Open door of TP</rdfs:label>
    </owl:Class>
    


    <!-- http://purl.org/auto/criticality_phenomena#CP_308 -->

    <owl:Class rdf:about="http://purl.org/auto/criticality_phenomena#CP_308">
        <rdfs:subClassOf rdf:resource="http://purl.org/auto/criticality_phenomena#CP_116"/>
        <dcterms:identifier rdf:datatype="http://www.w3.org/2001/XMLSchema#nonNegativeInteger">308</dcterms:identifier>
        <rdfs:comment xml:lang="en">Broken tires can lead to changes in the dynamic of vehicles.</rdfs:comment>
        <rdfs:label xml:lang="en">Broken tires</rdfs:label>
        <rdfs:label xml:lang="de">Kaputte Reifen</rdfs:label>
    </owl:Class>
    


    <!-- http://purl.org/auto/criticality_phenomena#CP_309 -->

    <owl:Class rdf:about="http://purl.org/auto/criticality_phenomena#CP_309">
        <rdfs:subClassOf rdf:resource="http://purl.org/auto/criticality_phenomena#CP_115"/>
        <dcterms:identifier rdf:datatype="http://www.w3.org/2001/XMLSchema#nonNegativeInteger">309</dcterms:identifier>
        <rdfs:comment xml:lang="en">Decreased tread might lead to reduced friction.</rdfs:comment>
        <rdfs:label xml:lang="en">Decreased tread</rdfs:label>
        <rdfs:label xml:lang="de">Vermindertes Reifenprofil</rdfs:label>
    </owl:Class>
    


    <!-- http://purl.org/auto/criticality_phenomena#CP_31 -->

    <owl:Class rdf:about="http://purl.org/auto/criticality_phenomena#CP_31">
        <rdfs:subClassOf rdf:resource="http://purl.org/auto/criticality_phenomena#CP_32"/>
        <dcterms:identifier rdf:datatype="http://www.w3.org/2001/XMLSchema#nonNegativeInteger">31</dcterms:identifier>
        <rdfs:comment xml:lang="en">This includes pet animals with which collision should be avoided such as dogs and cats</rdfs:comment>
        <rdfs:label xml:lang="de">Haustier auf der Straße</rdfs:label>
        <rdfs:label xml:lang="en">Pet Animal On Road</rdfs:label>
    </owl:Class>
    


    <!-- http://purl.org/auto/criticality_phenomena#CP_310 -->

    <owl:Class rdf:about="http://purl.org/auto/criticality_phenomena#CP_310">
        <rdfs:subClassOf rdf:resource="http://purl.org/auto/criticality_phenomena#CP_275"/>
        <rdfs:subClassOf rdf:resource="http://purl.org/auto/criticality_phenomena#Perception_Criticality_Phenomenon"/>
        <dcterms:identifier rdf:datatype="http://www.w3.org/2001/XMLSchema#nonNegativeInteger">310</dcterms:identifier>
        <rdfs:comment xml:lang="en">Unusual appearance (or unusual form) might affect the ability to detect the according TP correctly.</rdfs:comment>
        <rdfs:label xml:lang="de">Ungewöhnliches Aussehen eines TP</rdfs:label>
        <rdfs:label xml:lang="en">Unusual appearance of TP</rdfs:label>
    </owl:Class>
    


    <!-- http://purl.org/auto/criticality_phenomena#CP_311 -->

    <owl:Class rdf:about="http://purl.org/auto/criticality_phenomena#CP_311">
        <rdfs:subClassOf rdf:resource="http://purl.org/auto/criticality_phenomena#CP_310"/>
        <dcterms:identifier rdf:datatype="http://www.w3.org/2001/XMLSchema#nonNegativeInteger">311</dcterms:identifier>
        <rdfs:comment xml:lang="en">A development mule is a car which is often camouflaged. This may lead to problems in detecting the vehicle correctly.</rdfs:comment>
        <rdfs:label xml:lang="en">Development mule</rdfs:label>
        <rdfs:label xml:lang="de">Erlkönig (Auto)</rdfs:label>
    </owl:Class>
    


    <!-- http://purl.org/auto/criticality_phenomena#CP_312 -->

    <owl:Class rdf:about="http://purl.org/auto/criticality_phenomena#CP_312">
        <rdfs:subClassOf rdf:resource="http://purl.org/auto/criticality_phenomena#CP_310"/>
        <rdfs:subClassOf rdf:resource="http://purl.org/auto/criticality_phenomena#Dynamical_Criticality_Phenomenon"/>
        <dcterms:identifier rdf:datatype="http://www.w3.org/2001/XMLSchema#nonNegativeInteger">312</dcterms:identifier>
        <rdfs:comment xml:lang="en">A tuned car is different from the original model. This may lead to changed dynamics as well as changed appearence.</rdfs:comment>
        <rdfs:label xml:lang="de">Getuntes Fahrzeug </rdfs:label>
        <rdfs:label xml:lang="en">Tuned vehicle</rdfs:label>
    </owl:Class>
    


    <!-- http://purl.org/auto/criticality_phenomena#CP_313 -->

    <owl:Class rdf:about="http://purl.org/auto/criticality_phenomena#CP_313">
        <rdfs:subClassOf rdf:resource="http://purl.org/auto/criticality_phenomena#CP_310"/>
        <rdfs:subClassOf rdf:resource="http://purl.org/auto/criticality_phenomena#Dynamical_Criticality_Phenomenon"/>
        <rdfs:subClassOf rdf:resource="http://purl.org/auto/criticality_phenomena#Unpredictability_Criticality_Phenomenon"/>
        <dcterms:identifier rdf:datatype="http://www.w3.org/2001/XMLSchema#nonNegativeInteger">313</dcterms:identifier>
        <rdfs:comment xml:lang="en">Special cars might have sliding doors or no side door. This allows passengers to exit the car without open a door to the side.</rdfs:comment>
        <rdfs:label xml:lang="de">Fahrzeug mit Schiebetür/ ohne Seitentür</rdfs:label>
        <rdfs:label xml:lang="en">Vehicle with sliding door/ without side door</rdfs:label>
    </owl:Class>
    


    <!-- http://purl.org/auto/criticality_phenomena#CP_314 -->

    <owl:Class rdf:about="http://purl.org/auto/criticality_phenomena#CP_314">
        <rdfs:subClassOf rdf:resource="http://purl.org/auto/criticality_phenomena#CP_216"/>
        <dcterms:identifier rdf:datatype="http://www.w3.org/2001/XMLSchema#nonNegativeInteger">314</dcterms:identifier>
        <rdfs:comment xml:lang="en">To enter the highway one has to merge on the right lane.</rdfs:comment>
        <rdfs:label xml:lang="de">Auffahren auf die Autobahn</rdfs:label>
        <rdfs:label xml:lang="en">Merging at highway entry</rdfs:label>
    </owl:Class>
    


    <!-- http://purl.org/auto/criticality_phenomena#CP_315 -->

    <owl:Class rdf:about="http://purl.org/auto/criticality_phenomena#CP_315">
        <rdfs:subClassOf rdf:resource="http://purl.org/auto/criticality_phenomena#CP_216"/>
        <dcterms:identifier rdf:datatype="http://www.w3.org/2001/XMLSchema#nonNegativeInteger">315</dcterms:identifier>
        <rdfs:comment xml:lang="en">To keep driving one has to merge on continuing lane.</rdfs:comment>
        <rdfs:label xml:lang="en">Merging at lane end</rdfs:label>
        <rdfs:label xml:lang="de">Spurwechsel vor Ende einer Spur</rdfs:label>
    </owl:Class>
    


    <!-- http://purl.org/auto/criticality_phenomena#CP_316 -->

    <owl:Class rdf:about="http://purl.org/auto/criticality_phenomena#CP_316">
        <rdfs:subClassOf rdf:resource="http://purl.org/auto/criticality_phenomena#CP_216"/>
        <dcterms:identifier rdf:datatype="http://www.w3.org/2001/XMLSchema#nonNegativeInteger">316</dcterms:identifier>
        <rdfs:comment xml:lang="en">Refers to the need of merging on an occupied lane (for example due to traffic jam). For this an estimation of the behavior of the other drivers is needed.</rdfs:comment>
        <rdfs:label xml:lang="en">Merging into an occupied lane</rdfs:label>
        <rdfs:label xml:lang="de">Spurwechsel auf eine volle Spur</rdfs:label>
    </owl:Class>
    


    <!-- http://purl.org/auto/criticality_phenomena#CP_317 -->

    <owl:Class rdf:about="http://purl.org/auto/criticality_phenomena#CP_317">
        <rdfs:subClassOf rdf:resource="http://purl.org/auto/criticality_phenomena#CP_216"/>
        <dcterms:identifier rdf:datatype="http://www.w3.org/2001/XMLSchema#nonNegativeInteger">317</dcterms:identifier>
        <rdfs:comment xml:lang="en">A TP cuts in in front of the ego-vehicle.</rdfs:comment>
        <rdfs:label xml:lang="en">Cut-in in front of ego-vehicle</rdfs:label>
        <rdfs:label xml:lang="de">Einscheren vor dem Ego-Fahrzeug</rdfs:label>
    </owl:Class>
    


    <!-- http://purl.org/auto/criticality_phenomena#CP_318 -->

    <owl:Class rdf:about="http://purl.org/auto/criticality_phenomena#CP_318">
        <rdfs:subClassOf rdf:resource="http://purl.org/auto/criticality_phenomena#CP_216"/>
        <dcterms:identifier rdf:datatype="http://www.w3.org/2001/XMLSchema#nonNegativeInteger">318</dcterms:identifier>
        <rdfs:comment xml:lang="en">A TP cuts out in front of the ego-vehicle.</rdfs:comment>
        <rdfs:label xml:lang="de">Ausscheren vor dem Ego-Fahrzeug</rdfs:label>
        <rdfs:label xml:lang="en">Cut-out in front of ego-vehicle</rdfs:label>
    </owl:Class>
    


    <!-- http://purl.org/auto/criticality_phenomena#CP_319 -->

    <owl:Class rdf:about="http://purl.org/auto/criticality_phenomena#CP_319">
        <rdfs:subClassOf rdf:resource="http://purl.org/auto/criticality_phenomena#CP_208"/>
        <rdfs:subClassOf rdf:resource="http://purl.org/auto/criticality_phenomena#Complexity_Criticality_Phenomenon"/>
        <dcterms:identifier rdf:datatype="http://www.w3.org/2001/XMLSchema#nonNegativeInteger">319</dcterms:identifier>
        <rdfs:comment xml:lang="en">A toll station is located on the road.</rdfs:comment>
        <rdfs:label xml:lang="de">Mautstelle</rdfs:label>
        <rdfs:label xml:lang="en">Toll</rdfs:label>
    </owl:Class>
    


    <!-- http://purl.org/auto/criticality_phenomena#CP_32 -->

    <owl:Class rdf:about="http://purl.org/auto/criticality_phenomena#CP_32">
        <rdfs:subClassOf rdf:resource="http://purl.org/auto/criticality_phenomena#Behavioral_Criticality_Phenomenon"/>
        <rdfs:subClassOf rdf:resource="http://purl.org/auto/criticality_phenomena#CP_212"/>
        <rdfs:subClassOf rdf:resource="http://purl.org/auto/criticality_phenomena#Perfect_Perception_Criticality_Phenomenon"/>
        <rdfs:subClassOf rdf:resource="http://purl.org/auto/criticality_phenomena#Unpredictability_Criticality_Phenomenon"/>
        <dcterms:identifier rdf:datatype="http://www.w3.org/2001/XMLSchema#nonNegativeInteger">32</dcterms:identifier>
        <rdfs:comment xml:lang="en">A subject (human or animal) is located on the road.</rdfs:comment>
        <rdfs:label xml:lang="en">Subject On Road</rdfs:label>
        <rdfs:label xml:lang="de">Subjekt auf der Straße</rdfs:label>
    </owl:Class>
    


    <!-- http://purl.org/auto/criticality_phenomena#CP_321 -->

    <owl:Class rdf:about="http://purl.org/auto/criticality_phenomena#CP_321">
        <rdfs:subClassOf rdf:resource="http://purl.org/auto/criticality_phenomena#CP_14"/>
        <rdfs:subClassOf rdf:resource="http://purl.org/auto/criticality_phenomena#Dynamical_Criticality_Phenomenon"/>
        <dcterms:identifier rdf:datatype="http://www.w3.org/2001/XMLSchema#nonNegativeInteger">321</dcterms:identifier>
        <rdfs:comment xml:lang="en">Refers to 10-minute sustained winds of 52-61 km/h. (According to classifications used by Regional Specialized Meteorological Centers worldwide)</rdfs:comment>
        <rdfs:label xml:lang="en">Moderate gale</rdfs:label>
        <rdfs:label xml:lang="de">Moderater Sturm</rdfs:label>
    </owl:Class>
    


    <!-- http://purl.org/auto/criticality_phenomena#CP_322 -->

    <owl:Class rdf:about="http://purl.org/auto/criticality_phenomena#CP_322">
        <rdfs:subClassOf rdf:resource="http://purl.org/auto/criticality_phenomena#CP_14"/>
        <rdfs:subClassOf rdf:resource="http://purl.org/auto/criticality_phenomena#Dynamical_Criticality_Phenomenon"/>
        <dcterms:identifier rdf:datatype="http://www.w3.org/2001/XMLSchema#nonNegativeInteger">322</dcterms:identifier>
        <rdfs:comment xml:lang="en">Refers to 10-minute sustained winds of 63-74 km/h. (According to classifications used by Regional Specialized Meteorological Centers worldwide)</rdfs:comment>
        <rdfs:label xml:lang="en">Fresh gale</rdfs:label>
        <rdfs:label xml:lang="de">Frischer Sturm</rdfs:label>
    </owl:Class>
    


    <!-- http://purl.org/auto/criticality_phenomena#CP_323 -->

    <owl:Class rdf:about="http://purl.org/auto/criticality_phenomena#CP_323">
        <rdfs:subClassOf rdf:resource="http://purl.org/auto/criticality_phenomena#CP_14"/>
        <rdfs:subClassOf rdf:resource="http://purl.org/auto/criticality_phenomena#Dynamical_Criticality_Phenomenon"/>
        <dcterms:identifier rdf:datatype="http://www.w3.org/2001/XMLSchema#nonNegativeInteger">323</dcterms:identifier>
        <rdfs:comment xml:lang="en">Refers to 10-minute sustained winds of 76-87 km/h. (According to classifications used by Regional Specialized Meteorological Centers worldwide)</rdfs:comment>
        <rdfs:label xml:lang="de">Starker Sturm</rdfs:label>
        <rdfs:label xml:lang="en">Strong gale</rdfs:label>
    </owl:Class>
    


    <!-- http://purl.org/auto/criticality_phenomena#CP_324 -->

    <owl:Class rdf:about="http://purl.org/auto/criticality_phenomena#CP_324">
        <rdfs:subClassOf rdf:resource="http://purl.org/auto/criticality_phenomena#CP_14"/>
        <rdfs:subClassOf rdf:resource="http://purl.org/auto/criticality_phenomena#Dynamical_Criticality_Phenomenon"/>
        <dcterms:identifier rdf:datatype="http://www.w3.org/2001/XMLSchema#nonNegativeInteger">324</dcterms:identifier>
        <rdfs:comment xml:lang="en">Refers to 10-minute sustained winds of 89-102 km/h. (According to classifications used by Regional Specialized Meteorological Centers worldwide)</rdfs:comment>
        <rdfs:label xml:lang="de">Orkan</rdfs:label>
        <rdfs:label xml:lang="en">Whole gale</rdfs:label>
    </owl:Class>
    


    <!-- http://purl.org/auto/criticality_phenomena#CP_325 -->

    <owl:Class rdf:about="http://purl.org/auto/criticality_phenomena#CP_325">
        <rdfs:subClassOf rdf:resource="http://purl.org/auto/criticality_phenomena#CP_14"/>
        <rdfs:subClassOf rdf:resource="http://purl.org/auto/criticality_phenomena#Dynamical_Criticality_Phenomenon"/>
        <dcterms:identifier rdf:datatype="http://www.w3.org/2001/XMLSchema#nonNegativeInteger">325</dcterms:identifier>
        <rdfs:comment xml:lang="en">Refers to 10-minute sustained winds of 104-117 km/h. (According to classifications used by Regional Specialized Meteorological Centers worldwide)</rdfs:comment>
        <rdfs:label xml:lang="en">Storm</rdfs:label>
        <rdfs:label xml:lang="de">Sturm</rdfs:label>
    </owl:Class>
    


    <!-- http://purl.org/auto/criticality_phenomena#CP_326 -->

    <owl:Class rdf:about="http://purl.org/auto/criticality_phenomena#CP_326">
        <rdfs:subClassOf rdf:resource="http://purl.org/auto/criticality_phenomena#CP_14"/>
        <rdfs:subClassOf rdf:resource="http://purl.org/auto/criticality_phenomena#Dynamical_Criticality_Phenomenon"/>
        <dcterms:identifier rdf:datatype="http://www.w3.org/2001/XMLSchema#nonNegativeInteger">326</dcterms:identifier>
        <rdfs:comment xml:lang="en">Refers to 10-minute sustained winds of &gt;119 km/h. (According to classifications used by Regional Specialized Meteorological Centers worldwide)</rdfs:comment>
        <rdfs:label xml:lang="en">Hurricane</rdfs:label>
        <rdfs:label xml:lang="de">Hurrikan</rdfs:label>
    </owl:Class>
    


    <!-- http://purl.org/auto/criticality_phenomena#CP_327 -->

    <owl:Class rdf:about="http://purl.org/auto/criticality_phenomena#CP_327">
        <rdfs:subClassOf rdf:resource="http://purl.org/auto/criticality_phenomena#CP_212"/>
        <dcterms:identifier rdf:datatype="http://www.w3.org/2001/XMLSchema#nonNegativeInteger">327</dcterms:identifier>
        <rdfs:comment xml:lang="en">Vehicle parts on the road. This could make evasion inevitable.</rdfs:comment>
        <rdfs:label xml:lang="de">Fahrzeugteile auf der Straße</rdfs:label>
        <rdfs:label xml:lang="en">Vehicle parts on the road</rdfs:label>
    </owl:Class>
    


    <!-- http://purl.org/auto/criticality_phenomena#CP_328 -->

    <owl:Class rdf:about="http://purl.org/auto/criticality_phenomena#CP_328">
        <rdfs:subClassOf rdf:resource="http://purl.org/auto/criticality_phenomena#CP_164"/>
        <rdfs:subClassOf rdf:resource="http://purl.org/auto/criticality_phenomena#Dynamical_Criticality_Phenomenon"/>
        <dcterms:identifier rdf:datatype="http://www.w3.org/2001/XMLSchema#nonNegativeInteger">328</dcterms:identifier>
        <rdfs:comment xml:lang="en">Impact Force refers to force applied by an other TP.</rdfs:comment>
        <rdfs:label xml:lang="en">Impact Force</rdfs:label>
        <rdfs:label xml:lang="de">Stoßkraft</rdfs:label>
    </owl:Class>
    


    <!-- http://purl.org/auto/criticality_phenomena#CP_329 -->

    <owl:Class rdf:about="http://purl.org/auto/criticality_phenomena#CP_329">
        <rdfs:subClassOf rdf:resource="http://purl.org/auto/criticality_phenomena#CP_328"/>
        <dcterms:identifier rdf:datatype="http://www.w3.org/2001/XMLSchema#nonNegativeInteger">329</dcterms:identifier>
        <rdfs:comment xml:lang="en">Rear-end collision forces the TP in front in driving direktion. Braking might be necessary.</rdfs:comment>
        <rdfs:label xml:lang="de">Auffahrunfall</rdfs:label>
        <rdfs:label xml:lang="en">Rear-end collision</rdfs:label>
    </owl:Class>
    


    <!-- http://purl.org/auto/criticality_phenomena#CP_33 -->

    <owl:Class rdf:about="http://purl.org/auto/criticality_phenomena#CP_33">
        <rdfs:subClassOf rdf:resource="http://purl.org/auto/criticality_phenomena#CP_32"/>
        <rdfs:subClassOf rdf:resource="http://purl.org/auto/criticality_phenomena#Human_Criticality_Phenomenon"/>
        <dcterms:identifier rdf:datatype="http://www.w3.org/2001/XMLSchema#nonNegativeInteger">33</dcterms:identifier>
        <rdfs:comment xml:lang="en">A pedestrian is crossing the road (whether allowed or not).</rdfs:comment>
        <rdfs:label xml:lang="de">Fußgänger überquert Straße auf direktem Weg</rdfs:label>
        <rdfs:label xml:lang="en">Pedestrian Crossing Road Directly</rdfs:label>
    </owl:Class>
    


    <!-- http://purl.org/auto/criticality_phenomena#CP_330 -->

    <owl:Class rdf:about="http://purl.org/auto/criticality_phenomena#CP_330">
        <rdfs:subClassOf rdf:resource="http://purl.org/auto/criticality_phenomena#CP_328"/>
        <dcterms:identifier rdf:datatype="http://www.w3.org/2001/XMLSchema#nonNegativeInteger">330</dcterms:identifier>
        <rdfs:comment xml:lang="en">A ball is kicked or thrown against the windshield. This might affect Sensor capability. The shock sensors could also be affected.</rdfs:comment>
        <rdfs:label xml:lang="en">Ball against windshield</rdfs:label>
        <rdfs:label xml:lang="de">Ball gegen Windschutzscheibe</rdfs:label>
    </owl:Class>
    


    <!-- http://purl.org/auto/criticality_phenomena#CP_331 -->

    <owl:Class rdf:about="http://purl.org/auto/criticality_phenomena#CP_331">
        <rdfs:subClassOf rdf:resource="http://purl.org/auto/criticality_phenomena#Behavioral_Criticality_Phenomenon"/>
        <rdfs:subClassOf rdf:resource="http://purl.org/auto/criticality_phenomena#CP_328"/>
        <rdfs:subClassOf rdf:resource="http://purl.org/auto/criticality_phenomena#Human_Criticality_Phenomenon"/>
        <rdfs:subClassOf rdf:resource="http://purl.org/auto/criticality_phenomena#Unpredictability_Criticality_Phenomenon"/>
        <dcterms:identifier rdf:datatype="http://www.w3.org/2001/XMLSchema#nonNegativeInteger">331</dcterms:identifier>
        <rdfs:comment xml:lang="en">Playing children might push each other onto the road.</rdfs:comment>
        <rdfs:label xml:lang="en">Playing Children</rdfs:label>
        <rdfs:label xml:lang="de">Spielende Kinder</rdfs:label>
    </owl:Class>
    


    <!-- http://purl.org/auto/criticality_phenomena#CP_34 -->

    <owl:Class rdf:about="http://purl.org/auto/criticality_phenomena#CP_34">
        <rdfs:subClassOf rdf:resource="http://purl.org/auto/criticality_phenomena#CP_32"/>
        <rdfs:subClassOf rdf:resource="http://purl.org/auto/criticality_phenomena#Human_Criticality_Phenomenon"/>
        <dcterms:identifier rdf:datatype="http://www.w3.org/2001/XMLSchema#nonNegativeInteger">34</dcterms:identifier>
        <rdfs:comment xml:lang="en">Pedestrian walks onto the road in a unforeseeable manner.</rdfs:comment>
        <rdfs:label xml:lang="de">Fußgänger spaziert willkürlich auf Straße</rdfs:label>
        <rdfs:label xml:lang="en">Pedestrian Walking Randomly On Road</rdfs:label>
    </owl:Class>
    


    <!-- http://purl.org/auto/criticality_phenomena#CP_35 -->

    <owl:Class rdf:about="http://purl.org/auto/criticality_phenomena#CP_35">
        <rdfs:subClassOf rdf:resource="http://purl.org/auto/criticality_phenomena#CP_91"/>
        <dcterms:identifier rdf:datatype="http://www.w3.org/2001/XMLSchema#nonNegativeInteger">35</dcterms:identifier>
        <rdfs:comment xml:lang="en">This includes only temporarily (less than 3 minutes)</rdfs:comment>
        <rdfs:label xml:lang="de">Passieren temporär parkender Fahrzeuge</rdfs:label>
        <rdfs:label xml:lang="en">Passing Of Temporarily Parking Vehicles</rdfs:label>
    </owl:Class>
    


    <!-- http://purl.org/auto/criticality_phenomena#CP_36 -->

    <owl:Class rdf:about="http://purl.org/auto/criticality_phenomena#CP_36">
        <rdfs:subClassOf rdf:resource="http://purl.org/auto/criticality_phenomena#CP_150"/>
        <dcterms:identifier rdf:datatype="http://www.w3.org/2001/XMLSchema#nonNegativeInteger">36</dcterms:identifier>
        <rdfs:comment xml:lang="en">Unsafe distance as defined by RSS to another TP</rdfs:comment>
        <rdfs:label xml:lang="en">Small Distance To TP</rdfs:label>
        <rdfs:label xml:lang="de">geringer Abstand zu Verkehrsteilnehmer</rdfs:label>
    </owl:Class>
    


    <!-- http://purl.org/auto/criticality_phenomena#CP_37 -->

    <owl:Class rdf:about="http://purl.org/auto/criticality_phenomena#CP_37">
        <rdfs:subClassOf rdf:resource="http://purl.org/auto/criticality_phenomena#CP_150"/>
        <dcterms:identifier rdf:datatype="http://www.w3.org/2001/XMLSchema#nonNegativeInteger">37</dcterms:identifier>
        <rdfs:comment xml:lang="en">Unsafe distance as defined by RSS to some lane marking</rdfs:comment>
        <rdfs:label xml:lang="en">Small Distance To Lane Marking</rdfs:label>
        <rdfs:label xml:lang="de">geringer Abstand zu Spurmarkierung</rdfs:label>
    </owl:Class>
    


    <!-- http://purl.org/auto/criticality_phenomena#CP_38 -->

    <owl:Class rdf:about="http://purl.org/auto/criticality_phenomena#CP_38">
        <rdfs:subClassOf rdf:resource="http://purl.org/auto/criticality_phenomena#CP_150"/>
        <dcterms:identifier rdf:datatype="http://www.w3.org/2001/XMLSchema#nonNegativeInteger">38</dcterms:identifier>
        <rdfs:comment xml:lang="en">Unsafe distance as defined by RSS to some road side</rdfs:comment>
        <rdfs:label xml:lang="en">Small Distance To Road Side</rdfs:label>
        <rdfs:label xml:lang="de">geringer Abstand zu Straßenrand</rdfs:label>
    </owl:Class>
    


    <!-- http://purl.org/auto/criticality_phenomena#CP_39 -->

    <owl:Class rdf:about="http://purl.org/auto/criticality_phenomena#CP_39">
        <rdfs:subClassOf rdf:resource="http://purl.org/auto/criticality_phenomena#CP_143"/>
        <rdfs:subClassOf rdf:resource="http://purl.org/auto/criticality_phenomena#Real_Human_Criticality_Phenomenon"/>
        <rdfs:subClassOf rdf:resource="http://purl.org/auto/criticality_phenomena#Real_Perception_Algorithm_Criticality_Phenomenon"/>
        <dcterms:identifier rdf:datatype="http://www.w3.org/2001/XMLSchema#nonNegativeInteger">39</dcterms:identifier>
        <rdfs:comment xml:lang="en">TP has wrongly or not at all interpreted a given signal from either another TP or the traffic infrastructure. It is an abstract phenomeon referring to signals as means of communication.</rdfs:comment>
        <rdfs:label xml:lang="en">(mis/missing)-interpretation Of Signal</rdfs:label>
        <rdfs:label xml:lang="de">Fehlinterpretation eines Signals</rdfs:label>
    </owl:Class>
    


    <!-- http://purl.org/auto/criticality_phenomena#CP_4 -->

    <owl:Class rdf:about="http://purl.org/auto/criticality_phenomena#CP_4">
        <rdfs:subClassOf rdf:resource="http://purl.org/auto/criticality_phenomena#CP_113"/>
        <rdfs:subClassOf rdf:resource="http://purl.org/auto/criticality_phenomena#Complexity_Criticality_Phenomenon"/>
        <rdfs:subClassOf rdf:resource="http://purl.org/auto/criticality_phenomena#Dynamical_Criticality_Phenomenon"/>
        <dcterms:identifier rdf:datatype="http://www.w3.org/2001/XMLSchema#nonNegativeInteger">4</dcterms:identifier>
        <rdfs:comment xml:lang="en">VRU legally crossing the road, but outside of designated areas such as pedestrian crossings, bicycle lanes, etc.</rdfs:comment>
        <rdfs:label xml:lang="de">Unerwartetes aber legitimes Überquerung einer Straße von VRU</rdfs:label>
        <rdfs:label xml:lang="en">Unexpected But Legitimate Crossing Of VRU</rdfs:label>
    </owl:Class>
    


    <!-- http://purl.org/auto/criticality_phenomena#CP_40 -->

    <owl:Class rdf:about="http://purl.org/auto/criticality_phenomena#CP_40">
        <rdfs:subClassOf rdf:resource="http://purl.org/auto/criticality_phenomena#CP_39"/>
        <dcterms:identifier rdf:datatype="http://www.w3.org/2001/XMLSchema#nonNegativeInteger">40</dcterms:identifier>
        <rdfs:comment xml:lang="en">TP has wrongly interpreted an accustic signal, e.g. horns, sirens, ...</rdfs:comment>
        <rdfs:label xml:lang="en">(mis/missing)-interpretation Of Accustic Signal</rdfs:label>
        <rdfs:label xml:lang="de">Fehlinterpretation eines akkustischen Signals</rdfs:label>
    </owl:Class>
    


    <!-- http://purl.org/auto/criticality_phenomena#CP_41 -->

    <owl:Class rdf:about="http://purl.org/auto/criticality_phenomena#CP_41">
        <rdfs:subClassOf rdf:resource="http://purl.org/auto/criticality_phenomena#CP_39"/>
        <rdfs:subClassOf rdf:resource="http://purl.org/auto/criticality_phenomena#Real_Camera_Criticality_Phenomenon"/>
        <rdfs:subClassOf rdf:resource="http://purl.org/auto/criticality_phenomena#Unpredictability_Criticality_Phenomenon"/>
        <dcterms:identifier rdf:datatype="http://www.w3.org/2001/XMLSchema#nonNegativeInteger">41</dcterms:identifier>
        <rdfs:comment xml:lang="en">TP has wrongly interpreted the hand signal of another TP, e.g. yielding right-of-way, policeman regulating traffic manually, ...</rdfs:comment>
        <rdfs:label xml:lang="en">(mis/missing)-interpretation Of Hand Signal</rdfs:label>
        <rdfs:label xml:lang="de">Fehlinterpretation eines Handzeichens</rdfs:label>
    </owl:Class>
    


    <!-- http://purl.org/auto/criticality_phenomena#CP_42 -->

    <owl:Class rdf:about="http://purl.org/auto/criticality_phenomena#CP_42">
        <rdfs:subClassOf rdf:resource="http://purl.org/auto/criticality_phenomena#CP_138"/>
        <dcterms:identifier rdf:datatype="http://www.w3.org/2001/XMLSchema#nonNegativeInteger">42</dcterms:identifier>
        <rdfs:comment xml:lang="en">This includes other TPs driving close to lane markings, road side or in sinuous lines. 
May be interpreted as the effect or distracted/impaired driving.</rdfs:comment>
        <rdfs:label xml:lang="de">Aufällige Trajektorie von Non-Ego-TP</rdfs:label>
        <rdfs:label xml:lang="en">Peculiar Trajectory Of Non-Ego-TP</rdfs:label>
    </owl:Class>
    


    <!-- http://purl.org/auto/criticality_phenomena#CP_43 -->

    <owl:Class rdf:about="http://purl.org/auto/criticality_phenomena#CP_43">
        <rdfs:subClassOf rdf:resource="http://purl.org/auto/criticality_phenomena#CP_18"/>
        <dcterms:identifier rdf:datatype="http://www.w3.org/2001/XMLSchema#nonNegativeInteger">43</dcterms:identifier>
        <rdfs:comment xml:lang="en">Street lights may be too sparsely placed or the lighting may be too weak</rdfs:comment>
        <rdfs:label xml:lang="en">Insufficient/defective Street Light</rdfs:label>
        <rdfs:label xml:lang="de">Unzureichende Straßenbeleuchtung</rdfs:label>
    </owl:Class>
    


    <!-- http://purl.org/auto/criticality_phenomena#CP_44 -->

    <owl:Class rdf:about="http://purl.org/auto/criticality_phenomena#CP_44">
        <rdfs:subClassOf rdf:resource="http://purl.org/auto/criticality_phenomena#CP_211"/>
        <rdfs:subClassOf rdf:resource="http://purl.org/auto/criticality_phenomena#Perfect_Perception_Criticality_Phenomenon"/>
        <dcterms:identifier rdf:datatype="http://www.w3.org/2001/XMLSchema#nonNegativeInteger">44</dcterms:identifier>
        <rdfs:comment xml:lang="en">When the official traffic sign does not fit the traffic reality, e.g. inappropriate speed limit</rdfs:comment>
        <rdfs:label xml:lang="en">Inappropriate Traffic Sign</rdfs:label>
        <rdfs:label xml:lang="de">Unpassendes Verkehrszeichen</rdfs:label>
    </owl:Class>
    


    <!-- http://purl.org/auto/criticality_phenomena#CP_45 -->

    <owl:Class rdf:about="http://purl.org/auto/criticality_phenomena#CP_45">
        <rdfs:subClassOf rdf:resource="http://purl.org/auto/criticality_phenomena#CP_162"/>
        <rdfs:subClassOf rdf:resource="http://purl.org/auto/criticality_phenomena#Dynamical_Criticality_Phenomenon"/>
        <rdfs:subClassOf rdf:resource="http://purl.org/auto/criticality_phenomena#Perfect_Perception_Criticality_Phenomenon"/>
        <dcterms:identifier rdf:datatype="http://www.w3.org/2001/XMLSchema#nonNegativeInteger">45</dcterms:identifier>
        <rdfs:comment xml:lang="en">If a road leads over the top of a hill, vision into progression of road or other arms of an intersection can be potentially obstructed.</rdfs:comment>
        <rdfs:label xml:lang="de">Kuppe eines Hügels</rdfs:label>
        <rdfs:label xml:lang="en">Summit Of Hill</rdfs:label>
    </owl:Class>
    


    <!-- http://purl.org/auto/criticality_phenomena#CP_46 -->

    <owl:Class rdf:about="http://purl.org/auto/criticality_phenomena#CP_46">
        <rdfs:subClassOf rdf:resource="http://purl.org/auto/criticality_phenomena#CP_209"/>
        <rdfs:subClassOf rdf:resource="http://purl.org/auto/criticality_phenomena#Perfect_Perception_Criticality_Phenomenon"/>
        <dcterms:identifier rdf:datatype="http://www.w3.org/2001/XMLSchema#nonNegativeInteger">46</dcterms:identifier>
        <rdfs:comment xml:lang="en">When official lane markings (white or yellow) are placed inappropriately, i.e. their meaning is not consistent with the actual situation.</rdfs:comment>
        <rdfs:label xml:lang="en">Inappropriate Lane Markings</rdfs:label>
        <rdfs:label xml:lang="de">Unpassende Fahrstreifenmarkierungen</rdfs:label>
    </owl:Class>
    


    <!-- http://purl.org/auto/criticality_phenomena#CP_47 -->

    <owl:Class rdf:about="http://purl.org/auto/criticality_phenomena#CP_47">
        <rdfs:subClassOf rdf:resource="http://purl.org/auto/criticality_phenomena#CP_143"/>
        <rdfs:subClassOf rdf:resource="http://purl.org/auto/criticality_phenomena#CP_275"/>
        <dcterms:identifier rdf:datatype="http://www.w3.org/2001/XMLSchema#nonNegativeInteger">47</dcterms:identifier>
        <rdfs:comment xml:lang="en">This refers to vehicles carrying either insecure load or are overloaded</rdfs:comment>
        <rdfs:label xml:lang="en">Dangerous Load Of Non-Ego-TP</rdfs:label>
        <rdfs:label xml:lang="de">Gefährliche Beladung eines Non-Ego-TP</rdfs:label>
    </owl:Class>
    


    <!-- http://purl.org/auto/criticality_phenomena#CP_48 -->

    <owl:Class rdf:about="http://purl.org/auto/criticality_phenomena#CP_48">
        <rdfs:subClassOf rdf:resource="http://purl.org/auto/criticality_phenomena#CP_216"/>
        <rdfs:subClassOf rdf:resource="http://purl.org/auto/criticality_phenomena#Perfect_Perception_Criticality_Phenomenon"/>
        <dcterms:identifier rdf:datatype="http://www.w3.org/2001/XMLSchema#nonNegativeInteger">48</dcterms:identifier>
        <rdfs:comment xml:lang="en">Unexpected steering of ego or non-ego-TPs refers to braking maneuvers that cannot be anticipated by other TPs or ego from the learned norm behavior of traffic participants (hard to quantify).</rdfs:comment>
        <rdfs:label xml:lang="en">Unexpected Steering Maneuver Of Ego/non-ego-tp</rdfs:label>
        <rdfs:label xml:lang="de">unerwartetes Lenkmanöver von Ego/Non-Ego-TP</rdfs:label>
    </owl:Class>
    


    <!-- http://purl.org/auto/criticality_phenomena#CP_49 -->

    <owl:Class rdf:about="http://purl.org/auto/criticality_phenomena#CP_49">
        <rdfs:subClassOf rdf:resource="http://purl.org/auto/criticality_phenomena#CP_113"/>
        <dcterms:identifier rdf:datatype="http://www.w3.org/2001/XMLSchema#nonNegativeInteger">49</dcterms:identifier>
        <rdfs:comment xml:lang="en">A parking vehicle is being (un)loaded by some operator, e.g. a delivery service.</rdfs:comment>
        <rdfs:label xml:lang="de">Be/-entladen eines parkenden Fahrzeugs</rdfs:label>
        <rdfs:label xml:lang="en">Loading/unloading Of Parking Vehicle (by VRUs)</rdfs:label>
    </owl:Class>
    


    <!-- http://purl.org/auto/criticality_phenomena#CP_5 -->

    <owl:Class rdf:about="http://purl.org/auto/criticality_phenomena#CP_5">
        <rdfs:subClassOf rdf:resource="http://purl.org/auto/criticality_phenomena#CP_212"/>
        <rdfs:subClassOf rdf:resource="http://purl.org/auto/criticality_phenomena#Environmental_Criticality_Phenomenon"/>
        <rdfs:subClassOf rdf:resource="http://purl.org/auto/criticality_phenomena#Perfect_Perception_Criticality_Phenomenon"/>
        <dcterms:identifier rdf:datatype="http://www.w3.org/2001/XMLSchema#nonNegativeInteger">5</dcterms:identifier>
        <rdfs:comment xml:lang="en">A pile of snow (meaning a deviation in height of more than 10cm) that may or may not be overridable. Can be compacted, but also loosely packed snow.</rdfs:comment>
        <rdfs:label xml:lang="en">Pile Of Snow On Road</rdfs:label>
        <rdfs:label xml:lang="de">Schneehaufen auf der Straße</rdfs:label>
    </owl:Class>
    


    <!-- http://purl.org/auto/criticality_phenomena#CP_50 -->

    <owl:Class rdf:about="http://purl.org/auto/criticality_phenomena#CP_50">
        <rdfs:subClassOf rdf:resource="http://purl.org/auto/criticality_phenomena#CP_216"/>
        <rdfs:subClassOf rdf:resource="http://purl.org/auto/criticality_phenomena#Perfect_Perception_Criticality_Phenomenon"/>
        <dcterms:identifier rdf:datatype="http://www.w3.org/2001/XMLSchema#nonNegativeInteger">50</dcterms:identifier>
        <rdfs:comment xml:lang="en">A TP is parking or stopping its vehicle on the road in places where such behavior is not allowed.</rdfs:comment>
        <rdfs:label xml:lang="en">Illegitimate Stopping Or Parking Vehicle</rdfs:label>
        <rdfs:label xml:lang="de">illegales Anhalten oder Parken eines Fahrzeugs</rdfs:label>
    </owl:Class>
    


    <!-- http://purl.org/auto/criticality_phenomena#CP_51 -->

    <owl:Class rdf:about="http://purl.org/auto/criticality_phenomena#CP_51">
        <rdfs:subClassOf rdf:resource="http://purl.org/auto/criticality_phenomena#CP_113"/>
        <rdfs:subClassOf rdf:resource="http://purl.org/auto/criticality_phenomena#CP_195"/>
        <rdfs:subClassOf rdf:resource="http://purl.org/auto/criticality_phenomena#CP_197"/>
        <dcterms:identifier rdf:datatype="http://www.w3.org/2001/XMLSchema#nonNegativeInteger">51</dcterms:identifier>
        <rdfs:comment xml:lang="en">VRU in dark clothing are generally harder to perceive, especially in bad lighting conditions</rdfs:comment>
        <rdfs:label xml:lang="en">Dark Clothing Of VRU</rdfs:label>
        <rdfs:label xml:lang="de">Dunkle Kleidung von VRU</rdfs:label>
    </owl:Class>
    


    <!-- http://purl.org/auto/criticality_phenomena#CP_52 -->

    <owl:Class rdf:about="http://purl.org/auto/criticality_phenomena#CP_52">
        <rdfs:subClassOf rdf:resource="http://purl.org/auto/criticality_phenomena#CP_195"/>
        <rdfs:subClassOf rdf:resource="http://purl.org/auto/criticality_phenomena#Perfect_Camera_Criticality_Phenomenon"/>
        <rdfs:subClassOf rdf:resource="http://purl.org/auto/criticality_phenomena#Perfect_Human_Criticality_Phenomenon"/>
        <rdfs:subClassOf rdf:resource="http://purl.org/auto/criticality_phenomena#Perfect_Lidar_Criticality_Phenomenon"/>
        <rdfs:subClassOf rdf:resource="http://purl.org/auto/criticality_phenomena#Perfect_Radar_Criticality_Phenomenon"/>
        <dcterms:identifier rdf:datatype="http://www.w3.org/2001/XMLSchema#nonNegativeInteger">52</dcterms:identifier>
        <rdfs:comment xml:lang="en">In densely built urban areas e.g. due to walls, buildings, billboards etc.</rdfs:comment>
        <rdfs:label xml:lang="en">Permanent Obstruction Of View</rdfs:label>
        <rdfs:label xml:lang="de">Permanente Sichtverhinderung</rdfs:label>
    </owl:Class>
    


    <!-- http://purl.org/auto/criticality_phenomena#CP_53 -->

    <owl:Class rdf:about="http://purl.org/auto/criticality_phenomena#CP_53">
        <rdfs:subClassOf rdf:resource="http://purl.org/auto/criticality_phenomena#CP_142"/>
        <dcterms:identifier rdf:datatype="http://www.w3.org/2001/XMLSchema#nonNegativeInteger">53</dcterms:identifier>
        <rdfs:comment xml:lang="en">Violating the driving direction of the lane, e.g. by ignoring obligations to drive on the right or 
bicyclist illegaly driving on unidirectional road</rdfs:comment>
        <rdfs:label xml:lang="en">Non-Ego-TP On Wrong Driveable Lane</rdfs:label>
        <rdfs:label xml:lang="de">Non-Ego-TP benutzt falsche, befahrbare Fahrbahn</rdfs:label>
    </owl:Class>
    


    <!-- http://purl.org/auto/criticality_phenomena#CP_54 -->

    <owl:Class rdf:about="http://purl.org/auto/criticality_phenomena#CP_54">
        <rdfs:subClassOf rdf:resource="http://purl.org/auto/criticality_phenomena#Behavioral_Criticality_Phenomenon"/>
        <rdfs:subClassOf rdf:resource="http://purl.org/auto/criticality_phenomena#CP_279"/>
        <rdfs:subClassOf rdf:resource="http://purl.org/auto/criticality_phenomena#Perfect_Perception_Criticality_Phenomenon"/>
        <dcterms:identifier rdf:datatype="http://www.w3.org/2001/XMLSchema#nonNegativeInteger">54</dcterms:identifier>
        <rdfs:comment xml:lang="en">Abstract phenomenon describing any kind of overtaking maneuver.</rdfs:comment>
        <rdfs:label xml:lang="en">Overtaking</rdfs:label>
        <rdfs:label xml:lang="de">Überholen</rdfs:label>
    </owl:Class>
    


    <!-- http://purl.org/auto/criticality_phenomena#CP_55 -->

    <owl:Class rdf:about="http://purl.org/auto/criticality_phenomena#CP_55">
        <rdfs:subClassOf rdf:resource="http://purl.org/auto/criticality_phenomena#CP_142"/>
        <dcterms:identifier rdf:datatype="http://www.w3.org/2001/XMLSchema#nonNegativeInteger">55</dcterms:identifier>
        <rdfs:comment xml:lang="en">E.g. Bicyclist in wrong direction on bicycle lane.</rdfs:comment>
        <rdfs:label xml:lang="en">Non-Ego-TP Illegitimately Using Lane</rdfs:label>
        <rdfs:label xml:lang="de">Non-Ego-TP nutzt unzulässige Fahrbahn</rdfs:label>
    </owl:Class>
    


    <!-- http://purl.org/auto/criticality_phenomena#CP_56 -->

    <owl:Class rdf:about="http://purl.org/auto/criticality_phenomena#CP_56">
        <rdfs:subClassOf rdf:resource="http://purl.org/auto/criticality_phenomena#CP_234"/>
        <rdfs:subClassOf rdf:resource="http://purl.org/auto/criticality_phenomena#Real_Camera_Criticality_Phenomenon"/>
        <rdfs:subClassOf rdf:resource="http://purl.org/auto/criticality_phenomena#Real_Human_Criticality_Phenomenon"/>
        <rdfs:subClassOf rdf:resource="http://purl.org/auto/criticality_phenomena#Real_Perception_Algorithm_Criticality_Phenomenon"/>
        <dcterms:identifier rdf:datatype="http://www.w3.org/2001/XMLSchema#nonNegativeInteger">56</dcterms:identifier>
        <rdfs:comment xml:lang="en">Glare from any direct or indirect illumination source as an abstract phenomenon.</rdfs:comment>
        <rdfs:label xml:lang="de">Blendung</rdfs:label>
        <rdfs:label xml:lang="en">Glare</rdfs:label>
    </owl:Class>
    


    <!-- http://purl.org/auto/criticality_phenomena#CP_57 -->

    <owl:Class rdf:about="http://purl.org/auto/criticality_phenomena#CP_57">
        <rdfs:subClassOf rdf:resource="http://purl.org/auto/criticality_phenomena#CP_211"/>
        <rdfs:subClassOf rdf:resource="http://purl.org/auto/criticality_phenomena#Perfect_Perception_Criticality_Phenomenon"/>
        <dcterms:identifier rdf:datatype="http://www.w3.org/2001/XMLSchema#nonNegativeInteger">57</dcterms:identifier>
        <rdfs:comment xml:lang="en">Traffic sign that was supposed to be there, but is missing e.g. due to vandalism or storms. Criticality depends on traffic sign</rdfs:comment>
        <rdfs:label xml:lang="en">Missing Traffic Sign</rdfs:label>
        <rdfs:label xml:lang="de">fehlendes Verkehrszeichen</rdfs:label>
    </owl:Class>
    


    <!-- http://purl.org/auto/criticality_phenomena#CP_58 -->

    <owl:Class rdf:about="http://purl.org/auto/criticality_phenomena#CP_58">
        <rdfs:subClassOf rdf:resource="http://purl.org/auto/criticality_phenomena#CP_178"/>
        <dcterms:identifier rdf:datatype="http://www.w3.org/2001/XMLSchema#nonNegativeInteger">58</dcterms:identifier>
        <rdfs:comment xml:lang="en">The scenario contains a railroad crossing (protected or unprotected).</rdfs:comment>
        <rdfs:label xml:lang="en">Railroad Crossing</rdfs:label>
        <rdfs:label xml:lang="de">kreuzender Bahnübergang</rdfs:label>
    </owl:Class>
    


    <!-- http://purl.org/auto/criticality_phenomena#CP_59 -->

    <owl:Class rdf:about="http://purl.org/auto/criticality_phenomena#CP_59">
        <rdfs:subClassOf rdf:resource="http://purl.org/auto/criticality_phenomena#CP_222"/>
        <rdfs:subClassOf rdf:resource="http://purl.org/auto/criticality_phenomena#Perfect_Human_Criticality_Phenomenon"/>
        <dcterms:identifier rdf:datatype="http://www.w3.org/2001/XMLSchema#nonNegativeInteger">59</dcterms:identifier>
        <rdfs:comment xml:lang="en">Area around the vehicle where the driver (or AD system) has no perception due to the spatial properties and construction of the vehicle.</rdfs:comment>
        <rdfs:label xml:lang="en">Blind Spot</rdfs:label>
        <rdfs:label xml:lang="de">toter Winkel</rdfs:label>
    </owl:Class>
    


    <!-- http://purl.org/auto/criticality_phenomena#CP_6 -->

    <owl:Class rdf:about="http://purl.org/auto/criticality_phenomena#CP_6">
        <rdfs:subClassOf rdf:resource="http://purl.org/auto/criticality_phenomena#CP_212"/>
        <rdfs:subClassOf rdf:resource="http://purl.org/auto/criticality_phenomena#Environmental_Criticality_Phenomenon"/>
        <rdfs:subClassOf rdf:resource="http://purl.org/auto/criticality_phenomena#Perfect_Perception_Criticality_Phenomenon"/>
        <dcterms:identifier rdf:datatype="http://www.w3.org/2001/XMLSchema#nonNegativeInteger">6</dcterms:identifier>
        <rdfs:comment xml:lang="en">A pile of leaves (meaning a deviation in height of more than 10cm) on the road.</rdfs:comment>
        <rdfs:label xml:lang="de">Laubhaufen auf der Straße</rdfs:label>
        <rdfs:label xml:lang="en">Pile Of Leaves On Road</rdfs:label>
    </owl:Class>
    


    <!-- http://purl.org/auto/criticality_phenomena#CP_60 -->

    <owl:Class rdf:about="http://purl.org/auto/criticality_phenomena#CP_60">
        <rdfs:subClassOf rdf:resource="http://purl.org/auto/criticality_phenomena#CP_12"/>
        <dcterms:identifier rdf:datatype="http://www.w3.org/2001/XMLSchema#nonNegativeInteger">60</dcterms:identifier>
        <rdfs:comment xml:lang="en">A road is covered with a layer of snow. In addition to reducing road friction, this increases the likelihood of a layer of ice under the snow layer and, above a certain thickness, impedes driving behavior.</rdfs:comment>
        <rdfs:label xml:lang="de">Schneebedeckte Straße</rdfs:label>
        <rdfs:label xml:lang="en">Snowy Road</rdfs:label>
    </owl:Class>
    


    <!-- http://purl.org/auto/criticality_phenomena#CP_61 -->

    <owl:Class rdf:about="http://purl.org/auto/criticality_phenomena#CP_61">
        <rdfs:subClassOf rdf:resource="http://purl.org/auto/criticality_phenomena#CP_274"/>
        <rdfs:subClassOf rdf:resource="http://purl.org/auto/criticality_phenomena#Dynamical_Criticality_Phenomenon"/>
        <dcterms:identifier rdf:datatype="http://www.w3.org/2001/XMLSchema#nonNegativeInteger">61</dcterms:identifier>
        <rdfs:comment xml:lang="en">Spray is a whitish mixture of water and air that occurs when the water of natural or artificial bodies of water is agitated by mechanical action. Spray near roadways can affect sensors (e.g., by reflecting and deflecting light through the water droplets).</rdfs:comment>
        <rdfs:label xml:lang="de">Gischt</rdfs:label>
        <rdfs:label xml:lang="en">Spray</rdfs:label>
    </owl:Class>
    


    <!-- http://purl.org/auto/criticality_phenomena#CP_62 -->

    <owl:Class rdf:about="http://purl.org/auto/criticality_phenomena#CP_62">
        <rdfs:subClassOf rdf:resource="http://purl.org/auto/criticality_phenomena#CP_208"/>
        <rdfs:subClassOf rdf:resource="http://purl.org/auto/criticality_phenomena#Perfect_Perception_Criticality_Phenomenon"/>
        <dcterms:identifier rdf:datatype="http://www.w3.org/2001/XMLSchema#nonNegativeInteger">62</dcterms:identifier>
        <rdfs:comment xml:lang="en">Rails (e.g. from a tram) are sticking out from the drivable road space.</rdfs:comment>
        <rdfs:label xml:lang="en">Sticking Out Rails On Road</rdfs:label>
        <rdfs:label xml:lang="de">herausragende Schienen auf der Straße</rdfs:label>
    </owl:Class>
    


    <!-- http://purl.org/auto/criticality_phenomena#CP_63 -->

    <owl:Class rdf:about="http://purl.org/auto/criticality_phenomena#CP_63">
        <rdfs:subClassOf rdf:resource="http://purl.org/auto/criticality_phenomena#CP_208"/>
        <rdfs:subClassOf rdf:resource="http://purl.org/auto/criticality_phenomena#Perfect_Perception_Criticality_Phenomenon"/>
        <dcterms:identifier rdf:datatype="http://www.w3.org/2001/XMLSchema#nonNegativeInteger">63</dcterms:identifier>
        <rdfs:comment xml:lang="en">A lane is closed for traffic, e.g. due to construction site, road structure, flooding, trees, ...</rdfs:comment>
        <rdfs:label xml:lang="en">Lane Closure</rdfs:label>
        <rdfs:label xml:lang="de">Sperrung eines Fahrstreifens</rdfs:label>
    </owl:Class>
    


    <!-- http://purl.org/auto/criticality_phenomena#CP_64 -->

    <owl:Class rdf:about="http://purl.org/auto/criticality_phenomena#CP_64">
        <rdfs:subClassOf rdf:resource="http://purl.org/auto/criticality_phenomena#CP_209"/>
        <rdfs:subClassOf rdf:resource="http://purl.org/auto/criticality_phenomena#Perfect_Perception_Criticality_Phenomenon"/>
        <dcterms:identifier rdf:datatype="http://www.w3.org/2001/XMLSchema#nonNegativeInteger">64</dcterms:identifier>
        <rdfs:comment xml:lang="en">A lane marking in which pieces are missing, colors are deviated, etc.</rdfs:comment>
        <rdfs:label xml:lang="en">Degraded Lane Markings</rdfs:label>
        <rdfs:label xml:lang="de">verschlechterte Fahrstreifenmarkierungen</rdfs:label>
    </owl:Class>
    


    <!-- http://purl.org/auto/criticality_phenomena#CP_65 -->

    <owl:Class rdf:about="http://purl.org/auto/criticality_phenomena#CP_65">
        <rdfs:subClassOf rdf:resource="http://purl.org/auto/criticality_phenomena#CP_208"/>
        <rdfs:subClassOf rdf:resource="http://purl.org/auto/criticality_phenomena#Perfect_Perception_Criticality_Phenomenon"/>
        <dcterms:identifier rdf:datatype="http://www.w3.org/2001/XMLSchema#nonNegativeInteger">65</dcterms:identifier>
        <rdfs:comment xml:lang="en">A lane with width &lt; 2m. E.g. old roads, construction sites, serpentines</rdfs:comment>
        <rdfs:label xml:lang="en">Small Lane Width</rdfs:label>
        <rdfs:label xml:lang="de">geringe Fahrspurbreite</rdfs:label>
    </owl:Class>
    


    <!-- http://purl.org/auto/criticality_phenomena#CP_66 -->

    <owl:Class rdf:about="http://purl.org/auto/criticality_phenomena#CP_66">
        <rdfs:subClassOf rdf:resource="http://purl.org/auto/criticality_phenomena#Behavioral_Criticality_Phenomenon"/>
        <rdfs:subClassOf rdf:resource="http://purl.org/auto/criticality_phenomena#CP_162"/>
        <rdfs:subClassOf rdf:resource="http://purl.org/auto/criticality_phenomena#Perfect_Perception_Criticality_Phenomenon"/>
        <rdfs:subClassOf rdf:resource="http://purl.org/auto/criticality_phenomena#Spatial_Criticality_Phenomenon"/>
        <dcterms:identifier rdf:datatype="http://www.w3.org/2001/XMLSchema#nonNegativeInteger">66</dcterms:identifier>
        <rdfs:comment xml:lang="en">This phenomenon refers to the legal situation, e.g. old roads, driveways, oncoming bicyclists</rdfs:comment>
        <rdfs:label xml:lang="de">Einbahnstraße mit Verkehr in beiden Richtungen</rdfs:label>
        <rdfs:label xml:lang="en">One-way Street With Two-way Traffic</rdfs:label>
    </owl:Class>
    


    <!-- http://purl.org/auto/criticality_phenomena#CP_67 -->

    <owl:Class rdf:about="http://purl.org/auto/criticality_phenomena#CP_67">
        <rdfs:subClassOf rdf:resource="http://purl.org/auto/criticality_phenomena#CP_245"/>
        <rdfs:subClassOf rdf:resource="http://purl.org/auto/criticality_phenomena#Perfect_Perception_Criticality_Phenomenon"/>
        <rdfs:subClassOf rdf:resource="http://purl.org/auto/criticality_phenomena#Spatial_Criticality_Phenomenon"/>
        <dcterms:identifier rdf:datatype="http://www.w3.org/2001/XMLSchema#nonNegativeInteger">67</dcterms:identifier>
        <rdfs:comment xml:lang="en">Existence of a tunnel in the scenario, leads to particular driving/perception conditions.</rdfs:comment>
        <rdfs:label xml:lang="de">Tunnel</rdfs:label>
        <rdfs:label xml:lang="en">Tunnel</rdfs:label>
    </owl:Class>
    


    <!-- http://purl.org/auto/criticality_phenomena#CP_68 -->

    <owl:Class rdf:about="http://purl.org/auto/criticality_phenomena#CP_68">
        <rdfs:subClassOf rdf:resource="http://purl.org/auto/criticality_phenomena#CP_208"/>
        <rdfs:subClassOf rdf:resource="http://purl.org/auto/criticality_phenomena#Perfect_Perception_Criticality_Phenomenon"/>
        <dcterms:identifier rdf:datatype="http://www.w3.org/2001/XMLSchema#nonNegativeInteger">68</dcterms:identifier>
        <rdfs:comment xml:lang="en">Pollution such as oil spill, shippings, dirt, mud, gravel, leaves, clay etc. on the road surface.</rdfs:comment>
        <rdfs:label xml:lang="en">Polluted Road Surface</rdfs:label>
        <rdfs:label xml:lang="de">verschmutzte Straßenoberfläche</rdfs:label>
    </owl:Class>
    


    <!-- http://purl.org/auto/criticality_phenomena#CP_69 -->

    <owl:Class rdf:about="http://purl.org/auto/criticality_phenomena#CP_69">
        <rdfs:subClassOf rdf:resource="http://purl.org/auto/criticality_phenomena#CP_142"/>
        <rdfs:subClassOf rdf:resource="http://purl.org/auto/criticality_phenomena#Human_Criticality_Phenomenon"/>
        <formalized rdf:datatype="http://www.w3.org/2001/XMLSchema#boolean">true</formalized>
        <dcterms:identifier rdf:datatype="http://www.w3.org/2001/XMLSchema#nonNegativeInteger">69</dcterms:identifier>
        <rdfs:comment xml:lang="en">A non-pedestrian TP uses a pedestrian crossing. In particular, not dismounting of bicyclists, E-bikes, mobility-scooter, e-scooter, skateboards etc. before use the pedestrian crossing.</rdfs:comment>
        <rdfs:label xml:lang="en">Illegitimate Use of Pedestrian Crossing</rdfs:label>
        <rdfs:label xml:lang="de">Illegitime Benutzung von Fußgängerüberwegen</rdfs:label>
    </owl:Class>
    


    <!-- http://purl.org/auto/criticality_phenomena#CP_7 -->

    <owl:Class rdf:about="http://purl.org/auto/criticality_phenomena#CP_7">
        <rdfs:subClassOf rdf:resource="http://purl.org/auto/criticality_phenomena#CP_212"/>
        <rdfs:subClassOf rdf:resource="http://purl.org/auto/criticality_phenomena#Human_Criticality_Phenomenon"/>
        <rdfs:subClassOf rdf:resource="http://purl.org/auto/criticality_phenomena#Perfect_Perception_Criticality_Phenomenon"/>
        <rdfs:subClassOf rdf:resource="http://purl.org/auto/criticality_phenomena#Unpredictability_Criticality_Phenomenon"/>
        <dcterms:identifier rdf:datatype="http://www.w3.org/2001/XMLSchema#nonNegativeInteger">7</dcterms:identifier>
        <rdfs:comment xml:lang="en">A ball is present on the road (can be still, but also be moving). May indiciate playing children near road.</rdfs:comment>
        <rdfs:label xml:lang="en">Ball On Road</rdfs:label>
        <rdfs:label xml:lang="de">Ball auf der Straße</rdfs:label>
    </owl:Class>
    


    <!-- http://purl.org/auto/criticality_phenomena#CP_70 -->

    <owl:Class rdf:about="http://purl.org/auto/criticality_phenomena#CP_70">
        <rdfs:subClassOf rdf:resource="http://purl.org/auto/criticality_phenomena#CP_211"/>
        <rdfs:subClassOf rdf:resource="http://purl.org/auto/criticality_phenomena#Perfect_Perception_Criticality_Phenomenon"/>
        <dcterms:identifier rdf:datatype="http://www.w3.org/2001/XMLSchema#nonNegativeInteger">70</dcterms:identifier>
        <rdfs:comment xml:lang="en">Any sign that was not officially authorized (but may be legetimate) such as fake signs but also additional warning signs by local residents. Criticality depends on traffic sign; e.g. &apos;Slow Down, Children Playing&apos;</rdfs:comment>
        <rdfs:label xml:lang="en">Unofficial Traffic Sign</rdfs:label>
        <rdfs:label xml:lang="de">inoffizielles Verkehrszeichen</rdfs:label>
    </owl:Class>
    


    <!-- http://purl.org/auto/criticality_phenomena#CP_71 -->

    <owl:Class rdf:about="http://purl.org/auto/criticality_phenomena#CP_71">
        <rdfs:subClassOf rdf:resource="http://purl.org/auto/criticality_phenomena#CP_72"/>
        <dcterms:identifier rdf:datatype="http://www.w3.org/2001/XMLSchema#nonNegativeInteger">71</dcterms:identifier>
        <rdfs:comment xml:lang="en">An official traffic sign that has been altered maliciously. Criticality depends on traffic sign</rdfs:comment>
        <rdfs:label xml:lang="en">Vandalized Traffic Sign</rdfs:label>
        <rdfs:label xml:lang="de">beschädigtes Verkehrszeichen</rdfs:label>
    </owl:Class>
    


    <!-- http://purl.org/auto/criticality_phenomena#CP_72 -->

    <owl:Class rdf:about="http://purl.org/auto/criticality_phenomena#CP_72">
        <rdfs:subClassOf rdf:resource="http://purl.org/auto/criticality_phenomena#CP_276"/>
        <rdfs:subClassOf rdf:resource="http://purl.org/auto/criticality_phenomena#Dynamical_Criticality_Phenomenon"/>
        <rdfs:subClassOf rdf:resource="http://purl.org/auto/criticality_phenomena#Real_Camera_Criticality_Phenomenon"/>
        <rdfs:subClassOf rdf:resource="http://purl.org/auto/criticality_phenomena#Real_Human_Criticality_Phenomenon"/>
        <rdfs:subClassOf rdf:resource="http://purl.org/auto/criticality_phenomena#Real_Perception_Algorithm_Criticality_Phenomenon"/>
        <dcterms:identifier rdf:datatype="http://www.w3.org/2001/XMLSchema#nonNegativeInteger">72</dcterms:identifier>
        <rdfs:comment xml:lang="en">Traffic infrastructure that has been altered maliciously. Criticality depends on damage/infrastructure</rdfs:comment>
        <rdfs:label xml:lang="en">Vandalized Infrastructure</rdfs:label>
        <rdfs:label xml:lang="de">beschädigte Infrastruktur</rdfs:label>
    </owl:Class>
    


    <!-- http://purl.org/auto/criticality_phenomena#CP_73 -->

    <owl:Class rdf:about="http://purl.org/auto/criticality_phenomena#CP_73">
        <rdfs:subClassOf rdf:resource="http://purl.org/auto/criticality_phenomena#CP_211"/>
        <rdfs:subClassOf rdf:resource="http://purl.org/auto/criticality_phenomena#Perfect_Perception_Criticality_Phenomenon"/>
        <dcterms:identifier rdf:datatype="http://www.w3.org/2001/XMLSchema#nonNegativeInteger">73</dcterms:identifier>
        <rdfs:comment xml:lang="en">A falsely or non operating traffic light.</rdfs:comment>
        <rdfs:label xml:lang="en">Defective/suspended Traffic Light</rdfs:label>
        <rdfs:label xml:lang="de">defekte oder außer Betrieb befindliche LSA</rdfs:label>
    </owl:Class>
    


    <!-- http://purl.org/auto/criticality_phenomena#CP_74 -->

    <owl:Class rdf:about="http://purl.org/auto/criticality_phenomena#CP_74">
        <rdfs:subClassOf rdf:resource="http://purl.org/auto/criticality_phenomena#CP_208"/>
        <rdfs:subClassOf rdf:resource="http://purl.org/auto/criticality_phenomena#Perfect_Perception_Criticality_Phenomenon"/>
        <dcterms:identifier rdf:datatype="http://www.w3.org/2001/XMLSchema#nonNegativeInteger">74</dcterms:identifier>
        <rdfs:comment xml:lang="en">Remains of infrastructure or objects belonging to an already abandoned construction site, e.g. temporary traffic signs, yellow lane markings, pylons, ...</rdfs:comment>
        <rdfs:label xml:lang="de">Baustellenrückstände</rdfs:label>
        <rdfs:label xml:lang="en">Construction Site Remains</rdfs:label>
    </owl:Class>
    


    <!-- http://purl.org/auto/criticality_phenomena#CP_75 -->

    <owl:Class rdf:about="http://purl.org/auto/criticality_phenomena#CP_75">
        <rdfs:subClassOf rdf:resource="http://purl.org/auto/criticality_phenomena#CP_65"/>
        <dcterms:identifier rdf:datatype="http://www.w3.org/2001/XMLSchema#nonNegativeInteger">75</dcterms:identifier>
        <rdfs:comment xml:lang="en">A construction site modifies the road passage such that the lane becomes small (&lt;2m).</rdfs:comment>
        <rdfs:label xml:lang="en">Narrow Construction Site Passage</rdfs:label>
        <rdfs:label xml:lang="de">schmale Baustellen-Passage</rdfs:label>
    </owl:Class>
    


    <!-- http://purl.org/auto/criticality_phenomena#CP_76 -->

    <owl:Class rdf:about="http://purl.org/auto/criticality_phenomena#CP_76">
        <rdfs:subClassOf rdf:resource="http://purl.org/auto/criticality_phenomena#CP_208"/>
        <rdfs:subClassOf rdf:resource="http://purl.org/auto/criticality_phenomena#Perfect_Perception_Criticality_Phenomenon"/>
        <dcterms:identifier rdf:datatype="http://www.w3.org/2001/XMLSchema#nonNegativeInteger">76</dcterms:identifier>
        <rdfs:comment xml:lang="en">Redirection on opposite lane due to construction site, may be regulated through a traffic light.</rdfs:comment>
        <rdfs:label xml:lang="en">Temporary Opposite Lane</rdfs:label>
        <rdfs:label xml:lang="de">temporäre Nutzung des Gegenfahrstreifens</rdfs:label>
    </owl:Class>
    


    <!-- http://purl.org/auto/criticality_phenomena#CP_77 -->

    <owl:Class rdf:about="http://purl.org/auto/criticality_phenomena#CP_77">
        <rdfs:subClassOf rdf:resource="http://purl.org/auto/criticality_phenomena#Behavioral_Criticality_Phenomenon"/>
        <rdfs:subClassOf rdf:resource="http://purl.org/auto/criticality_phenomena#Criticality_Phenomenon"/>
        <rdfs:subClassOf rdf:resource="http://purl.org/auto/criticality_phenomena#Human_Criticality_Phenomenon"/>
        <rdfs:subClassOf rdf:resource="http://purl.org/auto/criticality_phenomena#Perfect_Perception_Criticality_Phenomenon"/>
        <rdfs:subClassOf rdf:resource="http://purl.org/auto/criticality_phenomena#Unpredictability_Criticality_Phenomenon"/>
        <dcterms:identifier rdf:datatype="http://www.w3.org/2001/XMLSchema#nonNegativeInteger">77</dcterms:identifier>
        <rdfs:comment xml:lang="en">Manual traffic control e.g. by police, traffic guard, pedestrian at some temporary site, e.g. at an accident.</rdfs:comment>
        <rdfs:label xml:lang="de">(Bau-)Stelle mit manueller Verkehrsregelung</rdfs:label>
        <rdfs:label xml:lang="en">Manual Traffic Control</rdfs:label>
    </owl:Class>
    


    <!-- http://purl.org/auto/criticality_phenomena#CP_78 -->

    <owl:Class rdf:about="http://purl.org/auto/criticality_phenomena#CP_78">
        <rdfs:subClassOf rdf:resource="http://purl.org/auto/criticality_phenomena#Behavioral_Criticality_Phenomenon"/>
        <rdfs:subClassOf rdf:resource="http://purl.org/auto/criticality_phenomena#CP_56"/>
        <rdfs:subClassOf rdf:resource="http://purl.org/auto/criticality_phenomena#Unpredictability_Criticality_Phenomenon"/>
        <dcterms:identifier rdf:datatype="http://www.w3.org/2001/XMLSchema#nonNegativeInteger">78</dcterms:identifier>
        <rdfs:comment xml:lang="en">Possible glare of other TPs due to beam angle being too high when beams are on.</rdfs:comment>
        <rdfs:label xml:lang="de">Abblendlicht zu hoch eingestellt</rdfs:label>
        <rdfs:label xml:lang="en">Low Beam Angle Too High</rdfs:label>
    </owl:Class>
    


    <!-- http://purl.org/auto/criticality_phenomena#CP_79 -->

    <owl:Class rdf:about="http://purl.org/auto/criticality_phenomena#CP_79">
        <rdfs:subClassOf rdf:resource="http://purl.org/auto/criticality_phenomena#CP_213"/>
        <rdfs:subClassOf rdf:resource="http://purl.org/auto/criticality_phenomena#Perfect_Perception_Criticality_Phenomenon"/>
        <dcterms:identifier rdf:datatype="http://www.w3.org/2001/XMLSchema#nonNegativeInteger">79</dcterms:identifier>
        <rdfs:comment xml:lang="en">Can be any object such as waste bin, tree, ...</rdfs:comment>
        <rdfs:label xml:lang="en">Burning Object Near Road</rdfs:label>
        <rdfs:label xml:lang="de">brennendes Objekt in Fahrbahnnähe</rdfs:label>
    </owl:Class>
    


    <!-- http://purl.org/auto/criticality_phenomena#CP_8 -->

    <owl:Class rdf:about="http://purl.org/auto/criticality_phenomena#CP_8">
        <rdfs:subClassOf rdf:resource="http://purl.org/auto/criticality_phenomena#CP_213"/>
        <rdfs:subClassOf rdf:resource="http://purl.org/auto/criticality_phenomena#Human_Criticality_Phenomenon"/>
        <rdfs:subClassOf rdf:resource="http://purl.org/auto/criticality_phenomena#Perfect_Perception_Criticality_Phenomenon"/>
        <dcterms:identifier rdf:datatype="http://www.w3.org/2001/XMLSchema#nonNegativeInteger">8</dcterms:identifier>
        <rdfs:comment xml:lang="en">A balloon is close to the ego vehicle.</rdfs:comment>
        <rdfs:label xml:lang="de">Ballon in der Nähe von Ego</rdfs:label>
        <rdfs:label xml:lang="en">Balloon Near Ego</rdfs:label>
    </owl:Class>
    


    <!-- http://purl.org/auto/criticality_phenomena#CP_80 -->

    <owl:Class rdf:about="http://purl.org/auto/criticality_phenomena#CP_80">
        <rdfs:subClassOf rdf:resource="http://purl.org/auto/criticality_phenomena#CP_79"/>
        <dcterms:identifier rdf:datatype="http://www.w3.org/2001/XMLSchema#nonNegativeInteger">80</dcterms:identifier>
        <rdfs:comment xml:lang="en">A burning vehicle on or close to the road.</rdfs:comment>
        <rdfs:label xml:lang="en">Burning Vehicle Near Road</rdfs:label>
        <rdfs:label xml:lang="de">brennendes Fahrzeug in Fahrbahnnähe</rdfs:label>
    </owl:Class>
    


    <!-- http://purl.org/auto/criticality_phenomena#CP_81 -->

    <owl:Class rdf:about="http://purl.org/auto/criticality_phenomena#CP_81">
        <rdfs:subClassOf rdf:resource="http://purl.org/auto/criticality_phenomena#CP_113"/>
        <dcterms:identifier rdf:datatype="http://www.w3.org/2001/XMLSchema#nonNegativeInteger">81</dcterms:identifier>
        <rdfs:comment xml:lang="en">In the scenario, there is at least one URU that has physical access to the road.</rdfs:comment>
        <rdfs:label xml:lang="de">Anwesenheit von URUs mit Fahrbahnzugang</rdfs:label>
        <rdfs:label xml:lang="en">Presence Of URUs With Road Access</rdfs:label>
    </owl:Class>
    


    <!-- http://purl.org/auto/criticality_phenomena#CP_82 -->

    <owl:Class rdf:about="http://purl.org/auto/criticality_phenomena#CP_82">
        <rdfs:subClassOf rdf:resource="http://purl.org/auto/criticality_phenomena#CP_32"/>
        <rdfs:subClassOf rdf:resource="http://purl.org/auto/criticality_phenomena#Human_Criticality_Phenomenon"/>
        <formalized rdf:datatype="http://www.w3.org/2001/XMLSchema#boolean">true</formalized>
        <dcterms:identifier rdf:datatype="http://www.w3.org/2001/XMLSchema#nonNegativeInteger">82</dcterms:identifier>
        <rdfs:comment xml:lang="en">A pedestrian is located on the road. Criticality depends on context</rdfs:comment>
        <rdfs:label xml:lang="de">Fußgänger auf der Straße</rdfs:label>
        <rdfs:label xml:lang="en">Pedestrian On Road</rdfs:label>
    </owl:Class>
    


    <!-- http://purl.org/auto/criticality_phenomena#CP_83 -->

    <owl:Class rdf:about="http://purl.org/auto/criticality_phenomena#CP_83">
        <rdfs:subClassOf rdf:resource="http://purl.org/auto/criticality_phenomena#CP_32"/>
        <dcterms:identifier rdf:datatype="http://www.w3.org/2001/XMLSchema#nonNegativeInteger">83</dcterms:identifier>
        <rdfs:comment xml:lang="en">This includes wild animals that cannot simply be run over due to accident potentual such as wild boards</rdfs:comment>
        <rdfs:label xml:lang="en">Wild Animal On Road</rdfs:label>
        <rdfs:label xml:lang="de">wildes Tier auf der Straße</rdfs:label>
    </owl:Class>
    


    <!-- http://purl.org/auto/criticality_phenomena#CP_84 -->

    <owl:Class rdf:about="http://purl.org/auto/criticality_phenomena#CP_84">
        <rdfs:subClassOf rdf:resource="http://purl.org/auto/criticality_phenomena#Behavioral_Criticality_Phenomenon"/>
        <rdfs:subClassOf rdf:resource="http://purl.org/auto/criticality_phenomena#CP_24"/>
        <dcterms:identifier rdf:datatype="http://www.w3.org/2001/XMLSchema#nonNegativeInteger">84</dcterms:identifier>
        <rdfs:comment xml:lang="en">An accident has happened and the site is not protected by e.g. warning signs.</rdfs:comment>
        <rdfs:label xml:lang="en">Unprotected Accident Site</rdfs:label>
        <rdfs:label xml:lang="de">ungesicherte Unfallstelle</rdfs:label>
    </owl:Class>
    


    <!-- http://purl.org/auto/criticality_phenomena#CP_85 -->

    <owl:Class rdf:about="http://purl.org/auto/criticality_phenomena#CP_85">
        <rdfs:subClassOf rdf:resource="http://purl.org/auto/criticality_phenomena#CP_212"/>
        <rdfs:subClassOf rdf:resource="http://purl.org/auto/criticality_phenomena#CP_275"/>
        <rdfs:subClassOf rdf:resource="http://purl.org/auto/criticality_phenomena#Perfect_Perception_Criticality_Phenomenon"/>
        <dcterms:identifier rdf:datatype="http://www.w3.org/2001/XMLSchema#nonNegativeInteger">85</dcterms:identifier>
        <rdfs:comment xml:lang="en">A vehicle is present on the road that is not able to move by its own power.</rdfs:comment>
        <rdfs:label xml:lang="en">Immobilized Vehicle</rdfs:label>
        <rdfs:label xml:lang="de">liegen gebliebenes Fahrzeug</rdfs:label>
    </owl:Class>
    


    <!-- http://purl.org/auto/criticality_phenomena#CP_86 -->

    <owl:Class rdf:about="http://purl.org/auto/criticality_phenomena#CP_86">
        <rdfs:subClassOf rdf:resource="http://purl.org/auto/criticality_phenomena#CP_54"/>
        <rdfs:subClassOf rdf:resource="http://purl.org/auto/criticality_phenomena#Human_Criticality_Phenomenon"/>
        <rdfs:subClassOf rdf:resource="http://purl.org/auto/criticality_phenomena#Spatial_Criticality_Phenomenon"/>
        <rdfs:subClassOf rdf:resource="http://purl.org/auto/criticality_phenomena#Unpredictability_Criticality_Phenomenon"/>
        <dcterms:identifier rdf:datatype="http://www.w3.org/2001/XMLSchema#nonNegativeInteger">86</dcterms:identifier>
        <rdfs:comment xml:lang="en">A TP is overtaking a bicyclist which is driving on a protection lane.</rdfs:comment>
        <rdfs:label xml:lang="en">Overtaking Of Bicyclist On Bicycle Protection Lane</rdfs:label>
        <rdfs:label xml:lang="de">Überholen eines Radfahrers auf Radfahrschutzstreifen</rdfs:label>
    </owl:Class>
    


    <!-- http://purl.org/auto/criticality_phenomena#CP_87 -->

    <owl:Class rdf:about="http://purl.org/auto/criticality_phenomena#CP_87">
        <rdfs:subClassOf rdf:resource="http://purl.org/auto/criticality_phenomena#CP_54"/>
        <rdfs:subClassOf rdf:resource="http://purl.org/auto/criticality_phenomena#Human_Criticality_Phenomenon"/>
        <rdfs:subClassOf rdf:resource="http://purl.org/auto/criticality_phenomena#Unpredictability_Criticality_Phenomenon"/>
        <dcterms:identifier rdf:datatype="http://www.w3.org/2001/XMLSchema#nonNegativeInteger">87</dcterms:identifier>
        <rdfs:comment xml:lang="en">A TP is overtaking a bicyclist which is driving on a bicycle lane.</rdfs:comment>
        <rdfs:label xml:lang="en">Overtaking Of Bicyclist On Bicycle On Bicycle Lane</rdfs:label>
        <rdfs:label xml:lang="de">Überholen eines Radfahrers auf dem Fahrradweg</rdfs:label>
    </owl:Class>
    


    <!-- http://purl.org/auto/criticality_phenomena#CP_88 -->

    <owl:Class rdf:about="http://purl.org/auto/criticality_phenomena#CP_88">
        <rdfs:subClassOf rdf:resource="http://purl.org/auto/criticality_phenomena#CP_54"/>
        <rdfs:subClassOf rdf:resource="http://purl.org/auto/criticality_phenomena#Human_Criticality_Phenomenon"/>
        <rdfs:subClassOf rdf:resource="http://purl.org/auto/criticality_phenomena#Spatial_Criticality_Phenomenon"/>
        <rdfs:subClassOf rdf:resource="http://purl.org/auto/criticality_phenomena#Unpredictability_Criticality_Phenomenon"/>
        <dcterms:identifier rdf:datatype="http://www.w3.org/2001/XMLSchema#nonNegativeInteger">88</dcterms:identifier>
        <rdfs:comment xml:lang="en">A TP is overtaking a bicyclist which is driving on a car lane.</rdfs:comment>
        <rdfs:label xml:lang="en">Overtaking Of Bicyclist On Car Lane</rdfs:label>
        <rdfs:label xml:lang="de">Überholen eines Radfahrers auf PKW-Fahrstreifen</rdfs:label>
    </owl:Class>
    


    <!-- http://purl.org/auto/criticality_phenomena#CP_89 -->

    <owl:Class rdf:about="http://purl.org/auto/criticality_phenomena#CP_89">
        <rdfs:subClassOf rdf:resource="http://purl.org/auto/criticality_phenomena#CP_54"/>
        <rdfs:subClassOf rdf:resource="http://purl.org/auto/criticality_phenomena#Human_Criticality_Phenomenon"/>
        <rdfs:subClassOf rdf:resource="http://purl.org/auto/criticality_phenomena#Spatial_Criticality_Phenomenon"/>
        <rdfs:subClassOf rdf:resource="http://purl.org/auto/criticality_phenomena#Unpredictability_Criticality_Phenomenon"/>
        <dcterms:identifier rdf:datatype="http://www.w3.org/2001/XMLSchema#nonNegativeInteger">89</dcterms:identifier>
        <rdfs:comment xml:lang="en">A TP is overtaking a bus which is currently stopping at a bus stop.</rdfs:comment>
        <rdfs:label xml:lang="en">Overtaking Of Bus At Bus Stop</rdfs:label>
        <rdfs:label xml:lang="de">Überholen eines Busses an einer Bushaltestelle</rdfs:label>
    </owl:Class>
    


    <!-- http://purl.org/auto/criticality_phenomena#CP_9 -->

    <owl:Class rdf:about="http://purl.org/auto/criticality_phenomena#CP_9">
        <rdfs:subClassOf rdf:resource="http://purl.org/auto/criticality_phenomena#CP_217"/>
        <rdfs:subClassOf rdf:resource="http://purl.org/auto/criticality_phenomena#Perfect_Perception_Criticality_Phenomenon"/>
        <dcterms:identifier rdf:datatype="http://www.w3.org/2001/XMLSchema#nonNegativeInteger">9</dcterms:identifier>
        <rdfs:comment xml:lang="en">A metallic can (e.g. drinking can) is close to the ego. May influence radar sensor; criticality depends on sensor setup &amp; fusion.</rdfs:comment>
        <rdfs:label xml:lang="de">Metall Dose auf der Fahrbahn</rdfs:label>
        <rdfs:label xml:lang="en">Metallic Can On Road</rdfs:label>
    </owl:Class>
    


    <!-- http://purl.org/auto/criticality_phenomena#CP_90 -->

    <owl:Class rdf:about="http://purl.org/auto/criticality_phenomena#CP_90">
        <rdfs:subClassOf rdf:resource="http://purl.org/auto/criticality_phenomena#CP_54"/>
        <rdfs:subClassOf rdf:resource="http://purl.org/auto/criticality_phenomena#Spatial_Criticality_Phenomenon"/>
        <dcterms:identifier rdf:datatype="http://www.w3.org/2001/XMLSchema#nonNegativeInteger">90</dcterms:identifier>
        <rdfs:comment xml:lang="en">Slower vehicle here means speed difference of at least 20 km/h, i.e. (depending on local speed limits) waste collection, heavy loads, agricultural traffic, construction machines</rdfs:comment>
        <rdfs:label xml:lang="en">Overtaking Of Slower Vehicle</rdfs:label>
        <rdfs:label xml:lang="de">Überholen eines langsameren Fahrzeugs</rdfs:label>
    </owl:Class>
    


    <!-- http://purl.org/auto/criticality_phenomena#CP_91 -->

    <owl:Class rdf:about="http://purl.org/auto/criticality_phenomena#CP_91">
        <rdfs:subClassOf rdf:resource="http://purl.org/auto/criticality_phenomena#Behavioral_Criticality_Phenomenon"/>
        <rdfs:subClassOf rdf:resource="http://purl.org/auto/criticality_phenomena#CP_279"/>
        <rdfs:subClassOf rdf:resource="http://purl.org/auto/criticality_phenomena#Complexity_Criticality_Phenomenon"/>
        <rdfs:subClassOf rdf:resource="http://purl.org/auto/criticality_phenomena#Human_Criticality_Phenomenon"/>
        <rdfs:subClassOf rdf:resource="http://purl.org/auto/criticality_phenomena#Perfect_Perception_Criticality_Phenomenon"/>
        <rdfs:subClassOf rdf:resource="http://purl.org/auto/criticality_phenomena#Unpredictability_Criticality_Phenomenon"/>
        <dcterms:identifier rdf:datatype="http://www.w3.org/2001/XMLSchema#nonNegativeInteger">91</dcterms:identifier>
        <rdfs:comment xml:lang="en">This includes all parking vehicles</rdfs:comment>
        <rdfs:label xml:lang="de">Passieren parkender Fahrzeugen</rdfs:label>
        <rdfs:label xml:lang="en">Passing Of Parking Vehicle</rdfs:label>
    </owl:Class>
    


    <!-- http://purl.org/auto/criticality_phenomena#CP_92 -->

    <owl:Class rdf:about="http://purl.org/auto/criticality_phenomena#CP_92">
        <rdfs:subClassOf rdf:resource="http://purl.org/auto/criticality_phenomena#Behavioral_Criticality_Phenomenon"/>
        <rdfs:subClassOf rdf:resource="http://purl.org/auto/criticality_phenomena#CP_279"/>
        <rdfs:subClassOf rdf:resource="http://purl.org/auto/criticality_phenomena#Complexity_Criticality_Phenomenon"/>
        <rdfs:subClassOf rdf:resource="http://purl.org/auto/criticality_phenomena#Human_Criticality_Phenomenon"/>
        <rdfs:subClassOf rdf:resource="http://purl.org/auto/criticality_phenomena#Perfect_Perception_Criticality_Phenomenon"/>
        <rdfs:subClassOf rdf:resource="http://purl.org/auto/criticality_phenomena#Unpredictability_Criticality_Phenomenon"/>
        <dcterms:identifier rdf:datatype="http://www.w3.org/2001/XMLSchema#nonNegativeInteger">92</dcterms:identifier>
        <rdfs:comment xml:lang="en">Operation areas refers to areas with active police, fire service and ambulance operations</rdfs:comment>
        <rdfs:label xml:lang="de">Passieren von Einsatzstelle</rdfs:label>
        <rdfs:label xml:lang="en">Passing Of Operation Area</rdfs:label>
    </owl:Class>
    


    <!-- http://purl.org/auto/criticality_phenomena#CP_93 -->

    <owl:Class rdf:about="http://purl.org/auto/criticality_phenomena#CP_93">
        <rdfs:subClassOf rdf:resource="http://purl.org/auto/criticality_phenomena#CP_54"/>
        <rdfs:subClassOf rdf:resource="http://purl.org/auto/criticality_phenomena#Spatial_Criticality_Phenomenon"/>
        <rdfs:subClassOf rdf:resource="http://purl.org/auto/criticality_phenomena#Unpredictability_Criticality_Phenomenon"/>
        <dcterms:identifier rdf:datatype="http://www.w3.org/2001/XMLSchema#nonNegativeInteger">93</dcterms:identifier>
        <rdfs:comment xml:lang="en">Generally, Non-Ego-TP who is performing an overtaking maneuver. 
Includes overtaking multiples vehicles without merging back into lane.</rdfs:comment>
        <rdfs:label xml:lang="de">Non-Ego-TP  überholt (mehrere) Fahrzeug(e)</rdfs:label>
        <rdfs:label xml:lang="en">Non-Ego-TP Overtaking Other Vehicles</rdfs:label>
    </owl:Class>
    


    <!-- http://purl.org/auto/criticality_phenomena#CP_94 -->

    <owl:Class rdf:about="http://purl.org/auto/criticality_phenomena#CP_94">
        <rdfs:subClassOf rdf:resource="http://purl.org/auto/criticality_phenomena#CP_54"/>
        <rdfs:subClassOf rdf:resource="http://purl.org/auto/criticality_phenomena#Spatial_Criticality_Phenomenon"/>
        <rdfs:subClassOf rdf:resource="http://purl.org/auto/criticality_phenomena#Unpredictability_Criticality_Phenomenon"/>
        <dcterms:identifier rdf:datatype="http://www.w3.org/2001/XMLSchema#nonNegativeInteger">94</dcterms:identifier>
        <rdfs:comment xml:lang="en">Overtaking maneuver on the right side.</rdfs:comment>
        <rdfs:label xml:lang="en">Non-Ego-TP Overtaking On Right Side</rdfs:label>
        <rdfs:label xml:lang="de">Non-Ego-TP überholt rechtsseitig</rdfs:label>
    </owl:Class>
    


    <!-- http://purl.org/auto/criticality_phenomena#CP_95 -->

    <owl:Class rdf:about="http://purl.org/auto/criticality_phenomena#CP_95">
        <rdfs:subClassOf rdf:resource="http://purl.org/auto/criticality_phenomena#CP_54"/>
        <rdfs:subClassOf rdf:resource="http://purl.org/auto/criticality_phenomena#Spatial_Criticality_Phenomenon"/>
        <rdfs:subClassOf rdf:resource="http://purl.org/auto/criticality_phenomena#Unpredictability_Criticality_Phenomenon"/>
        <dcterms:identifier rdf:datatype="http://www.w3.org/2001/XMLSchema#nonNegativeInteger">95</dcterms:identifier>
        <rdfs:comment xml:lang="en">Overtaking is not allowed, but a non-ego TP does so nevertheless.</rdfs:comment>
        <rdfs:label xml:lang="en">Non-Ego-TP Overtaking Illegitimately</rdfs:label>
        <rdfs:label xml:lang="de">Non-Ego-TP überholt trotz Überholverbot</rdfs:label>
    </owl:Class>
    


    <!-- http://purl.org/auto/criticality_phenomena#CP_96 -->

    <owl:Class rdf:about="http://purl.org/auto/criticality_phenomena#CP_96">
        <rdfs:subClassOf rdf:resource="http://purl.org/auto/criticality_phenomena#CP_216"/>
        <rdfs:subClassOf rdf:resource="http://purl.org/auto/criticality_phenomena#Perfect_Perception_Criticality_Phenomenon"/>
        <dcterms:identifier rdf:datatype="http://www.w3.org/2001/XMLSchema#nonNegativeInteger">96</dcterms:identifier>
        <rdfs:comment xml:lang="en">Risky here means lane changes that either brake traffic rules, are unexpected or violate safety distances</rdfs:comment>
        <rdfs:label xml:lang="de">Non-Ego-TP führt riskanten Fahrstreifenwechsel aus</rdfs:label>
        <rdfs:label xml:lang="en">Risky Lane Change Of Non-Ego-TP</rdfs:label>
    </owl:Class>
    


    <!-- http://purl.org/auto/criticality_phenomena#CP_97 -->

    <owl:Class rdf:about="http://purl.org/auto/criticality_phenomena#CP_97">
        <rdfs:subClassOf rdf:resource="http://purl.org/auto/criticality_phenomena#CP_216"/>
        <rdfs:subClassOf rdf:resource="http://purl.org/auto/criticality_phenomena#Perfect_Perception_Criticality_Phenomenon"/>
        <dcterms:identifier rdf:datatype="http://www.w3.org/2001/XMLSchema#nonNegativeInteger">97</dcterms:identifier>
        <rdfs:comment xml:lang="en">E.g. merging/ending bicycle lanes on street/sidewalk</rdfs:comment>
        <rdfs:label xml:lang="en">Bicycle Lane Change Onto Road</rdfs:label>
        <rdfs:label xml:lang="de">Radfahrer wechselt auf die Fahrbahn</rdfs:label>
    </owl:Class>
    


    <!-- http://purl.org/auto/criticality_phenomena#CP_98 -->

    <owl:Class rdf:about="http://purl.org/auto/criticality_phenomena#CP_98">
        <rdfs:subClassOf rdf:resource="http://purl.org/auto/criticality_phenomena#CP_143"/>
        <rdfs:subClassOf rdf:resource="http://purl.org/auto/criticality_phenomena#Dynamical_Criticality_Phenomenon"/>
        <dcterms:identifier rdf:datatype="http://www.w3.org/2001/XMLSchema#nonNegativeInteger">98</dcterms:identifier>
        <rdfs:comment xml:lang="en">A driver not following the driving direction of the lane.</rdfs:comment>
        <rdfs:label xml:lang="de">Falschfahrer (motorisiertes Fahrzeug)</rdfs:label>
        <rdfs:label xml:lang="en">Wrong-way Driver</rdfs:label>
    </owl:Class>
    


    <!-- http://purl.org/auto/criticality_phenomena#CP_99 -->

    <owl:Class rdf:about="http://purl.org/auto/criticality_phenomena#CP_99">
        <rdfs:subClassOf rdf:resource="http://purl.org/auto/criticality_phenomena#CP_143"/>
        <rdfs:subClassOf rdf:resource="http://purl.org/auto/criticality_phenomena#Dynamical_Criticality_Phenomenon"/>
        <rdfs:subClassOf rdf:resource="http://purl.org/auto/criticality_phenomena#Human_Criticality_Phenomenon"/>
        <rdfs:subClassOf rdf:resource="http://purl.org/auto/criticality_phenomena#Spatial_Criticality_Phenomenon"/>
        <dcterms:identifier rdf:datatype="http://www.w3.org/2001/XMLSchema#nonNegativeInteger">99</dcterms:identifier>
        <rdfs:comment xml:lang="en">E.g. on one-way roads that are not open for bicycles in both directions</rdfs:comment>
        <rdfs:label xml:lang="de">Falschfahrer (Fahrrad)</rdfs:label>
        <rdfs:label xml:lang="en">Wrong-way Bicyclist</rdfs:label>
    </owl:Class>
    


    <!-- http://purl.org/auto/criticality_phenomena#Complexity_Criticality_Phenomenon -->

    <owl:Class rdf:about="http://purl.org/auto/criticality_phenomena#Complexity_Criticality_Phenomenon">
        <rdfs:subClassOf rdf:resource="http://purl.org/auto/criticality_phenomena#Tagged_Criticality_Phenomenon"/>
        <rdfs:label xml:lang="en">Complexity Criticality Phenomenon</rdfs:label>
        <rdfs:label xml:lang="de">Komplexitäts_Kritikalitätsphänomen</rdfs:label>
    </owl:Class>
    


    <!-- http://purl.org/auto/criticality_phenomena#Criticality_Phenomenon -->

    <owl:Class rdf:about="http://purl.org/auto/criticality_phenomena#Criticality_Phenomenon">
        <rdfs:label xml:lang="en">Criticality Phenomenon</rdfs:label>
        <rdfs:label xml:lang="de">Kritikalitätsphänomen</rdfs:label>
    </owl:Class>
    


    <!-- http://purl.org/auto/criticality_phenomena#Dynamical_Criticality_Phenomenon -->

    <owl:Class rdf:about="http://purl.org/auto/criticality_phenomena#Dynamical_Criticality_Phenomenon">
        <rdfs:subClassOf rdf:resource="http://purl.org/auto/criticality_phenomena#Tagged_Criticality_Phenomenon"/>
        <rdfs:label xml:lang="en">Dynamical Criticality Phenomenon</rdfs:label>
        <rdfs:label xml:lang="de">Dynamisches_Kritikalitätsphänomen</rdfs:label>
    </owl:Class>
    


    <!-- http://purl.org/auto/criticality_phenomena#Environmental_Criticality_Phenomenon -->

    <owl:Class rdf:about="http://purl.org/auto/criticality_phenomena#Environmental_Criticality_Phenomenon">
        <rdfs:subClassOf rdf:resource="http://purl.org/auto/criticality_phenomena#Tagged_Criticality_Phenomenon"/>
        <rdfs:label xml:lang="en">Environmental Criticality Phenomenon</rdfs:label>
        <rdfs:label xml:lang="de">Umwelt_Kritikalitätsphänomen</rdfs:label>
    </owl:Class>
    


    <!-- http://purl.org/auto/criticality_phenomena#Human_Criticality_Phenomenon -->

    <owl:Class rdf:about="http://purl.org/auto/criticality_phenomena#Human_Criticality_Phenomenon">
        <rdfs:subClassOf rdf:resource="http://purl.org/auto/criticality_phenomena#Tagged_Criticality_Phenomenon"/>
        <rdfs:label xml:lang="en">Human Criticality Phenomenon</rdfs:label>
        <rdfs:label xml:lang="de">Menschliches_Kritikalitätsphänomen</rdfs:label>
    </owl:Class>
    


    <!-- http://purl.org/auto/criticality_phenomena#Perception_Criticality_Phenomenon -->

    <owl:Class rdf:about="http://purl.org/auto/criticality_phenomena#Perception_Criticality_Phenomenon">
        <rdfs:subClassOf rdf:resource="http://purl.org/auto/criticality_phenomena#Tagged_Criticality_Phenomenon"/>
        <rdfs:label xml:lang="en">Perception Criticality Phenomenon</rdfs:label>
        <rdfs:label xml:lang="de">Perzeptions_Kritikalitätsphänomen</rdfs:label>
    </owl:Class>
    


    <!-- http://purl.org/auto/criticality_phenomena#Perfect_Camera_Criticality_Phenomenon -->

    <owl:Class rdf:about="http://purl.org/auto/criticality_phenomena#Perfect_Camera_Criticality_Phenomenon">
        <rdfs:subClassOf rdf:resource="http://purl.org/auto/criticality_phenomena#Perfect_Perception_Criticality_Phenomenon"/>
        <rdfs:label xml:lang="de">Perekte_Kamera_Kritikalitätsphänomen</rdfs:label>
        <rdfs:label xml:lang="en">Perfect Camera Criticality Phenomenon</rdfs:label>
    </owl:Class>
    


    <!-- http://purl.org/auto/criticality_phenomena#Perfect_Human_Criticality_Phenomenon -->

    <owl:Class rdf:about="http://purl.org/auto/criticality_phenomena#Perfect_Human_Criticality_Phenomenon">
        <rdfs:subClassOf rdf:resource="http://purl.org/auto/criticality_phenomena#Perfect_Perception_Criticality_Phenomenon"/>
        <rdfs:label xml:lang="de">Perekter_Mensch_Kritikalitätsphänomen</rdfs:label>
        <rdfs:label xml:lang="en">Perfect Human Criticality Phenomenon</rdfs:label>
    </owl:Class>
    


    <!-- http://purl.org/auto/criticality_phenomena#Perfect_Lidar_Criticality_Phenomenon -->

    <owl:Class rdf:about="http://purl.org/auto/criticality_phenomena#Perfect_Lidar_Criticality_Phenomenon">
        <rdfs:subClassOf rdf:resource="http://purl.org/auto/criticality_phenomena#Perfect_Perception_Criticality_Phenomenon"/>
        <rdfs:label xml:lang="de">Perektes_Lidar_Kritikalitätsphänomen</rdfs:label>
        <rdfs:label xml:lang="en">Perfect Lidar Criticality Phenomenon</rdfs:label>
    </owl:Class>
    


    <!-- http://purl.org/auto/criticality_phenomena#Perfect_Perception_Algorithm_Criticality_Phenomenon -->

    <owl:Class rdf:about="http://purl.org/auto/criticality_phenomena#Perfect_Perception_Algorithm_Criticality_Phenomenon">
        <rdfs:subClassOf rdf:resource="http://purl.org/auto/criticality_phenomena#Perfect_Perception_Criticality_Phenomenon"/>
        <rdfs:label xml:lang="en">Perfect Perception Criticality Phenomenon</rdfs:label>
        <rdfs:label xml:lang="de">Perfekter_Perzeptionsalgorithmen_Kritikalitätsphänomen</rdfs:label>
    </owl:Class>
    


    <!-- http://purl.org/auto/criticality_phenomena#Perfect_Perception_Criticality_Phenomenon -->

    <owl:Class rdf:about="http://purl.org/auto/criticality_phenomena#Perfect_Perception_Criticality_Phenomenon">
        <rdfs:subClassOf rdf:resource="http://purl.org/auto/criticality_phenomena#Perception_Criticality_Phenomenon"/>
        <rdfs:label xml:lang="en">Perfect erception Criticality Phenomenon</rdfs:label>
        <rdfs:label xml:lang="de">Perfektes_Perzeptions_Kritikalitätsphänomen</rdfs:label>
    </owl:Class>
    


    <!-- http://purl.org/auto/criticality_phenomena#Perfect_Radar_Criticality_Phenomenon -->

    <owl:Class rdf:about="http://purl.org/auto/criticality_phenomena#Perfect_Radar_Criticality_Phenomenon">
        <rdfs:subClassOf rdf:resource="http://purl.org/auto/criticality_phenomena#Perfect_Perception_Criticality_Phenomenon"/>
        <rdfs:label xml:lang="de">Perektes_Radar_Kritikalitätsphänomen</rdfs:label>
        <rdfs:label xml:lang="en">Perfect Radar Criticality Phenomenon</rdfs:label>
    </owl:Class>
    


    <!-- http://purl.org/auto/criticality_phenomena#Real_Camera_Criticality_Phenomenon -->

    <owl:Class rdf:about="http://purl.org/auto/criticality_phenomena#Real_Camera_Criticality_Phenomenon">
        <rdfs:subClassOf rdf:resource="http://purl.org/auto/criticality_phenomena#Real_Perception_Criticality_Phenomenon"/>
        <rdfs:label xml:lang="en">Real Camera Criticality Phenomenon</rdfs:label>
        <rdfs:label xml:lang="de">Reale_Kamera_Kritikalitätsphänomen</rdfs:label>
    </owl:Class>
    


    <!-- http://purl.org/auto/criticality_phenomena#Real_Human_Criticality_Phenomenon -->

    <owl:Class rdf:about="http://purl.org/auto/criticality_phenomena#Real_Human_Criticality_Phenomenon">
        <rdfs:subClassOf rdf:resource="http://purl.org/auto/criticality_phenomena#Real_Perception_Criticality_Phenomenon"/>
        <rdfs:label xml:lang="en">Real Human Criticality Phenomenon</rdfs:label>
        <rdfs:label xml:lang="de">Realer_Mensch_Kritikalitätsphänomen</rdfs:label>
    </owl:Class>
    


    <!-- http://purl.org/auto/criticality_phenomena#Real_Lidar_Criticality_Phenomenon -->

    <owl:Class rdf:about="http://purl.org/auto/criticality_phenomena#Real_Lidar_Criticality_Phenomenon">
        <rdfs:subClassOf rdf:resource="http://purl.org/auto/criticality_phenomena#Real_Perception_Criticality_Phenomenon"/>
        <rdfs:label xml:lang="en">Real Lidar Criticality Phenomenon</rdfs:label>
        <rdfs:label xml:lang="de">Reales_Lidar_Kritikalitätsphänomen</rdfs:label>
    </owl:Class>
    


    <!-- http://purl.org/auto/criticality_phenomena#Real_Perception_Algorithm_Criticality_Phenomenon -->

    <owl:Class rdf:about="http://purl.org/auto/criticality_phenomena#Real_Perception_Algorithm_Criticality_Phenomenon">
        <rdfs:subClassOf rdf:resource="http://purl.org/auto/criticality_phenomena#Real_Perception_Criticality_Phenomenon"/>
        <rdfs:label xml:lang="en">Real Perception Criticality Phenomenon</rdfs:label>
        <rdfs:label xml:lang="de">Realer_Perzeptionsalgorithmen_Kritikalitätsphänomen</rdfs:label>
    </owl:Class>
    


    <!-- http://purl.org/auto/criticality_phenomena#Real_Perception_Criticality_Phenomenon -->

    <owl:Class rdf:about="http://purl.org/auto/criticality_phenomena#Real_Perception_Criticality_Phenomenon">
        <rdfs:subClassOf rdf:resource="http://purl.org/auto/criticality_phenomena#Perception_Criticality_Phenomenon"/>
        <rdfs:label xml:lang="en">Real Perception Criticality Phenomenon</rdfs:label>
        <rdfs:label xml:lang="de">Reales_Perzeptions_Kritikalitätsphänomen</rdfs:label>
    </owl:Class>
    


    <!-- http://purl.org/auto/criticality_phenomena#Real_Radar_Criticality_Phenomenon -->

    <owl:Class rdf:about="http://purl.org/auto/criticality_phenomena#Real_Radar_Criticality_Phenomenon">
        <rdfs:subClassOf rdf:resource="http://purl.org/auto/criticality_phenomena#Real_Perception_Criticality_Phenomenon"/>
        <rdfs:label xml:lang="en">Real Radar Criticality Phenomenon</rdfs:label>
        <rdfs:label xml:lang="de">Reales_Radar_Kritikalitätsphänomen</rdfs:label>
    </owl:Class>
    


    <!-- http://purl.org/auto/criticality_phenomena#Spatial_Criticality_Phenomenon -->

    <owl:Class rdf:about="http://purl.org/auto/criticality_phenomena#Spatial_Criticality_Phenomenon">
        <rdfs:subClassOf rdf:resource="http://purl.org/auto/criticality_phenomena#Tagged_Criticality_Phenomenon"/>
        <rdfs:label xml:lang="de">Räumliches_Kritikalitätsphänomen</rdfs:label>
        <rdfs:label xml:lang="en">Spatial Criticality Phenomenon</rdfs:label>
    </owl:Class>
    


    <!-- http://purl.org/auto/criticality_phenomena#Tagged_Criticality_Phenomenon -->

    <owl:Class rdf:about="http://purl.org/auto/criticality_phenomena#Tagged_Criticality_Phenomenon">
        <rdfs:subClassOf rdf:resource="http://purl.org/auto/criticality_phenomena#Criticality_Phenomenon"/>
        <rdfs:label xml:lang="de">Getaggtes_Kritikalitätsphänomen</rdfs:label>
        <rdfs:label xml:lang="en">Tagged Criticality Phenomenon</rdfs:label>
    </owl:Class>
    


    <!-- http://purl.org/auto/criticality_phenomena#Temporal_Criticality_Phenomenon -->

    <owl:Class rdf:about="http://purl.org/auto/criticality_phenomena#Temporal_Criticality_Phenomenon">
        <rdfs:subClassOf rdf:resource="http://purl.org/auto/criticality_phenomena#Tagged_Criticality_Phenomenon"/>
        <rdfs:label xml:lang="en">Temporal Criticality Phenomenon</rdfs:label>
        <rdfs:label xml:lang="de">Temporales_Kritikalitätsphänomen</rdfs:label>
    </owl:Class>
    


    <!-- http://purl.org/auto/criticality_phenomena#Unpredictability_Criticality_Phenomenon -->

    <owl:Class rdf:about="http://purl.org/auto/criticality_phenomena#Unpredictability_Criticality_Phenomenon">
        <rdfs:subClassOf rdf:resource="http://purl.org/auto/criticality_phenomena#Tagged_Criticality_Phenomenon"/>
        <rdfs:label xml:lang="en">Unpredictability Criticality Phenomenon</rdfs:label>
        <rdfs:label xml:lang="de">Unvorhersehbarkeits_Kritikalitätsphänomen</rdfs:label>
    </owl:Class>
</rdf:RDF>



<!-- Generated by the OWL API (version 4.5.9.2019-02-01T07:24:44Z) https://github.com/owlcs/owlapi -->

