<?xml version="1.0"?>
<rdf:RDF xmlns="http://purl.org/auto/l2_core#"
     xml:base="http://purl.org/auto/l2_core"
     xmlns:WV="http://www.wurvoc.org/vocabularies/WV/"
     xmlns:dc="http://purl.org/dc/elements/1.1/"
     xmlns:owl="http://www.w3.org/2002/07/owl#"
     xmlns:rdf="http://www.w3.org/1999/02/22-rdf-syntax-ns#"
     xmlns:xml="http://www.w3.org/XML/1998/namespace"
     xmlns:xsd="http://www.w3.org/2001/XMLSchema#"
     xmlns:bibo="http://purl.org/ontology/bibo/"
     xmlns:foaf="http://xmlns.com/foaf/0.1/"
     xmlns:rdfs="http://www.w3.org/2000/01/rdf-schema#"
     xmlns:skos="http://www.w3.org/2004/02/skos/core#"
     xmlns:swrla="http://swrl.stanford.edu/ontologies/3.3/swrla.owl#"
     xmlns:terms="http://purl.org/dc/terms/"
     xmlns:l2_core="http://purl.org/auto/l2_core#"
     xmlns:physics="http://purl.org/auto/physics#">
    <owl:Ontology rdf:about="http://purl.org/auto/l2_core">
        <owl:imports rdf:resource="http://purl.org/auto/physics"/>
        <owl:imports rdf:resource="http://www.opengis.net/ont/geosparql"/>
    </owl:Ontology>
    


    <!-- 
    ///////////////////////////////////////////////////////////////////////////////////////
    //
    // Object Properties
    //
    ///////////////////////////////////////////////////////////////////////////////////////
     -->

    


    <!-- http://purl.org/auto/l2_core#L2_property -->

    <owl:ObjectProperty rdf:about="http://purl.org/auto/l2_core#L2_property">
        <rdfs:label xml:lang="de">L2_eigenschaft</rdfs:label>
    </owl:ObjectProperty>
    


    <!-- 
    ///////////////////////////////////////////////////////////////////////////////////////
    //
    // Data properties
    //
    ///////////////////////////////////////////////////////////////////////////////////////
     -->

    


    <!-- http://purl.org/auto/l2_core#L2_data_property -->

    <owl:DatatypeProperty rdf:about="http://purl.org/auto/l2_core#L2_data_property">
        <rdfs:label xml:lang="de">L2_dateneigenschaft</rdfs:label>
    </owl:DatatypeProperty>
    


    <!-- 
    ///////////////////////////////////////////////////////////////////////////////////////
    //
    // Classes
    //
    ///////////////////////////////////////////////////////////////////////////////////////
     -->

    


    <!-- http://purl.org/auto/l2_core#Guidance_System -->

    <owl:Class rdf:about="http://purl.org/auto/l2_core#Guidance_System">
        <rdfs:subClassOf rdf:resource="http://purl.org/auto/l2_core#Traffic_Support_System"/>
        <rdfs:comment xml:lang="en">A system that guides traffic not through its regulating or advising effect but through its spatial properties.</rdfs:comment>
        <rdfs:label xml:lang="de">Leiteinrichtung</rdfs:label>
    </owl:Class>
    


    <!-- http://purl.org/auto/l2_core#L2_Entity -->

    <owl:Class rdf:about="http://purl.org/auto/l2_core#L2_Entity">
        <rdfs:subClassOf rdf:resource="http://purl.org/auto/physics#Spatial_Object"/>
        <rdfs:label xml:lang="de">L2_Entität</rdfs:label>
    </owl:Class>
    


    <!-- http://purl.org/auto/l2_core#Lighting_System -->

    <owl:Class rdf:about="http://purl.org/auto/l2_core#Lighting_System">
        <rdfs:subClassOf rdf:resource="http://purl.org/auto/l2_core#Traffic_Support_System"/>
        <rdfs:subClassOf rdf:resource="http://purl.org/auto/physics#Illumination_Source"/>
        <rdfs:comment xml:lang="en">A system that supports traffic through its illuminative properties.</rdfs:comment>
        <rdfs:label xml:lang="de">Beleuchtungseinrichtung</rdfs:label>
    </owl:Class>
    


    <!-- http://purl.org/auto/l2_core#Road_Construction -->

    <owl:Class rdf:about="http://purl.org/auto/l2_core#Road_Construction">
        <rdfs:subClassOf rdf:resource="http://purl.org/auto/l2_core#L2_Entity"/>
        <rdfs:comment xml:lang="en">A human-made construction that is permanently installed as an integral part of the shape of the road infrastructure but not placed alongside the road, e.g. a tunnel.</rdfs:comment>
        <rdfs:label xml:lang="de">Straßenbebauung</rdfs:label>
    </owl:Class>
    


    <!-- http://purl.org/auto/l2_core#Road_Furniture -->

    <owl:Class rdf:about="http://purl.org/auto/l2_core#Road_Furniture">
        <rdfs:subClassOf rdf:resource="http://purl.org/auto/l2_core#L2_Entity"/>
        <rdfs:comment xml:lang="en">A piece of equipment that is installed near roads for non-traffic guiding purposes, e.g. benches or bins.</rdfs:comment>
        <rdfs:label xml:lang="de">Straßenmöbel</rdfs:label>
    </owl:Class>
    


    <!-- http://purl.org/auto/l2_core#Road_Side_Vegetation -->

    <owl:Class rdf:about="http://purl.org/auto/l2_core#Road_Side_Vegetation">
        <rdfs:subClassOf rdf:resource="http://purl.org/auto/l2_core#Vegetation"/>
        <rdfs:comment xml:lang="en">A vegetation that is placed alongside the road or on specially designated vegetation strips on roads.</rdfs:comment>
        <rdfs:label xml:lang="de">Verkehrsbegleitgrün</rdfs:label>
    </owl:Class>
    


    <!-- http://purl.org/auto/l2_core#Roadside_Construction -->

    <owl:Class rdf:about="http://purl.org/auto/l2_core#Roadside_Construction">
        <rdfs:subClassOf rdf:resource="http://purl.org/auto/l2_core#L2_Entity"/>
        <rdfs:comment xml:lang="en">A human-made construction that is permanently installed on the road side, e.g. buildings and walls.</rdfs:comment>
        <rdfs:label xml:lang="de">Straßenrandbebauung</rdfs:label>
    </owl:Class>
    


    <!-- http://purl.org/auto/l2_core#Traffic_Support_System -->

    <owl:Class rdf:about="http://purl.org/auto/l2_core#Traffic_Support_System">
        <rdfs:subClassOf rdf:resource="http://purl.org/auto/l2_core#L2_Entity"/>
        <rdfs:comment xml:lang="en">A construction whose purpose it is to support the traffic e.g. by increasing safety but is not a major part of the road infrastructure, e.g. traffic lights and guard rails.</rdfs:comment>
        <rdfs:label xml:lang="de">Verkehrsunterstützendes_System</rdfs:label>
    </owl:Class>
    


    <!-- http://purl.org/auto/l2_core#Vegetation -->

    <owl:Class rdf:about="http://purl.org/auto/l2_core#Vegetation">
        <rdfs:subClassOf rdf:resource="http://purl.org/auto/l2_core#L2_Entity"/>
        <rdfs:label xml:lang="de">Vegetation</rdfs:label>
    </owl:Class>
    


    <!-- http://purl.org/auto/l2_core#Water_Body -->

    <owl:Class rdf:about="http://purl.org/auto/l2_core#Water_Body">
        <rdfs:subClassOf rdf:resource="http://purl.org/auto/l2_core#L2_Entity"/>
        <rdfs:subClassOf rdf:resource="http://purl.org/auto/physics#Liquid"/>
        <rdfs:comment xml:lang="en">A human-made or natural accumulation of larger amounts of water that are mostly permanent (i.e. not a puddle etc.).</rdfs:comment>
        <rdfs:label xml:lang="de">Gewässer</rdfs:label>
    </owl:Class>
    


    <!-- http://purl.org/auto/physics#Illumination_Source -->

    <owl:Class rdf:about="http://purl.org/auto/physics#Illumination_Source"/>
</rdf:RDF>



<!-- Generated by the OWL API (version 4.5.9.2019-02-01T07:24:44Z) https://github.com/owlcs/owlapi -->

