<?xml version="1.0"?>
<rdf:RDF xmlns="http://purl.org/auto/act#"
     xml:base="http://purl.org/auto/act"
     xmlns:dc="http://purl.org/dc/elements/1.1/"
     xmlns:act="http://purl.org/auto/act#"
     xmlns:owl="http://www.w3.org/2002/07/owl#"
     xmlns:rdf="http://www.w3.org/1999/02/22-rdf-syntax-ns#"
     xmlns:xml="http://www.w3.org/XML/1998/namespace"
     xmlns:xsd="http://www.w3.org/2001/XMLSchema#"
     xmlns:rdfs="http://www.w3.org/2000/01/rdf-schema#"
     xmlns:skos="http://www.w3.org/2004/02/skos/core#"
     xmlns:swrla="http://swrl.stanford.edu/ontologies/3.3/swrla.owl#"
     xmlns:terms="http://purl.org/dc/terms/"
     xmlns:physics="http://purl.org/auto/physics#">
    <owl:Ontology rdf:about="http://purl.org/auto/act">
        <owl:imports rdf:resource="http://purl.org/auto/perception"/>
        <owl:imports rdf:resource="http://www.w3.org/2006/time"/>
    </owl:Ontology>
    


    <!-- 
    ///////////////////////////////////////////////////////////////////////////////////////
    //
    // Object Properties
    //
    ///////////////////////////////////////////////////////////////////////////////////////
     -->

    


    <!-- http://purl.org/auto/act#changes_continuous_state_of -->

    <owl:ObjectProperty rdf:about="http://purl.org/auto/act#changes_continuous_state_of">
        <rdfs:subPropertyOf rdf:resource="http://purl.org/auto/act#changes_state_of"/>
        <rdfs:domain rdf:resource="http://purl.org/auto/act#Activity"/>
        <rdfs:range rdf:resource="http://www.w3.org/2002/07/owl#Thing"/>
        <rdfs:label xml:lang="de">aendert_kontinuierlichen_zustand_von</rdfs:label>
    </owl:ObjectProperty>
    


    <!-- http://purl.org/auto/act#changes_discrete_state_of -->

    <owl:ObjectProperty rdf:about="http://purl.org/auto/act#changes_discrete_state_of">
        <rdfs:subPropertyOf rdf:resource="http://purl.org/auto/act#changes_state_of"/>
        <rdfs:domain rdf:resource="http://purl.org/auto/act#Event"/>
        <rdfs:range rdf:resource="http://www.w3.org/2002/07/owl#Thing"/>
        <rdfs:label xml:lang="de">aendert_diskreten_zustand_von</rdfs:label>
    </owl:ObjectProperty>
    


    <!-- http://purl.org/auto/act#changes_state_of -->

    <owl:ObjectProperty rdf:about="http://purl.org/auto/act#changes_state_of">
        <rdfs:domain>
            <owl:Class>
                <owl:unionOf rdf:parseType="Collection">
                    <rdf:Description rdf:about="http://purl.org/auto/act#Activity"/>
                    <rdf:Description rdf:about="http://purl.org/auto/act#Event"/>
                </owl:unionOf>
            </owl:Class>
        </rdfs:domain>
        <rdfs:range rdf:resource="http://www.w3.org/2002/07/owl#Thing"/>
        <rdfs:label xml:lang="de">aendert_zustand_von</rdfs:label>
    </owl:ObjectProperty>
    


    <!-- http://purl.org/auto/act#conducted_by -->

    <owl:ObjectProperty rdf:about="http://purl.org/auto/act#conducted_by">
        <owl:inverseOf rdf:resource="http://purl.org/auto/act#conducts"/>
        <rdfs:domain rdf:resource="http://purl.org/auto/act#Activity"/>
        <rdfs:range rdf:resource="http://purl.org/auto/act#Actor"/>
        <rdfs:comment xml:lang="en">An activity can be conducted by (a set of) actors that are causative for the activity to happen. 
Example: A left turn on an intersection is conducted by the vehicle turning left.</rdfs:comment>
        <rdfs:label xml:lang="de">ausgefuehrt_von</rdfs:label>
    </owl:ObjectProperty>
    


    <!-- http://purl.org/auto/act#conducts -->

    <owl:ObjectProperty rdf:about="http://purl.org/auto/act#conducts">
        <rdfs:domain rdf:resource="http://purl.org/auto/act#Actor"/>
        <rdfs:range rdf:resource="http://purl.org/auto/act#Activity"/>
        <rdfs:label xml:lang="de">fuehrt_aus</rdfs:label>
    </owl:ObjectProperty>
    


    <!-- http://purl.org/auto/act#has_intent -->

    <owl:ObjectProperty rdf:about="http://purl.org/auto/act#has_intent">
        <rdfs:domain rdf:resource="http://purl.org/auto/act#Actor"/>
        <rdfs:range rdf:resource="http://purl.org/auto/act#Intent"/>
        <rdfs:label xml:lang="de">hat_intention</rdfs:label>
    </owl:ObjectProperty>
    


    <!-- http://purl.org/auto/act#has_participant -->

    <owl:ObjectProperty rdf:about="http://purl.org/auto/act#has_participant">
        <owl:inverseOf rdf:resource="http://purl.org/auto/act#participates_in"/>
        <rdfs:domain rdf:resource="http://purl.org/auto/act#Activity"/>
        <rdfs:range rdf:resource="http://www.w3.org/2002/07/owl#Thing"/>
        <rdfs:comment xml:lang="en">Things can actively or passively participate in activities. Those things are not causative for the activity (i.e. are not the main driver), but play a certain role in it. 
Example: A driving vehicle is passing three parking vehicles, which are the participants of the driving vehicle&apos;s passing activity.</rdfs:comment>
        <rdfs:label xml:lang="de">hat_teilnehmer</rdfs:label>
    </owl:ObjectProperty>
    


    <!-- http://purl.org/auto/act#induced_by_event -->

    <owl:ObjectProperty rdf:about="http://purl.org/auto/act#induced_by_event">
        <owl:inverseOf rdf:resource="http://purl.org/auto/act#leads_to_activity"/>
        <rdfs:domain rdf:resource="http://purl.org/auto/act#Activity"/>
        <rdfs:range rdf:resource="http://purl.org/auto/act#Event"/>
        <rdfs:label xml:lang="de">induziert_von_ereignis</rdfs:label>
    </owl:ObjectProperty>
    


    <!-- http://purl.org/auto/act#leads_to_activity -->

    <owl:ObjectProperty rdf:about="http://purl.org/auto/act#leads_to_activity">
        <rdfs:domain rdf:resource="http://purl.org/auto/act#Event"/>
        <rdfs:range rdf:resource="http://purl.org/auto/act#Activity"/>
        <rdfs:label xml:lang="de">fuehrt_zu_aktivitaet</rdfs:label>
    </owl:ObjectProperty>
    


    <!-- http://purl.org/auto/act#participates_in -->

    <owl:ObjectProperty rdf:about="http://purl.org/auto/act#participates_in">
        <rdfs:domain rdf:resource="http://www.w3.org/2002/07/owl#Thing"/>
        <rdfs:range rdf:resource="http://purl.org/auto/act#Activity"/>
        <rdfs:label xml:lang="de">nimmt_teil_an</rdfs:label>
    </owl:ObjectProperty>
    


    <!-- 
    ///////////////////////////////////////////////////////////////////////////////////////
    //
    // Classes
    //
    ///////////////////////////////////////////////////////////////////////////////////////
     -->

    


    <!-- http://purl.org/auto/act#Activity -->

    <owl:Class rdf:about="http://purl.org/auto/act#Activity">
        <rdfs:subClassOf rdf:resource="http://www.w3.org/2006/time#Interval"/>
        <rdfs:comment xml:lang="en">An activity is a description of the (possibly continuous) temporal change of a related entity. It can be divided into sub-activities. Activities may induce an infinite number of scenes describing the temporal behavior of the related entity.</rdfs:comment>
        <rdfs:comment xml:lang="en">Examples:
- &quot;Right turn&quot; activity, conducted by the ego, which is divided into 3 sub-activities: &quot;turning steering wheel to defined angle&quot;, &quot;conducting turn&quot;, &quot;turning steering wheel to 0° angle&quot;
- &quot;Emergency brake&quot; of a vehicle e in which the following continuous behaviors apply: e.a = e.a_min and e.v&apos; = e.a
- &quot;Rain storm&quot; with an intensity constrained to be in [30, 50] mm/h</rdfs:comment>
        <rdfs:label xml:lang="de">Aktivität</rdfs:label>
    </owl:Class>
    


    <!-- http://purl.org/auto/act#Actor -->

    <owl:Class rdf:about="http://purl.org/auto/act#Actor">
        <rdfs:subClassOf rdf:resource="http://purl.org/auto/perception#Observer"/>
        <rdfs:comment xml:lang="en">An observer that has an intent and is able to act upon that intent. Thus, it has not only a &quot;perceive&quot;, but also an &quot;act&quot; component.</rdfs:comment>
        <rdfs:comment xml:lang="en">Examples:
- &quot;Car driver&quot;
- &quot;Pedestrian&quot;
- &quot;Automated vehicle&quot;
- &quot;Pet&quot;</rdfs:comment>
        <rdfs:label xml:lang="de">Akteur</rdfs:label>
    </owl:Class>
    


    <!-- http://purl.org/auto/act#Event -->

    <owl:Class rdf:about="http://purl.org/auto/act#Event">
        <rdfs:subClassOf rdf:resource="http://www.w3.org/2006/time#Instant"/>
        <rdfs:comment xml:lang="en">A temporal instant that describes a discrete state change of an entity. It has a temporal extent of 0 and can lead to a subsequent activity conducted by the related entity. It can be divided into sub-events.</rdfs:comment>
        <rdfs:comment xml:lang="en">Examples:
- Initiating emergency brake: ego changes from state &quot;straight drive&quot; into &quot;emergency brake&quot;
- Traffic light changes to &quot;green&quot;</rdfs:comment>
        <rdfs:label xml:lang="de">Ereignis</rdfs:label>
    </owl:Class>
    


    <!-- http://purl.org/auto/act#Intent -->

    <owl:Class rdf:about="http://purl.org/auto/act#Intent">
        <rdfs:comment xml:lang="en">An actor can have an intention that guides its behavior.</rdfs:comment>
        <rdfs:comment xml:lang="en">Examples:
- &quot;Reaching eastern arm of the crossing&quot;
- &quot;Safe driving&quot;
- &quot;Having fun&quot;</rdfs:comment>
        <rdfs:label xml:lang="de">Intention</rdfs:label>
    </owl:Class>
    


    <!-- http://purl.org/auto/perception#Observer -->

    <owl:Class rdf:about="http://purl.org/auto/perception#Observer"/>
</rdf:RDF>



<!-- Generated by the OWL API (version 4.5.9.2019-02-01T07:24:44Z) https://github.com/owlcs/owlapi -->

